@prefix ppb: <http://parliament.uk/ontologies/parliamentary-bloc/> . 
@prefix xsd: <http://www.w3.org/2001/XMLSchema#> . 
@prefix rdf: <http://www.w3.org/1999/02/22-rdf-syntax-ns#> .
@prefix dcterms: <http://purl.org/dc/terms/> .
@prefix owl:     <http://www.w3.org/2002/07/owl#> .
@prefix rdfs:    <http://www.w3.org/2000/01/rdf-schema#> .
@prefix foaf:	<http://xmlns.com/foaf/0.1/> .

<http://parliament.uk/ontologies/parliamentary-bloc/> 
    rdf:type owl:Ontology ;
    dcterms:title "Parliamentary bloc ontology"@en ;
    dcterms:created "2017-06-14"^^xsd:date ;
	dcterms:rights "Open Parliament Licence v3.0"@en ;
    dcterms:description "A model describing the whipping of a Member to a parliamentary party or the affiliation of a Member with a parliamentary bloc. A parliamentary bloc may be a parliamentary party, or may be a non-political group, for example: the Crossbenchers in the House of Lords."@en ;
	foaf:depiction <https://ukparliament.github.io/ontologies/parliamentary-bloc/parliamentary-bloc.svg> ;
	foaf:maker
		[ foaf:name "David Beamish" ],
		[ foaf:name "Robert Brook"; foaf:homepage <https://robert-brook.com/> ],
		[ foaf:name "Oli Hawkins"; foaf:homepage <https://olihawkins.com/> ],
		[ foaf:name "Lucinda Maer" ],
		[ foaf:name "Ned Morrell" ],
		[ foaf:name "Silver Oliver" ],
		[ foaf:name "Michael Smethurst"; foaf:homepage <https://smethur.st/> ],
	    [ foaf:name "Anya Somerville" ].


#######  Classes #####
	
ppb:PoliticalParty rdf:type owl:Class ;
	rdfs:label "Political party"@en ;
	rdfs:comment "An organisation registered by the Electoral Commission as a political party."@en ;
	rdfs:isDefinedBy <http://parliament.uk/ontologies/parliamentary-bloc/> .
	
ppb:Sistership rdf:type owl:Class ;
	rdfs:label "Sistership"@en ;
	rdfs:comment "A relationship between political parties which have agreed to co-operate, for example: Labour and the SDLP being sister parties."@en ;
	rdfs:isDefinedBy <http://parliament.uk/ontologies/parliamentary-bloc/> .

ppb:ElectoralPact rdf:type owl:Class ;
	rdfs:label "Electoral pact"@en ;
	rdfs:comment "A relationship between two or more political parties which have agreed that only one party forming part of that agreement will field a candidate in a given constituency, for example: the Unite to Remain electoral pact between the Liberal Democrats, the Green Party of England and Wales, and Plaid Cymru in the 2019 general election."@en ;
	rdfs:isDefinedBy <http://parliament.uk/ontologies/parliamentary-bloc/> .
	
ppb:ParliamentaryBloc rdf:type owl:Class ;
	rdfs:label "Parliamentary bloc"@en ;
	rdfs:comment "A group of Members of Parliament sharing the same affiliation, for example: a parliamentary party, the bishops or Crossbenchers in the House of Lords."@en ;
	rdfs:isDefinedBy <http://parliament.uk/ontologies/parliamentary-bloc/> .
	
ppb:ParliamentaryParty rdf:type owl:Class ;
	rdfs:subClassOf ppb:ParliamentaryBloc ;
	rdfs:label "Parliamentary party"@en ;
	rdfs:comment "A group of Members of Parliament accepting the same party whip."@en ;
	rdfs:isDefinedBy <http://parliament.uk/ontologies/parliamentary-bloc/> .
	
ppb:ParliamentaryAgreement rdf:type owl:Class ;
	rdfs:label "Parliamentary agreement"@en ;
	rdfs:comment "An agreement between two or more parliamentary parties to cooperate within Parliament, for example: a confidence and supply or coalition agreement."@en ;
	rdfs:isDefinedBy <http://parliament.uk/ontologies/parliamentary-bloc/> .
	
ppb:Affiliation rdf:type owl:Class ;
	rdfs:label "Affiliation"@en ;
	rdfs:comment "An affiliation to a parliamentary bloc held by a Member between two dates, for example: a peer being affiliated to the Crossbenchers, or an affiliation to the Co-operative Party whilst accepting the whip of the Labour Party."@en ;
	rdfs:isDefinedBy <http://parliament.uk/ontologies/parliamentary-bloc/> .

ppb:MemberWhipping rdf:type owl:Class ;
	rdfs:subClassOf ppb:Affiliation ;
	rdfs:label "Member whipping"@en ;
	rdfs:comment "The acceptance of a whip to a parliamentary party by a Member between two dates."@en ;
	rdfs:isDefinedBy <http://parliament.uk/ontologies/parliamentary-bloc/> .
	
ppb:Person rdf:type owl:Class ;
	rdfs:label "Person"@en ;
	rdfs:comment "A person."@en ;
	rdfs:isDefinedBy <http://parliament.uk/ontologies/parliamentary-bloc/> .
	

	
##### Object properties ####

ppb:sistershipOf rdf:type owl:ObjectProperty ;
	rdfs:label "Sistership of"@en ;
	rdfs:comment "Relates a sistership to a political party forming part of that sistership, for example: the sistership of Labour and the SDLP relating to the SDLP. A sistership of is to one political party."@en ;
	rdfs:domain ppb:Sistership ;
	rdfs:range ppb:PoliticalParty ;
	rdfs:isDefinedBy <http://parliament.uk/ontologies/parliamentary-bloc/> .
	
ppb:electoralPactOf rdf:type owl:ObjectProperty ;
	rdfs:label "Electoral pact of"@en ;
	rdfs:comment "Relates an electoral pact to a political party forming part of that pact, for example: the Unite to Remain pact relating to Plaid Cymru. An electoral pact of is to one political party."@en ;
	rdfs:domain ppb:ElectoralPact ;
	rdfs:range ppb:PoliticalParty ;
	rdfs:isDefinedBy <http://parliament.uk/ontologies/parliamentary-bloc/> .
	
ppb:isParliamentaryPartyOf rdf:type owl:ObjectProperty ;
	rdfs:label "Is parliamentary party of"@en ;
	rdfs:comment "Relates a parliamentary party to that political party as registered with the Electoral Commission. A parliamentary party is related to one political party."@en ;
	rdfs:domain ppb:ParliamentaryParty ;
	rdfs:range ppb:PoliticalParty ;
	rdfs:isDefinedBy <http://parliament.uk/ontologies/parliamentary-bloc/> .
	
ppb:parliamentaryAgreementOf rdf:type owl:ObjectProperty ;
	rdfs:label "Parliamentary agreement of"@en ;
	rdfs:comment "Relates a parliamentary agreement to a parliamentary party being part of that agreement, for example: the coalition agreement between the Conservatives and the Liberal Democrats relating to the Liberal Democrats. A parliamentary agreement of is to one parliamentary party."@en ;
	rdfs:domain ppb:ParliamentaryAgreement ;
	rdfs:range ppb:ParliamentaryParty ;
	rdfs:isDefinedBy <http://parliament.uk/ontologies/parliamentary-bloc/> .
	
ppb:toParliamentaryBloc rdf:type owl:ObjectProperty ;
	rdfs:label "To parliamentary bloc"@en ;
	rdfs:comment "Relates an affiliation of a Member to a parliamentary bloc to that parliamentary bloc, for example: from an affiliation of a Crossbencher to the Crossbenchers in the House of Lords. An affiliation is to one parliamentary bloc."@en ;
	rdfs:domain ppb:Affiliation ;
	rdfs:range ppb:ParliamentaryBloc ;
	rdfs:isDefinedBy <http://parliament.uk/ontologies/parliamentary-bloc/> .
	
ppb:whippedTo rdf:type owl:ObjectProperty ;
	rdfs:label "Whipped to"@en ;
	rdfs:comment "Relates a whipping of a Member to a parliamentary party to that parliamentary party, for example: between the whipping of a Liberal Member and the parliamentary Liberal Party. A whipping is to one parliamentary party."@en ;
	rdfs:domain ppb:MemberWhipping ;
	rdfs:range ppb:ParliamentaryParty ;
	rdfs:isDefinedBy <http://parliament.uk/ontologies/parliamentary-bloc/> .
	
ppb:acceptedBy rdf:type owl:ObjectProperty ;
	rdfs:label "Accepted by"@en ;
	rdfs:comment "Relates a whipping of a person to that person: the acceptance of a whip by a Member. A whipping is of one person."@en ;
	rdfs:domain ppb:MemberWhipping ;
	rdfs:range ppb:Person ;
	rdfs:isDefinedBy <http://parliament.uk/ontologies/parliamentary-bloc/> .

						