@prefix ppb: <http://parliament.uk/ontologies/parliamentary-bloc/> . 
@prefix xsd: <http://www.w3.org/2001/XMLSchema#> . 
@prefix rdf: <http://www.w3.org/1999/02/22-rdf-syntax-ns#> .
@prefix dcterms: <http://purl.org/dc/terms/> .
@prefix owl:     <http://www.w3.org/2002/07/owl#> .
@prefix rdfs:    <http://www.w3.org/2000/01/rdf-schema#> .
@prefix foaf:	<http://xmlns.com/foaf/0.1/> .

<http://parliament.uk/ontologies/parliamentary-bloc/> 
    rdf:type owl:Ontology ;
    dcterms:title "Parliamentary bloc ontology"@en ;
    dcterms:created "2017-06-14"^^xsd:date ;
	dcterms:rights "Open Parliament Licence v3.0"@en ;
    dcterms:description "A model describing the whipping of a Member to a parliamentary party or the affiliation of a Member with a parliamentary bloc. A parliamentary bloc may be a parliamentary party, or may be a non-political group, for example: the Crossbenchers in the House of Lords."@en ;
	foaf:depiction <https://ukparliament.github.io/ontologies/parliamentary-bloc/parliamentary-bloc.svg> ;
	foaf:maker
		[ foaf:name "David Beamish" ],
		[ foaf:name "Robert Brook"; foaf:homepage <https://robert-brook.com/> ],
		[ foaf:name "Oli Hawkins"; foaf:homepage <https://olihawkins.com/> ],
		[ foaf:name "Lucinda Maer" ],
		[ foaf:name "Ned Morrell" ],
		[ foaf:name "Silver Oliver" ],
		[ foaf:name "Michael Smethurst"; foaf:homepage <https://smethur.st/> ],
	    [ foaf:name "Anya Somerville" ].


#######  Classes #####
	
ppb:PoliticalParty rdf:type owl:Class ;
	rdfs:label "Political party"@en ;
	rdfs:comment "An organisation registered by the Electoral Commission as a political party."@en ;
	rdfs:isDefinedBy <http://parliament.uk/ontologies/parliamentary-bloc/> .
	
ppb:Sistership rdf:type owl:Class ;
	rdfs:label "Sistership"@en ;
	rdfs:comment "xxxx - A relationship between political parties who have agreed to co-operate."@en ;
	rdfs:isDefinedBy <http://parliament.uk/ontologies/parliamentary-bloc/> .

ppb:Pact rdf:type owl:Class ;
	rdfs:label "Pact"@en ;
	rdfs:comment "xxxx - An agreement between two or more political parties."@en ;
	rdfs:isDefinedBy <http://parliament.uk/ontologies/parliamentary-bloc/> .
	
ppb:ParliamentaryBloc rdf:type owl:Class ;
	rdfs:label "Parliamentary bloc"@en ;
	rdfs:comment "A group of Members of Parliament sharing the same affiliation, for example: a parliamentary party, the bishops or Crossbenchers in the House of Lords."@en ;
	rdfs:isDefinedBy <http://parliament.uk/ontologies/parliamentary-bloc/> .
	
ppb:ParliamentaryParty rdf:type owl:Class ;
	rdfs:subClassOf ppb:ParliamentaryBloc ;
	rdfs:label "Parliamentary party"@en ;
	rdfs:comment "A group of Members of Parliament accepting the same party whip."@en ;
	rdfs:isDefinedBy <http://parliament.uk/ontologies/parliamentary-bloc/> .
	
ppb:ParliamentaryAgreement rdf:type owl:Class ;
	rdfs:label "Parliamentary agreement"@en ;
	rdfs:comment "xxxxx - An agreement between two or more parliamentary parties to cooperate within Parliament, for example: a confidence and supply or coalition agreement."@en ;
	rdfs:isDefinedBy <http://parliament.uk/ontologies/parliamentary-bloc/> .
	
ppb:Affiliation rdf:type owl:Class ;
	rdfs:label "Affiliation"@en ;
	rdfs:comment "An affiliation to a parliamentary bloc held by a Member between two dates, for example: a peer being affiliated to the Crossbenchers, or an affiliation to the Co-operative Party whilst accepting the whip of the Labour Party."@en ;
	rdfs:isDefinedBy <http://parliament.uk/ontologies/parliamentary-bloc/> .

ppb:MemberWhipping rdf:type owl:Class ;
	rdfs:subClassOf ppb:Affiliation ;
	rdfs:label "Member whipping"@en ;
	rdfs:comment "The acceptance of a whip to a parliamentary party by a Member between two dates."@en ;
	rdfs:isDefinedBy <http://parliament.uk/ontologies/parliamentary-bloc/> .
	
ppb:Person rdf:type owl:Class ;
	rdfs:label "Person"@en ;
	rdfs:comment "A person."@en ;
	rdfs:isDefinedBy <http://parliament.uk/ontologies/parliamentary-bloc/> .
	

	
##### Object properties ####

ppb:sistershipOf rdf:type owl:ObjectProperty ;
	rdfs:label "Sistership of"@en ;
	rdfs:comment "xxxx - The relationship between a political party and the participation of that party within a sistership."@en ;
	rdfs:domain ppb:Sistership ;
	rdfs:range ppb:PoliticalParty ;
	rdfs:isDefinedBy <http://parliament.uk/ontologies/parliamentary-bloc/> .

ppb:pactHasParty rdf:type owl:ObjectProperty ;
	rdfs:label "Pact has party"@en ;
	rdfs:comment "xxxx - The relationship between a political party and the inclusion of that party within a pact."@en ;
	rdfs:domain ppb:Pact ;
	rdfs:range ppb:PoliticalParty ;
	rdfs:isDefinedBy <http://parliament.uk/ontologies/parliamentary-bloc/> .
	
ppb:isParliamentaryPartyOf rdf:type owl:ObjectProperty ;
	rdfs:label "Is parliamentary party of"@en ;
	rdfs:comment "The relationship between a party within Parliament and that party as registered with the Electoral Commission."@en ;
	rdfs:domain ppb:ParliamentaryParty ;
	rdfs:range ppb:PoliticalParty ;
	rdfs:isDefinedBy <http://parliament.uk/ontologies/parliamentary-bloc/> .
	
ppb:agreementOf rdf:type owl:ObjectProperty ;
	rdfs:label "Agreement of"@en ;
	rdfs:comment "xxxxx - The relationship between a parliamentary party and the participation of that party in an agreement."@en ;
	rdfs:domain ppb:ParliamentaryAgreement ;
	rdfs:range ppb:ParliamentaryParty ;
	rdfs:isDefinedBy <http://parliament.uk/ontologies/parliamentary-bloc/> .
	
ppb:toParliamentaryBloc rdf:type owl:ObjectProperty ;
	rdfs:label "To parliamentary bloc"@en ;
	rdfs:comment "The relationship between an affiliation of a Member to a parliamentary bloc and that parliamentary bloc, for example: from an affiliation of a Crossbencher to the Crossbenchers in the House of Lords. An affiliation is to one parliamentary bloc."@en ;
	rdfs:domain ppb:Affiliation ;
	rdfs:range ppb:ParliamentaryBloc ;
	rdfs:isDefinedBy <http://parliament.uk/ontologies/parliamentary-bloc/> .
	
ppb:whippedTo rdf:type owl:ObjectProperty ;
	rdfs:label "Whipped to"@en ;
	rdfs:comment "The relationship between a whipping of a Member to a parliamentary party and that parliamentary party, for example: between the whipping of a Liberal Member and the parliamentary Liberal Party. A whipping is to one parliamentary party."@en ;
	rdfs:domain ppb:MemberWhipping ;
	rdfs:range ppb:ParliamentaryParty ;
	rdfs:isDefinedBy <http://parliament.uk/ontologies/parliamentary-bloc/> .
	
ppb:acceptedBy rdf:type owl:ObjectProperty ;
	rdfs:label "Accepted by"@en ;
	rdfs:comment "The relationship between a whipping of a person and that person: the acceptance of a whip by a Member. A whipping is of one person."@en ;
	rdfs:domain ppb:MemberWhipping ;
	rdfs:range ppb:Person ;
	rdfs:isDefinedBy <http://parliament.uk/ontologies/parliamentary-bloc/> .

						