@prefix pbi: <http://parliament.uk/ontologies/business-item/> . 
@prefix xsd: <http://www.w3.org/2001/XMLSchema#> . 
@prefix rdf: <http://www.w3.org/1999/02/22-rdf-syntax-ns#> .
@prefix dcterms: <http://purl.org/dc/terms/> .
@prefix owl:     <http://www.w3.org/2002/07/owl#> .
@prefix rdfs:    <http://www.w3.org/2000/01/rdf-schema#> .
@prefix foaf:	<http://xmlns.com/foaf/0.1/> .

<http://parliament.uk/ontologies/business-item/> 
    rdf:type owl:Ontology ;
    dcterms:title "Business item ontology"@en ;
    dcterms:created "2018-10-13"^^xsd:date ;
	dcterms:rights "Open Parliament Licence v3.0"@en ;
    dcterms:description "A model describing items of business taking place in Parliament or outside Parliament - as part of a process involving Parliament - and their scheduling."@en ;
	foaf:depiction <https://ukparliament.github.io/ontologies/business-item/business-item.png> ;
	foaf:maker
		[ foaf:name "Robert Brook"; foaf:homepage <https://robert-brook.com/> ],
		[ foaf:name "Silver Oliver" ],
		[ foaf:name "Michael Smethurst"; foaf:homepage <http://smethur.st/> ],
	   	[ foaf:name "Anya Somerville" ].


#######  Classes ##### 	

pbi:BusinessItem rdf:type owl:Class ;
	rdfs:label "Business item"@en ;
	rdfs:comment "An item of business conducted either within or outside Parliament. For example: a second reading debate, the tabling of an early day motion, a laying of a paper or the making of a statutory instrument by a government minister."@en ;
	rdfs:isDefinedBy <http://parliament.uk/ontologies/business-item/> .

pbi:BusinessItemSeries rdf:type owl:Class ;
	rdfs:label "Business item series"@en ;
	rdfs:comment "A series of regularly recurring business items. For example: questions to the Department of Health and Social Care."@en ;
	rdfs:isDefinedBy <http://parliament.uk/ontologies/business-item/> .

pbi:BusinessItemType rdf:type owl:Class ;
	rdfs:label "Business item type"@en ;
	rdfs:comment "The type of a business item. For example: a committee visit, a committee evidence session or a chamber debate."@en ;
	rdfs:isDefinedBy <http://parliament.uk/ontologies/business-item/> .

pbi:Document rdf:type owl:Class ;
	rdfs:label "Document"@en ;
	rdfs:comment "A document being a FRBR work."@en ;
	rdfs:isDefinedBy <http://parliament.uk/ontologies/business-item/> .
	
pbi:CalendaredEvent rdf:type owl:Class ;
	rdfs:label "Calendared event"@en ;
	rdfs:comment "An event during which business items happen."@en ;
	rdfs:isDefinedBy <http://parliament.uk/ontologies/business-item/> .
	
pbi:Place rdf:type owl:Class ;
	rdfs:label "Place"@en ;
	rdfs:comment "A place named in a geography."@en ;
	rdfs:isDefinedBy <http://parliament.uk/ontologies/business-item/> .



##### Object properties ####

pbi:partOfSeries rdf:type owl:ObjectProperty ;
	rdfs:label "Part of series"@en ;
	rdfs:comment "Relates a business item to a business item series it is part of."@en ;
	rdfs:domain pbi:BusinessItem ;
	rdfs:range pbi:BusinessItemSeries ;
	rdfs:isDefinedBy <http://parliament.uk/ontologies/business-item/> .
	
pbi:containsBusinessItem rdf:type owl:ObjectProperty ;
	rdfs:label "Contains business item"@en ;
	rdfs:comment "Allows a business item to be nested inside another business item. For example, a committee meeting during a committee visit."@en ;
	rdfs:domain pbi:BusinessItem ;
	rdfs:range pbi:BusinessItem ;
	rdfs:isDefinedBy <http://parliament.uk/ontologies/business-item/> .
	
pbi:hasBusinessItemType rdf:type owl:ObjectProperty ;
	rdfs:label "Has business item type"@en ;
	rdfs:comment "Relates a business item to its type."@en ;
	rdfs:domain pbi:BusinessItem ;
	rdfs:range pbi:BusinessItemType ;
	rdfs:isDefinedBy <http://parliament.uk/ontologies/business-item/> .
	
pbi:recordOf rdf:type owl:ObjectProperty ;
	rdfs:label "Record of"@en ;
	rdfs:comment "Relates a document to the calendared event it records."@en ;
	rdfs:domain pbi:Document ;
	rdfs:range pbi:CalendaredEvent ;
	rdfs:isDefinedBy <http://parliament.uk/ontologies/business-item/> .
	
pbi:calendarisation rdf:type owl:ObjectProperty ;
	rdfs:label "Calendarisation"@en ;
	rdfs:comment "Describes the process of setting a time or date at which a business item is expected to take place."@en ;
	rdfs:domain pbi:BusinessItem ;
	rdfs:range pbi:CalendaredEvent ;
	rdfs:isDefinedBy <http://parliament.uk/ontologies/business-item/> .
	
pbi:followedBy rdf:type owl:ObjectProperty ;
	rdfs:label "Followed by"@en ;
	rdfs:comment "Relates a calendared event to a subsequent calendared event"@en ;
	rdfs:domain pbi:CalendaredEvent ;
	rdfs:range pbi:CalendaredEvent ;
	rdfs:isDefinedBy <http://parliament.uk/ontologies/business-item/> .
	
pbi:takesPlaceIn rdf:type owl:ObjectProperty ;
	rdfs:label "Takes place in"@en ;
	rdfs:comment "Relates a calendared event to the place it occurs."@en ;
	rdfs:domain pbi:CalendaredEvent ;
	rdfs:range pbi:Place ;
	rdfs:isDefinedBy <http://parliament.uk/ontologies/business-item/> .
	
					
	
##### Data properties ####	
			
pbi:notReached rdf:type owl:DatatypeProperty ;
	rdfs:label "Not reached"@en ;
	rdfs:comment "A boolean which is true when a calendared event was not reached or became unavailable for disposal."@en ;
	rdfs:domain pbi:CalendaredEvent ;
	rdfs:range xsd:boolean ;
	rdfs:isDefinedBy <http://parliament.uk/ontologies/business-item/> .
	
pbi:cancelledAt rdf:type owl:DatatypeProperty ;
	rdfs:label "Cancelled at"@en ;
	rdfs:comment "The time at which a calendared event was cancelled."@en ;
	rdfs:domain pbi:CalendaredEvent ;
	rdfs:range xsd:dateTime ;
	rdfs:isDefinedBy <http://parliament.uk/ontologies/business-item/> .

pbi:disposedOfAt rdf:type owl:DatatypeProperty ;
	rdfs:label "Disposed of at"@en ;
	rdfs:comment "The time at which an agenda item was completed."@en ;
	rdfs:domain pbi:CalendaredEvent ;
	rdfs:range xsd:dateTime ;
	rdfs:isDefinedBy <http://parliament.uk/ontologies/business-item/> .