@prefix ptable: <http://parliament.uk/ontologies/tabling/> . 
@prefix xsd: <http://www.w3.org/2001/XMLSchema#> . 
@prefix rdf: <http://www.w3.org/1999/02/22-rdf-syntax-ns#> .
@prefix dcterms: <http://purl.org/dc/terms/> .
@prefix owl:     <http://www.w3.org/2002/07/owl#> .
@prefix rdfs:    <http://www.w3.org/2000/01/rdf-schema#> .
@prefix foaf:	<http://xmlns.com/foaf/0.1/> .

<http://parliament.uk/ontologies/tabling/> 
    rdf:type owl:Ontology ;
    dcterms:title "Tabling ontology"@en ;
    dcterms:created "2017-12-01"^^xsd:date ;
	dcterms:rights "Open Parliament Licence v3.0"@en ;
    dcterms:description "A model describing the act of tabling by a Member."@en ;
	foaf:depiction <https://ukparliament.github.io/ontologies/tabling/tabling.svg> ;
	foaf:maker
		[ foaf:name "Robert Brook"; foaf:homepage <https://robert-brook.com/> ],
		[ foaf:name "Ned Morrell" ],
		[ foaf:name "Michael Smethurst"; foaf:homepage <http://smethur.st/> ],
		[ foaf:name "Anya Somerville" ] .


#######  Classes #####

ptable:Event rdf:type owl:Class ;
	rdfs:label "Event"@en ;
	rdfs:comment "An event taking place inside or outside Parliament. For example: a second reading debate, the tabling of an early day motion, a laying of a paper or the making of a statutory instrument by a government minister."@en ;
	rdfs:isDefinedBy <http://parliament.uk/ontologies/tabling/> .

ptable:Tabling rdf:type owl:Class ;
	rdfs:subClassOf ptable:Event ;
	rdfs:label "Tabling"@en ;
	rdfs:comment "The act of tabling a business item - being a question, a motion, an amendment or a committee membership nomination - into either the House of Commons or House of Lords. Members submit business items to the procedural offices. If accepted, the business item is considered to be tabled and will then appear as a written notice in the business papers for the next day. Each House has a Table Office where parliamentary questions, motions for debate and, in the Commons, early day motions are tabled. Amendments to bills are always tabled in the Public Bill Offices of each House."@en ;
	rdfs:isDefinedBy <http://parliament.uk/ontologies/tabling/> .
	
ptable:Session rdf:type owl:Class ;
	rdfs:label "Session"@en ;
	rdfs:comment "A period during which Parliament is able to conduct business on days of its choosing. A session is within a Parliament period. The first session of a Parliament begins on the same day as the Parliament period and ends on a day named in a subsequent prorogation proclamation. Subsequent sessions within the Parliament period begin and end on dates named in subsequent prorogation proclamations. The final session of a Parliament ends either with prorogation followed by dissolution or with dissolution. Session periods are the same for both Houses."@en ;
	rdfs:isDefinedBy <http://parliament.uk/ontologies/tabling/> .
	
ptable:House rdf:type owl:Class ;
	rdfs:label "House"@en ;
	rdfs:comment "A parliamentary House, for example: the House of Lords."@en ;
	rdfs:isDefinedBy <http://parliament.uk/ontologies/tabling/> .
	
ptable:TabledThing rdf:type owl:Class ;
	rdfs:label "Tabled thing"@en ;
	rdfs:comment "Any item of business which has been tabled, for example: a tabled motion, a tabled parliamentary question, a tabled amendment or a tabled committee membership nomination."@en ;
	rdfs:isDefinedBy <http://parliament.uk/ontologies/tabling/> .

ptable:Incumbency rdf:type owl:Class ;
	rdfs:label "Incumbency"@en ;
	rdfs:comment "The holding of a position by a person, including the time period for which this was the case. For example, Philip Hammond holding the position of Foreign Secretary between two dates."@en ;
	rdfs:isDefinedBy <http://parliament.uk/ontologies/tabling/> .
	
ptable:Withdrawal rdf:type owl:Class ;
	rdfs:subClassOf ptable:Event ;
	rdfs:label "Withdrawal"@en ;
	rdfs:comment "The act of withdrawing a tabled thing from a House."@en ;
	rdfs:isDefinedBy <http://parliament.uk/ontologies/tabling/> .
	
ptable:WithdrawnThing rdf:type owl:Class ;
	rdfs:subClassOf ptable:TabledThing ;
	rdfs:label "Withdrawn thing"@en ;
	rdfs:comment "A tabled thing which has been withdrawn."@en ;
	rdfs:isDefinedBy <http://parliament.uk/ontologies/tabling/> .
	
ptable:WrittenNotice rdf:type owl:Class ;
	rdfs:label "Written notice"@en ;
	rdfs:comment "Notice of an item of future business."@en ;
	rdfs:isDefinedBy <http://parliament.uk/ontologies/tabling/> .
	


##### Object properties ####

ptable:during rdf:type owl:ObjectProperty ;
	rdfs:label "During"@en ;
	rdfs:comment "Relates an act of tabling to the session in which the tabling takes place. An act of tabling is during one session."@en ;
	rdfs:domain ptable:Tabling ;
	rdfs:range ptable:Session ;
	rdfs:isDefinedBy <http://parliament.uk/ontologies/tabling/> .
	
ptable:intoHouse rdf:type owl:ObjectProperty ;
	rdfs:label "Into House"@en ;
	rdfs:comment "Relates an act of tabling to the House in which the tabling takes place. An act of tabling is into one House."@en ;
	rdfs:domain ptable:Tabling ;
	rdfs:range ptable:House ;
	rdfs:isDefinedBy <http://parliament.uk/ontologies/tabling/> .
	
ptable:tables rdf:type owl:ObjectProperty ;
	rdfs:label "Tables"@en ;
	rdfs:comment "Relates an act of tabling to the business item which is tabled. An act of tabling tables one tabled thing. A tabled thing is tabled by one act of tabling."@en ;
	rdfs:domain ptable:Tabling ;
	rdfs:range ptable:TabledThing ;
	rdfs:isDefinedBy <http://parliament.uk/ontologies/tabling/> .
	
ptable:tabledBy rdf:type owl:ObjectProperty ;
	rdfs:label "Tabled by"@en ;
	rdfs:comment "Relates an act of tabling to the incumbency of the Member tabling. An act of tabling is by one incumbent Member."@en ;
	rdfs:domain ptable:Tabling ;
	rdfs:range ptable:Incumbency ;
	rdfs:isDefinedBy <http://parliament.uk/ontologies/tabling/> .

ptable:withdraws rdf:type owl:ObjectProperty ;
	rdfs:label "Withdraws"@en ;
	rdfs:comment "Relates an act of withdrawal to the tabled thing withdrawn by the act of withdrawal. An act of withdrawal withdraws one tabled thing. A tabled thing is withdrawn by one act of tabling, or none."@en ;
	rdfs:domain ptable:Withdrawal ;
	rdfs:range ptable:TabledThing ;
	rdfs:isDefinedBy <http://parliament.uk/ontologies/tabling/> .

ptable:resultsIn rdf:type owl:ObjectProperty ;
	rdfs:label "Results in"@en ;
	rdfs:comment "Relates an act of withdrawal to the resulting withdrawn thing. An act of withdrawal results in one withdrawn thing. A withdrawn thing results from one act of withdrawal."@en ;
	rdfs:domain ptable:Withdrawal ;
	rdfs:range ptable:WithdrawnThing ;
	rdfs:isDefinedBy <http://parliament.uk/ontologies/tabling/> .
	
ptable:replaces rdf:type owl:ObjectProperty ;
	rdfs:label "Replaces"@en ;
	rdfs:comment "Relates a tabled thing to the withdrawn thing it replaces. A withdrawn thing is replaced by one tabled thing, or none."@en ;
	rdfs:domain ptable:TabledThing ;
	rdfs:range ptable:WithdrawnThing ;
	rdfs:isDefinedBy <http://parliament.uk/ontologies/tabling/> .
	
ptable:givesNotice rdf:type owl:ObjectProperty ;
	rdfs:label "Gives notice"@en ;
	rdfs:comment "Relates an act of tabling to a written notice. An act of tabling results in one written notice."@en ;
	rdfs:domain ptable:Tabling ;
	rdfs:range ptable:WrittenNotice ;
	rdfs:isDefinedBy <http://parliament.uk/ontologies/tabling/> .
	


##### Data properties ####	

ptable:tabledOn rdf:type owl:DatatypeProperty ;
	rdfs:label "Tabled on"@en ;
	rdfs:comment "Relates an act of tabling to the date on which that tabling takes place."@en ;
	rdfs:domain ptable:Tabling ;
	rdfs:range xsd:date ;
	rdfs:isDefinedBy <http://parliament.uk/ontologies/tabling/> .
	
ptable:isInterestDeclared rdf:type owl:DatatypeProperty ;
	rdfs:label "Is interest declared"@en ;
	rdfs:comment "Used to record if the tabling Member has declared a relevant interest."@en ;
	rdfs:domain ptable:Tabling ;
	rdfs:range xsd:boolean ;
	rdfs:isDefinedBy <http://parliament.uk/ontologies/tabling/> .
	
ptable:withdrawnOn rdf:type owl:DatatypeProperty ;
	rdfs:label "Withdrawn on"@en ;
	rdfs:comment "Relates an act of withdrawal to the date on which that withdrawal takes place."@en ;
	rdfs:domain ptable:Withdrawal ;
	rdfs:range xsd:date ;
	rdfs:isDefinedBy <http://parliament.uk/ontologies/tabling/> .