@prefix pma: <http://parliament.uk/ontologies/making-available/> . 
@prefix xsd: <http://www.w3.org/2001/XMLSchema#> . 
@prefix rdf: <http://www.w3.org/1999/02/22-rdf-syntax-ns#> .
@prefix dcterms: <http://purl.org/dc/terms/> .
@prefix owl:     <http://www.w3.org/2002/07/owl#> .
@prefix rdfs:    <http://www.w3.org/2000/01/rdf-schema#> .
@prefix foaf:	<http://xmlns.com/foaf/0.1/> .

<http://parliament.uk/ontologies/making-available/> 
    rdf:type owl:Ontology ;
    dcterms:title "Making available ontology"@en ;
    dcterms:created "2018-12-09"^^xsd:date ;
	dcterms:rights "Open Parliament Licence v3.0"@en ;
    dcterms:description "A model describing the act of making material available to a House and any subsequent withdrawal."@en;
	foaf:depiction <https://ukparliament.github.io/ontologies/making-available/making-available.svg> ;
	foaf:maker
		[ foaf:name "Jayne Bosworth" ],
		[ foaf:name "Robert Brook"; foaf:homepage <https://robert-brook.com/> ],
		[ foaf:name "Jack Dent" ],
		[ foaf:name "Mike Hennessy" ],
		[ foaf:name "Matt Korris" ],
		[ foaf:name "Ned Morrell" ],
		[ foaf:name "Michael Smethurst"; foaf:homepage <http://smethur.st/> ],
		[ foaf:name "Anya Somerville" ].


#######  Classes #####
	
pma:Session rdf:type owl:Class ;
	rdfs:label "Session"@en ;
	rdfs:comment "A period during which Parliament is able to conduct business on days of its choosing. A session is within a Parliament period. The first session of a Parliament begins on the same day as the Parliament period and ends on a day named in a subsequent prorogation proclamation. Subsequent sessions within the Parliament period begin and end on dates named in subsequent prorogation proclamations. The final session of a Parliament ends either with prorogation followed by dissolution or with dissolution. Session periods are the same for both Houses."@en ;
	rdfs:isDefinedBy <http://parliament.uk/ontologies/making-available/> .
	
pma:MakingAvailable rdf:type owl:Class ;
	rdfs:label "Making available"@en ;
	rdfs:comment "The act of making a thing available to a House or to a House by means of its Library."@en ;
	rdfs:isDefinedBy <http://parliament.uk/ontologies/making-available/> .
	
pma:Incumbency rdf:type owl:Class ;
	rdfs:label "Incumbency"@en ;
	rdfs:comment "The holding of a position by a person, including the time period for which this was the case. For example, Philip Hammond holding the position of Foreign Secretary between two dates."@en ;
	rdfs:isDefinedBy <http://parliament.uk/ontologies/making-available/> .
	
pma:House rdf:type owl:Class ;
	rdfs:label "House"@en ;
	rdfs:comment "A parliamentary House, for example: the House of Lords."@en ;
	rdfs:isDefinedBy <http://parliament.uk/ontologies/making-available/> .

pma:OrganisationAccountableToParliament rdf:type owl:Class ;
	rdfs:label "Organisation accountable to Parliament"@en ;
	rdfs:comment "An organisation accountable to Parliament: being a Government department, a Government organisation, a non-governmental organisation with a duty to answer questions or an organisation with a duty to lay papers."@en ;
	rdfs:isDefinedBy <http://parliament.uk/ontologies/making-available/> .

pma:PaperExpression rdf:type owl:Class ;
	rdfs:label "Paper expression"@en ;
	rdfs:comment "A paper made available to a House, being an expression of a paper work."@en ;
	rdfs:isDefinedBy <http://parliament.uk/ontologies/making-available/> .
	
pma:MadeAvailableThing rdf:type owl:Class ;
	rdfs:subClassOf pma:PaperExpression ;
	rdfs:label "Made available thing"@en ;
	rdfs:comment "A thing made available to a House or to a House by means of its Library."@en ;
	rdfs:isDefinedBy <http://parliament.uk/ontologies/making-available/> .

pma:Withdrawal rdf:type owl:Class ;
	rdfs:label "Withdrawal"@en ;
	rdfs:comment "The act of withdrawing a thing previously made available to a House or to a House by means of its Library."@en ;
	rdfs:isDefinedBy <http://parliament.uk/ontologies/making-available/> .
	
pma:WithdrawnThing rdf:type owl:Class ;
	rdfs:subClassOf pma:MadeAvailableThing ;
	rdfs:label "Withdrawn thing"@en ;
	rdfs:comment "A thing withdrawn from a House, having previously been made available to that House."@en ;
	rdfs:isDefinedBy <http://parliament.uk/ontologies/making-available/> .
	

	
	
#######  Object properties #####

pma:duringSession rdf:type owl:ObjectProperty ;
	rdfs:label "During session"@en ;
	rdfs:comment "Relates an act of making a thing available to the session during which that thing is made available. A thing made available during prorogation is during no session. An act of making available is during one session, or none."@en ;
	rdfs:domain pma:MakingAvailable ;
	rdfs:range pma:Session ;
	rdfs:isDefinedBy <http://parliament.uk/ontologies/making-available/> .
	
pma:intoSession rdf:type owl:ObjectProperty ;
	rdfs:label "Into session"@en ;
	rdfs:comment "Relates an act of making a thing available to the session into which that thing is made available. A thing made available during a prorogation is considered to be made available into the following session. An act of making available is into one session."@en ;
	rdfs:domain pma:MakingAvailable ;
	rdfs:range pma:Session ;
	rdfs:isDefinedBy <http://parliament.uk/ontologies/making-available/> .
	
pma:madeAvailableBy rdf:type owl:ObjectProperty ;
	rdfs:label "Made available by"@en ;
	rdfs:comment "Relates an act of making a thing available to the incumbency of the person in a position who makes that thing available, for example: the depositing of a paper by Philip Hammond as Foreign Secretary. An act of making available is by one person incumbent in one position."@en ;
	rdfs:domain pma:MakingAvailable ;
	rdfs:range pma:Incumbency ;
	rdfs:isDefinedBy <http://parliament.uk/ontologies/making-available/> .

pma:toHouse rdf:type owl:ObjectProperty ;
	rdfs:label "To House"@en ;
	rdfs:comment "Relates an act of making a thing available to the House in which that thing is made available. An act of making available is to one House. A thing may be made available to both Houses by means of two acts of making available."@en ;
	rdfs:domain pma:MakingAvailable ;
	rdfs:range pma:House ;
	rdfs:isDefinedBy <http://parliament.uk/ontologies/making-available/> .

pma:providedBy rdf:type owl:ObjectProperty ;
	rdfs:label "Provided by"@en ;
	rdfs:comment "Relates a thing made available to the organisation providing that thing. A thing made available is provided by one or more organisations, or none."@en ;
	rdfs:domain pma:MadeAvailableThing ;
	rdfs:range pma:OrganisationAccountableToParliament ;
	rdfs:isDefinedBy <http://parliament.uk/ontologies/making-available/> .
	
pma:makesAvailable rdf:type owl:ObjectProperty ;
	rdfs:label "Makes available"@en ;
	rdfs:comment "Relates an act of making a thing available to the thing being made available. The act of making available makes one thing available. A thing is made available by one act of making available."@en ;
	rdfs:domain pma:MakingAvailable ;
	rdfs:range pma:MadeAvailableThing ;
	rdfs:isDefinedBy <http://parliament.uk/ontologies/making-available/> .
	
pma:withdraws rdf:type owl:ObjectProperty ;
	rdfs:label "Withdraws"@en ;
	rdfs:comment "Relates an act of withdrawal to the made available thing being withdrawn. An act of withdrawal withdraws one made available thing. A made available thing is withdrawn by one act of withdrawal."@en ;
	rdfs:domain pma:Withdrawal ;
	rdfs:range pma:MadeAvailableThing ;
	rdfs:isDefinedBy <http://parliament.uk/ontologies/making-available/> .
	
pma:resultsIn rdf:type owl:ObjectProperty ;
	rdfs:label "Results in"@en ;
	rdfs:comment "Relates an act of withdrawal to the thing having been withdrawn. An act of withdrawal results in one withdrawn thing. A withdrawn thing is the result of one act of withdrawal."@en ;
	rdfs:domain pma:Withdrawal ;
	rdfs:range pma:WithdrawnThing ;
	rdfs:isDefinedBy <http://parliament.uk/ontologies/making-available/> .
	
pma:withdrawnByIncumbency rdf:type owl:ObjectProperty ;
	rdfs:label "Withdrawn by incumbency"@en ;
	rdfs:comment "Relates an act of withdrawal to the incumbency of a person in a position performing the withdrawal. An act of withdrawal is performed by one incumbency."@en ;
	rdfs:domain pma:Withdrawal ;
	rdfs:range pma:Incumbency ;
	rdfs:isDefinedBy <http://parliament.uk/ontologies/making-available/> .

pma:withdrawnByOrganisation rdf:type owl:ObjectProperty ;
	rdfs:label "Withdrawn by organisation"@en ;
	rdfs:comment "Relates an act of withdrawal to the organisation performing the withdrawal. An act of withdrawal is by one or more organisations, or none."@en ;
	rdfs:domain pma:Withdrawal ;
	rdfs:range pma:OrganisationAccountableToParliament ;
	rdfs:isDefinedBy <http://parliament.uk/ontologies/making-available/> .
	

				

#######  Data properties ##### 

pma:madeAvailableOn rdf:type owl:DatatypeProperty ;
	rdfs:label "Made available on"@en ;
	rdfs:comment "Relates an act of making a thing available to the date on which that thing was made available."@en ;
	rdfs:domain pma:MakingAvailable ;
	rdfs:range xsd:date ;
	rdfs:isDefinedBy <http://parliament.uk/ontologies/making-available/> .

pma:withdrawnOn rdf:type owl:DatatypeProperty ;
	rdfs:label "Withdrawn on"@en ;
	rdfs:comment "Relates an act of withdrawal to the date on which that thing was withdrawn."@en ;
	rdfs:domain pma:Withdrawal ;
	rdfs:range xsd:date ;
	rdfs:isDefinedBy <http://parliament.uk/ontologies/making-available/> .