@prefix pdep: <http://parliament.uk/ontologies/depositing/> . 
@prefix xsd: <http://www.w3.org/2001/XMLSchema#> . 
@prefix rdf: <http://www.w3.org/1999/02/22-rdf-syntax-ns#> .
@prefix dcterms: <http://purl.org/dc/terms/> .
@prefix owl:     <http://www.w3.org/2002/07/owl#> .
@prefix rdfs:    <http://www.w3.org/2000/01/rdf-schema#> .
@prefix foaf:	<http://xmlns.com/foaf/0.1/> .

<http://parliament.uk/ontologies/depositing/> 
    rdf:type owl:Ontology ;
    dcterms:title "Depositing ontology"@en ;
    dcterms:created "2022-12-01"^^xsd:date ;
	dcterms:rights "Open Parliament Licence v3.0"@en ;
    dcterms:description "A model describing the commitment to make and the making of a deposit in the Library of either House."@en ;
	foaf:depiction <https://ukparliament.github.io/ontologies/depositing/depositing.svg> ;
	foaf:maker 
		[ foaf:name "Robert Brook"; foaf:homepage <https://robert-brook.com/> ],
		[ foaf:name "Karen Cox" ],
		[ foaf:name "Andrew Dommett" ],
		[ foaf:name "John Greenhead" ],
		[ foaf:name "Ann Reilly" ],
		[ foaf:name "Michael Smethurst"; foaf:homepage <http://smethur.st/> ],
		[ foaf:name "Anya Somerville" ].




#######  Classes #####
	
pdep:MakingAvailable rdf:type owl:Class ;
	rdfs:label "Making available"@en ;
	rdfs:comment "The act of making a thing available to a House or to a House by means of its Library."@en ;
	rdfs:isDefinedBy <http://parliament.uk/ontologies/depositing/> .
	
pdep:PaperExpression rdf:type owl:Class ;
	rdfs:label "Paper expression"@en ;
	rdfs:comment "A paper made available to a House, being an expression of a paper work."@en ;
	rdfs:isDefinedBy <http://parliament.uk/ontologies/depositing/> .

pdep:MadeAvailableThing rdf:type owl:Class ;
	rdfs:label "Made available thing"@en ;
	rdfs:comment "A thing made available to a House or to a House by means of its Library."@en ;
	rdfs:isDefinedBy <http://parliament.uk/ontologies/depositing/> .
	
pdep:DepositedThing rdf:type owl:Class ;
	rdfs:subClassOf pdep:MadeAvailableThing ;
	rdfs:label "Deposited thing"@en ;
	rdfs:comment "A thing having been deposited in a Library of a House."@en ;
	rdfs:isDefinedBy <http://parliament.uk/ontologies/depositing/> .
	
pdep:Depositing rdf:type owl:Class ;
	rdfs:subClassOf pdep:MakingAvailable ;
	rdfs:label "Depositing"@en ;
	rdfs:comment "The act of placing a thing in the Library of either House."@en ;
	rdfs:isDefinedBy <http://parliament.uk/ontologies/depositing/> .
	
pdep:DepositedPaper rdf:type owl:Class ;
	rdfs:subClassOf pdep:DepositedThing ;
	rdfs:subClassOf pdep:PaperExpression ;
	rdfs:label "Deposited paper"@en ;
	rdfs:comment "A paper which has been deposited in the Library of a House."@en ;
	rdfs:isDefinedBy <http://parliament.uk/ontologies/depositing/> .
	
pdep:TransportAndWorksActOrderApplication rdf:type owl:Class ;
	rdfs:subClassOf pdep:DepositedPaper ;
	rdfs:label "Transport and Works Act order application"@en ;
	rdfs:comment "An application for an order under the Transport and Works Act 1992. An order made under the Transport and Works Act 1992 is the usual way of authorising schemes for new railways or tramways in England and Wales. To apply for an order, an agent acting on behalf of an applicant must deposit an application into Parliament."@en ;
	rdfs:isDefinedBy <http://parliament.uk/ontologies/depositing/> .
	
pdep:Agent rdf:type owl:Class ;
	rdfs:label "Agent"@en ;
	rdfs:comment "An agent, being a body responsible for preparing and depositing a Transport and Works Act order application on behalf of an applicant."@en ;
	rdfs:isDefinedBy <http://parliament.uk/ontologies/depositing/> .
	
pdep:Applicant rdf:type owl:Class ;
	rdfs:label "Applicant"@en ;
	rdfs:comment "An applicant for a Transport and Works order, for example: Network Rail applying for an order to authorise the construction, maintenance and operation by Network Rail of works on the Transpennine Line between Stalybridge and Diggle (Saddleworth)."@en ;
	rdfs:isDefinedBy <http://parliament.uk/ontologies/depositing/> .
	
pdep:AvailabilityType rdf:type owl:Class ;
	rdfs:label "Availability type"@en ;
	rdfs:comment "The type of the availability of a deposited paper, being: available to the public, available to the public in a redacted form, or available only to Members."@en ;
	rdfs:isDefinedBy <http://parliament.uk/ontologies/depositing/> .
	
pdep:DepositedArtefact rdf:type owl:Class ;
	rdfs:subClassOf pdep:DepositedThing ;
	rdfs:label "Deposited artefact"@en ;
	rdfs:comment "An artefact which has been deposited in the Library of a House, for example: a breathalyser."@en ;
	rdfs:isDefinedBy <http://parliament.uk/ontologies/depositing/> .
	
pdep:PaperSeriesItem rdf:type owl:Class ;
	rdfs:label "Paper series item"@en ;
	rdfs:comment "A paper expression or artefact, as it exists as part of a paper series. A paper expression or artefact forming part of a series has an identifying number within that series."@en ;
	rdfs:isDefinedBy <http://parliament.uk/ontologies/depositing/> .
	
pdep:MadeStatutoryInstrumentWork rdf:type owl:Class ;
	rdfs:label "Made statutory instrument work"@en ;
	rdfs:comment "Made statutory instruments as signed into legislation. Made statutory instruments may result from a draft laid before Parliament or may be laid as made or may not be laid if the enabling legislation does not set out a duty to lay. Made statutory instruments laid before Parliament may be subject to a negative, affirmative or super affirmative procedure, or none. A made negative, having not been objected to within the scrutiny period, remains law. A made affirmative or made super affirmative, having been approved by Parliament within the approval period, remains law."@en ;
	rdfs:isDefinedBy <http://parliament.uk/ontologies/depositing/> .
	
pdep:Commitment rdf:type owl:Class ;
	rdfs:label "Commitment"@en ;
	rdfs:comment "A commitment to make a deposit in the Library of a House."@en ;
	rdfs:isDefinedBy <http://parliament.uk/ontologies/depositing/> .
	
pdep:CommittingThing rdf:type owl:Class ;
	rdfs:label "Committing thing"@en ;
	rdfs:comment "The means by which a commitment to deposit is made, for example: a contribution to a parliamentary debate, a letter to a Library or a written statement."@en ;
	rdfs:isDefinedBy <http://parliament.uk/ontologies/depositing/> .

pdep:Incumbency rdf:type owl:Class ;
	rdfs:label "Incumbency"@en ;
	rdfs:comment "The holding of a position by a person, including the time period for which this was the case. For example, Philip Hammond holding the position of Foreign Secretary between two dates."@en ;
	rdfs:isDefinedBy <http://parliament.uk/ontologies/depositing/> .

pdep:ParliamentaryPeriod rdf:type owl:Class ;
	rdfs:label "Parliamentary period"@en ;
	rdfs:comment "The time period of a single Parliament between the date of its first assembly after a general election and its dissolution. A Parliament period contains contiguous session and prorogation periods. During a parliament period Parliament is either in session or prorogued. The start date of a Parliament may be changed by subsequent proclamations. A Parliament ends at the next dissolution. While the Fixed-term Parliaments Act 2011 was in force, the date of dissolution was determined by that Act or was named in a proclamation following a vote in Parliament for an early general election. The next Parliament began on the date named in the proclamation issued following a dissolution. Before the Fixed-term Parliaments Act 2011 came into force and after that Act was repealed by the Dissolution and Calling of Parliament Act 2022, the date of dissolution is fixed by proclamation. The dissolution proclamation also names the date for Parliament to reassemble. Parliament periods are the same across both Houses. Parliaments are numbered ordinally from the first Parliament of the United Kingdom, sitting in 1801."@en ;
	rdfs:isDefinedBy <http://parliament.uk/ontologies/depositing/> .
	
pdep:CreditedContribution rdf:type owl:Class ;
	rdfs:label "Credited contribution"@en ;
	rdfs:comment "An oral contribution made by a known Member during a parliamentary proceeding."@en ;
	rdfs:isDefinedBy <http://parliament.uk/ontologies/depositing/> .



#######  Object properties ##### 
	
pdep:leadsTo rdf:type owl:ObjectProperty ;
	rdfs:label "Leads to"@en ;
	rdfs:comment "Relates a credited contribution in which the intention to make a commitment is recorded to the thing in which that commitment is made. Credited contributions may include the phrase, 'I will write'. A 'will write' is a contribution intended to lead to a letter of commitment to the Library, that letter being the committing thing. A letter of commitment may result from one credited contribution, or none."@en ;
	rdfs:domain pdep:CreditedContribution ;
	rdfs:range pdep:CommittingThing ;
	rdfs:isDefinedBy <http://parliament.uk/ontologies/depositing/> .
	
pdep:containsCommitment rdf:type owl:ObjectProperty ;
	rdfs:label "Contains commitment"@en ;
	rdfs:comment "Relates a committing thing to the commitment made. A committing thing contains one commitment. A commitment is contained by one committing thing."@en ;
	rdfs:domain pdep:CommittingThing ;
	rdfs:range pdep:Commitment ;
	rdfs:isDefinedBy <http://parliament.uk/ontologies/depositing/> .
	
pdep:madeBy rdf:type owl:ObjectProperty ;
	rdfs:label "Made by"@en ;
	rdfs:comment "Relates a commitment to the incumbency of a person in a position making that commitment. A commitment is made by one incumbency."@en ;
	rdfs:domain pdep:Commitment ;
	rdfs:range pdep:Incumbency ;
	rdfs:isDefinedBy <http://parliament.uk/ontologies/depositing/> .
	
pdep:madeDuring rdf:type owl:ObjectProperty ;
	rdfs:label "Made during"@en ;
	rdfs:comment "Relates a commitment to the parliamentary period during which the commitment is made. A commitment is made during one parliamentary period."@en ;
	rdfs:domain pdep:Commitment ;
	rdfs:range pdep:ParliamentaryPeriod ;
	rdfs:isDefinedBy <http://parliament.uk/ontologies/depositing/> .
	
pdep:resultsFromCommitment rdf:type owl:ObjectProperty ;
	rdfs:label "Results from commitment"@en ;
	rdfs:comment "Relates a deposit to the commitment to make that deposit. A commitment is made to provide one or more deposits. A deposit results from one commitment, or none. Where a deposit does not result from a commitment, it results from a duty set out in legislation."@en ;
	rdfs:domain pdep:Depositing ;
	rdfs:range pdep:Commitment ;
	rdfs:isDefinedBy <http://parliament.uk/ontologies/depositing/> .
	
pdep:resultsFromDutySetOutIn rdf:type owl:ObjectProperty ;
	rdfs:label "Results from duty set out in"@en ;
	rdfs:comment "Relates a deposit to the made statutory instrument setting out the duty under which that deposit is made. Transport and Works Act order applications are deposited under a duty set out in Rule 13 of The Transport and Works (Applications and Objections Procedure) (England and Wales) Rules 2006. Where a deposit does not result from a duty set out in legislation, it results from a commitment to make a deposit."@en ;
	rdfs:domain pdep:Depositing ;
	rdfs:range pdep:MadeStatutoryInstrumentWork ;
	rdfs:isDefinedBy <http://parliament.uk/ontologies/depositing/> .

pdep:resultsInDepositedArtefact rdf:type owl:ObjectProperty ;
	rdfs:label "Results in deposited artefact"@en ;
	rdfs:comment "Relates an act of depositing to the artefact or artefacts which have been deposited. A deposited artefact is the result of one deposit. An act of depositing results in one or more deposited artefacts, or none.  Where an act of depositing does not result in a deposited artefact, it results in a deposited paper or papers."@en ;
	rdfs:domain pdep:Depositing ;
	rdfs:range pdep:DepositedArtefact ;
	rdfs:isDefinedBy <http://parliament.uk/ontologies/depositing/> .

pdep:artefactAsSeriesItem rdf:type owl:ObjectProperty ;
	rdfs:label "Artefact as series item"@en ;
	rdfs:comment "Relates an artefact to the existence of that artefact in a paper series. A paper series item refers to one artefact. An artefact may exist as an item in one or more series, or none."@en ;
	rdfs:domain pdep:DepositedArtefact ;
	rdfs:range pdep:PaperSeriesItem ;
	rdfs:isDefinedBy <http://parliament.uk/ontologies/depositing/> .
	
pdep:resultsInDepositedPaper rdf:type owl:ObjectProperty ;
	rdfs:label "Results in deposited paper"@en ;
	rdfs:comment "Relates an act of depositing to the paper or papers which have been deposited. A deposited paper is the result of one deposit. An act of depositing results in one or more deposited papers, or none.  Where an act of depositing does not result in a deposited paper, it results in a deposited artefact or artefacts."@en ;
	rdfs:domain pdep:Depositing ;
	rdfs:range pdep:DepositedPaper ;
	rdfs:isDefinedBy <http://parliament.uk/ontologies/depositing/> .
	
pdep:hasAvailabilityType rdf:type owl:ObjectProperty ;
	rdfs:label "Has availability type"@en ;
	rdfs:comment "Relates a deposited paper to the availability type of that deposited paper. A deposited paper has one availability type."@en ;
	rdfs:domain pdep:DepositedPaper ;
	rdfs:range pdep:AvailabilityType ;
	rdfs:isDefinedBy <http://parliament.uk/ontologies/depositing/> .
	
pdep:hasAgent rdf:type owl:ObjectProperty ;
	rdfs:label "Has agent"@en ;
	rdfs:comment "Relates a Transport and Works Act order application to the agent responsible for preparing and depositing that application. A Transport and Works Act order application has one agent."@en ;
	rdfs:domain pdep:TransportAndWorkActOrderApplication ;
	rdfs:range pdep:Agent ;
	rdfs:isDefinedBy <http://parliament.uk/ontologies/depositing/> .
	
pdep:hasApplicant rdf:type owl:ObjectProperty ;
	rdfs:label "Has applicant"@en ;
	rdfs:comment "Relates a Transport and Works Act order application to the body applying for an order. A Transport and Works Act order application has one applicant."@en ;
	rdfs:domain pdep:TransportAndWorkActOrderApplication ;
	rdfs:range pdep:Applicant ;
	rdfs:isDefinedBy <http://parliament.uk/ontologies/depositing/> .

				

#######  Data properties #####

pdep:madeOn rdf:type owl:DatatypeProperty ;
	rdfs:label "Made on"@en ;
	rdfs:comment "Relates a commitment to the date on which that commitment was made."@en ;
	rdfs:domain pdep:Commitment ;
	rdfs:range xsd:date ;
	rdfs:isDefinedBy <http://parliament.uk/ontologies/depositing/> .
	
pdep:isStanding rdf:type owl:DatatypeProperty ;
	rdfs:label "Is standing"@en ;
	rdfs:comment "Used to record whether a commitment is a standing commitment. A standing commitment may lead to more than one deposit."@en ;
	rdfs:domain pdep:Commitment ;
	rdfs:range xsd:boolean ;
	rdfs:isDefinedBy <http://parliament.uk/ontologies/depositing/> .