@prefix pperson: <http://parliament.uk/ontologies/person/> . 
@prefix xsd: <http://www.w3.org/2001/XMLSchema#> . 
@prefix rdf: <http://www.w3.org/1999/02/22-rdf-syntax-ns#> .
@prefix dcterms: <http://purl.org/dc/terms/> .
@prefix owl:     <http://www.w3.org/2002/07/owl#> .
@prefix rdfs:    <http://www.w3.org/2000/01/rdf-schema#> .
@prefix foaf:	<http://xmlns.com/foaf/0.1/> .

<http://parliament.uk/ontologies/person/> 
    rdf:type owl:Ontology ;
    dcterms:title "Person ontology"@en ;
    dcterms:created "2025-07-04"^^xsd:date ;
	dcterms:rights "Open Parliament Licence v3.0"@en ;
    dcterms:description "A model describing a person."@en ;
	foaf:depiction <https://ukparliament.github.io/ontologies/paper-type/person.svg> ;
	foaf:maker
		[ foaf:name "Robert Brook"; foaf:homepage <https://robert-brook.com/> ],
		[ foaf:name "Ned Morrell" ],
		[ foaf:name "Michael Smethurst"; foaf:homepage <http://smethur.st/> ].
		
		
		
#######  Classes ##### 	

pperson:Person rdf:type owl:Class ;
	rdfs:label "Person"@en ;
	rdfs:comment "A person."@en ;
	rdfs:isDefinedBy <http://parliament.uk/ontologies/person/> .

				

#######  Data properties #####

pperson:givenName rdf:type owl:DatatypeProperty ;
	rdfs:label "Given name"@en ;
	rdfs:comment "Relates a person to their given name, for example: 'Alexander' in 'Alexander Boris de Pfeffel Johnson'."@en ;
	rdfs:domain pperson:Person ;
	rdfs:range rdf:langString ;
	rdfs:isDefinedBy <http://parliament.uk/ontologies/person/> .

pperson:familyName rdf:type owl:DatatypeProperty ;
	rdfs:label "Family name"@en ;
	rdfs:comment "Relates a person to their family name, for example: 'Johnson' in 'Alexander Boris de Pfeffel Johnson'."@en ;
	rdfs:domain pperson:Person ;
	rdfs:range rdf:langString ;
	rdfs:isDefinedBy <http://parliament.uk/ontologies/person/> .

pperson:knownBy rdf:type owl:DatatypeProperty ;
	rdfs:label "Known by"@en ;
	rdfs:comment "Relates a person to the name they are known by, for example: 'Boris' for 'Alexander Boris de Pfeffel Johnson'."@en ;
	rdfs:domain pperson:Person ;
	rdfs:range rdf:langString ;
	rdfs:isDefinedBy <http://parliament.uk/ontologies/person/> .

pperson:dateOfBirth rdf:type owl:DatatypeProperty ;
	rdfs:label "Date of birth"@en ;
	rdfs:comment "Relates a person to their date of birth."@en ;
	rdfs:domain pperson:Person ;
	rdfs:range xsd:date ;
	rdfs:isDefinedBy <http://parliament.uk/ontologies/person/> .

pperson:yearOfBirth rdf:type owl:DatatypeProperty ;
	rdfs:label "Year of birth"@en ;
	rdfs:comment "Relates a person to their year of birth. Used when an exact date of birth is not known."@en ;
	rdfs:domain pperson:Person ;
	rdfs:range xsd:integer ;
	rdfs:isDefinedBy <http://parliament.uk/ontologies/person/> .

pperson:monthOfBirth rdf:type owl:DatatypeProperty ;
	rdfs:label "Month of birth"@en ;
	rdfs:comment "Relates a person to their month of birth. Used when an exact date of birth is not known."@en ;
	rdfs:domain pperson:Person ;
	rdfs:range xsd:integer ;
	rdfs:isDefinedBy <http://parliament.uk/ontologies/person/> .

pperson:dayOfBirth rdf:type owl:DatatypeProperty ;
	rdfs:label "Day of birth"@en ;
	rdfs:comment "Relates a person to the day of their birth. Used when an exact date of birth is not known."@en ;
	rdfs:domain pperson:Person ;
	rdfs:range xsd:integer ;
	rdfs:isDefinedBy <http://parliament.uk/ontologies/person/> .
	
pperson:dateOfDeath rdf:type owl:DatatypeProperty ;
	rdfs:label "Date of death"@en ;
	rdfs:comment "Relates a person to their date of death."@en ;
	rdfs:domain pperson:Person ;
	rdfs:range xsd:date ;
	rdfs:isDefinedBy <http://parliament.uk/ontologies/person/> .

pperson:yearOfDeath rdf:type owl:DatatypeProperty ;
	rdfs:label "Year of death"@en ;
	rdfs:comment "Relates a person to their year of death. Used when an exact date of death is not known."@en ;
	rdfs:domain pperson:Person ;
	rdfs:range xsd:integer ;
	rdfs:isDefinedBy <http://parliament.uk/ontologies/person/> .

pperson:monthOfDeath rdf:type owl:DatatypeProperty ;
	rdfs:label "Month of death"@en ;
	rdfs:comment "Relates a person to their month of death. Used when an exact date of death is not known."@en ;
	rdfs:domain pperson:Person ;
	rdfs:range xsd:integer ;
	rdfs:isDefinedBy <http://parliament.uk/ontologies/person/> .

pperson:dayOfDeath rdf:type owl:DatatypeProperty ;
	rdfs:label "Day of death"@en ;
	rdfs:comment "Relates a person to the day of their death. Used when an exact date of death is not known."@en ;
	rdfs:domain pperson:Person ;
	rdfs:range xsd:integer ;
	rdfs:isDefinedBy <http://parliament.uk/ontologies/person/> .