@prefix pco: <https://parliament.uk/ontologies/concept/> . 
@prefix xsd: <http://www.w3.org/2001/XMLSchema#> . 
@prefix rdf: <http://www.w3.org/1999/02/22-rdf-syntax-ns#> .
@prefix dcterms: <http://purl.org/dc/terms/> .
@prefix owl:     <http://www.w3.org/2002/07/owl#> .
@prefix rdfs:    <http://www.w3.org/2000/01/rdf-schema#> .

<https://parliament.uk/ontologies/concept/> 
    rdf:type owl:Ontology ;
    dcterms:title "Concept ontology"@en ;
    dcterms:created "22/10/2016"^^xsd:date ;
	dcterms:rights "Open Parliament Licence v3.0"@en ;
    dcterms:description "Concept ontology for UK Parliament"@en .


#######  Classes ##### 	

pco:Concept rdf:type owl:Class ;
	rdfs:label "Concept"@en ;
	rdfs:comment "A concept. Similar to a SKOS concept / a library subject term."@en ;
	rdf:isDefinedBy <https://parliament.uk/ontologies/concept/> .

pco:ConceptScheme rdf:type owl:Class ;
	rdfs:label "ConceptScheme"@en ;
	rdfs:comment "A concept scheme. Provides an arbitrary way to group concepts e.g. Commons Library to Lords Library."@en ;
	rdf:isDefinedBy <https://parliament.uk/ontologies/concept/> .

pco:Thing rdf:type owl:Class ;
	rdfs:label "Thing"@en ;
	rdfs:comment "A thing. Anything at all."@en ;
	rdf:isDefinedBy <https://parliament.uk/ontologies/concept/> .
	
pco:AnnotatableThing rdf:type owl:Class ;
	rdfs:label "AnnotatableThing"@en ;
	rdfs:comment "A thing which can be annotated with a concept or free text tag. e.g. a debate or petition or answer."@en ;
	rdf:isDefinedBy <https://parliament.uk/ontologies/concept/> .
	
pco:Annotation rdf:type owl:Class ;
	rdfs:label "Annotation"@en ;
	rdfs:comment "A relationship between an annotatable thing and a concept or free-text tag. e.g. an act of subject indexing."@en ;
	rdf:isDefinedBy <https://parliament.uk/ontologies/concept/> .
	
pco:Agent rdf:type owl:Class ;
	rdfs:label "Agent"@en ;
	rdfs:comment "A person or group. In this context a librarian or machine subject indexing annotatable things."@en ;
	rdf:isDefinedBy <https://parliament.uk/ontologies/concept/> .


#######  data properties ##### 	

pco:alternativeLabel rdf:type owl:DatatypeProperty ;
	rdfs:label "alternativeLabel"@en ;
	rdfs:comment "An alternative label."@en ;
	rdfs:domain pco:Concept ;
	rdfs:range rdf:langString ;
	rdf:isDefinedBy <https://parliament.uk/ontologies/concept/> .

pco:historyNote rdf:type owl:DatatypeProperty ;
	rdfs:label "historyNote"@en ;
	rdfs:comment "A history note. Textual description of editorial changes to a concept over time."@en ;
	rdfs:domain pco:Concept ;
	rdfs:range rdf:langString ;
	rdf:isDefinedBy <https://parliament.uk/ontologies/concept/> .

pco:scopeNote rdf:type owl:DatatypeProperty ;
	rdfs:label "scopeNote"@en ;
	rdfs:comment "A scope note. Textual description of the intended usage of a concept."@en ;
	rdfs:domain pco:Concept ;
	rdfs:range rdf:langString ;
	rdf:isDefinedBy <https://parliament.uk/ontologies/concept/> .

pco:indexerNote rdf:type owl:DatatypeProperty ;
	rdfs:label "indexerNote"@en ;
	rdfs:comment "A note for indexers. Provides additional guidance on use of the concept."@en ;
	rdfs:domain pco:Concept ;
	rdfs:range rdf:langString ;
	rdf:isDefinedBy <https://parliament.uk/ontologies/concept/> .

pco:annotatedAt rdf:type owl:DatatypeProperty ;
	rdfs:label "annotatedAt"@en ;
	rdfs:comment "Date time an annotation was created."@en ;
	rdfs:domain pco:Annotation ;
	rdfs:range xsd:dateTime ;
	rdf:isDefinedBy <https://parliament.uk/ontologies/concept/> .

pco:uncontrolledTag rdf:type owl:DatatypeProperty ;
	rdfs:label "uncontrolledTag"@en ;
	rdfs:comment "To allow for annotations that reference free text tags rather than controlled concepts."@en ;
	rdfs:domain pco:Annotation ;
	rdfs:range rdf:langString ;
	rdf:isDefinedBy <https://parliament.uk/ontologies/concept/> .


#######  object properties ##### 	

pco:hasBroaderConcept rdf:type owl:ObjectProperty ;
	rdfs:label "hasBroaderConcept"@en ;
	rdfs:comment "Relates a concept to a broader concept."@en ;
	rdfs:domain pco:Concept ;
	rdfs:range pco:Concept ;
	rdf:isDefinedBy <https://parliament.uk/ontologies/concept/> .
	
pco:inConceptScheme rdf:type owl:ObjectProperty ;
	rdfs:label "inConceptScheme"@en ;
	rdfs:comment "Relates a concept to a concept scheme."@en ;
	rdfs:domain pco:Concept ;
	rdfs:range pco:ConceptScheme ;
	rdf:isDefinedBy <https://parliament.uk/ontologies/concept/> .
	
pco:hasFocus rdf:type owl:ObjectProperty ;
	rdfs:label "hasFocus"@en ;
	rdfs:comment "Relates a concept to a real world thing that is its focus e.g. The concept / library subject term Winston Churchill to the person Winston Churchill."@en ;
	rdfs:domain pco:Concept ;
	rdfs:range pco:Thing ;
	rdf:isDefinedBy <https://parliament.uk/ontologies/concept/> .	
	
pco:hasRelatedConcept rdf:type owl:ObjectProperty ;
	rdfs:label "hasRelatedConcept"@en ;
	rdfs:comment "Relates a concept to another concept."@en ;
	rdfs:domain pco:Concept ;
	rdfs:range pco:Concept ;
	rdf:isDefinedBy <https://parliament.uk/ontologies/concept/> .		
	
pco:hasAnnotation rdf:type owl:ObjectProperty ;
	rdfs:label "hasAnnotation"@en ;
	rdfs:comment "Relates an annotatable thing to an annotation."@en ;
	rdfs:domain pco:AnnotatableThing ;
	rdfs:range pco:Annotation ;
	rdf:isDefinedBy <https://parliament.uk/ontologies/concept/> .			
	
pco:hasConcept rdf:type owl:ObjectProperty ;
	rdfs:label "hasConcept"@en ;
	rdfs:comment "Relates an annotation to a concept."@en ;
	rdfs:domain pco:Annotation ;
	rdfs:range pco:Concept ;
	rdf:isDefinedBy <https://parliament.uk/ontologies/concept/> .				
	
pco:annotatedBy rdf:type owl:ObjectProperty ;
	rdfs:label "annotatedBy"@en ;
	rdfs:comment "Relates an annotation to a agent."@en ;
	rdfs:domain pco:Annotation ;
	rdfs:range pco:Agent ;
	rdf:isDefinedBy <https://parliament.uk/ontologies/concept/> .		