@prefix pev: <https://parliament.uk/ontologies/event/> . 
@prefix xsd: <http://www.w3.org/2001/XMLSchema#> . 
@prefix rdf: <http://www.w3.org/1999/02/22-rdf-syntax-ns#> .
@prefix dcterms: <http://purl.org/dc/terms/> .
@prefix owl:     <http://www.w3.org/2002/07/owl#> .
@prefix rdfs:    <http://www.w3.org/2000/01/rdf-schema#> .

<https://parliament.uk/ontologies/event/> 
    rdf:type owl:Ontology ;
    dcterms:title "Event ontology"@en ;
    dcterms:created "22/08/2017"^^xsd:date ;
	dcterms:rights "Open Parliament Licence v3.0"@en ;
    dcterms:description "Concept ontology for UK Parliament"@en .


#######  Classes ##### 	

pev:Event rdf:type owl:Class ;
	rdfs:label "Event"@en ;
	rdfs:comment "An event. A thing that happens over a time interval."@en ;
	rdf:isDefinedBy <https://parliament.uk/ontologies/event/> .
    
pev:CalendarEvent rdf:type owl:Class ;
    rdfs:subClassOf pev:Event ;
	rdfs:label "CalendarEvent"@en ;
	rdfs:comment "A planned or arranged event in a place."@en ;
	rdf:isDefinedBy <https://parliament.uk/ontologies/event/> .

pev:Attendance rdf:type owl:Class ;
    rdfs:label "Attendance"@en ;
    rdfs:comment "An attendance by a person at a calendar event. Sometimes attending in a certain capacity."@en ;
    rdf:isDefinedBy <https://parliament.uk/ontologies/event/> .

pev:Incumbency rdf:type owl:Class ;
    rdfs:label "Incumbency"@en ;
    rdfs:comment "A position held by a person for a period of time. e.g. Philip Hammond attending a meeting in his capacity of Foreign Secretary."@en ;
    rdf:isDefinedBy <https://parliament.uk/ontologies/event/> .
    
pev:Person rdf:type owl:Class ;
    rdfs:label "Person"@en ;
    rdfs:comment "A person."@en ;
    rdf:isDefinedBy <https://parliament.uk/ontologies/event/> .
    
pev:Place rdf:type owl:Class ;
    rdfs:label "Place"@en ;
    rdfs:comment "A geographic place."@en ;
    rdf:isDefinedBy <https://parliament.uk/ontologies/event/> . 
    
pev:BusinessItem rdf:type owl:Class ;
    rdfs:label "BusinessItem"@en ;
    rdfs:comment "An item of parliamentary business. e.g. an evidence session taking place in a meeting."@en ;
    rdf:isDefinedBy <https://parliament.uk/ontologies/event/> .

pev:BusinessItemType rdf:type owl:Class ;
    rdfs:label "BusinessItemType"@en ;
    rdfs:comment "Provides a means to associate a business item with a type of business item. e.g. a debate."@en ;
    rdf:isDefinedBy <https://parliament.uk/ontologies/event/> .

pev:Meeting rdf:type owl:Class ;
    rdfs:label "Meeting"@en ;
    rdfs:comment "A meeting. e.g. of a select committee."@en ;
    rdf:isDefinedBy <https://parliament.uk/ontologies/event/> .

pev:MeetingType rdf:type owl:Class ;
    rdfs:label "MeetingType"@en ;
    rdfs:comment "Provides a means to associate a meeting with a type of meeting. e.g. an informal briefing."@en ;
    rdf:isDefinedBy <https://parliament.uk/ontologies/event/> .
    
pev:Visit rdf:type owl:Class ;
    rdfs:label "Visit"@en ;
    rdfs:comment "A visit by a committee to a place outside the parliamentary estate. e.g. a visit to a factory or an overseas visit."@en ;
    rdf:isDefinedBy <https://parliament.uk/ontologies/event/> . 
    
pev:VisitType rdf:type owl:Class ;
    rdfs:label "VisitType"@en ;
    rdfs:comment "Provides a means to associate a visit with a type of visit. e.g. a visit for the purposes of an inquiry or seminar or conference."@en ;
    rdf:isDefinedBy <https://parliament.uk/ontologies/event/> .        
    
pev:EvidenceSession rdf:type owl:Class ;
    rdfs:subClassOf pev:BusinessItem ;
    rdfs:label "EvidenceSession"@en ;
    rdfs:comment "A type of business item where evidence is heard from witnesses."@en ;
    rdf:isDefinedBy <https://parliament.uk/ontologies/event/> .    

pev:OralEvidence rdf:type owl:Class ;
    rdfs:label "OralEvidence"@en ;
    rdfs:comment "A single piece of evidence provided by a witness at an evidence session."@en ;
    rdf:isDefinedBy <https://parliament.uk/ontologies/event/> . 

pev:Document rdf:type owl:Class ;
    rdfs:label "Document"@en ;
    rdfs:comment "A document."@en ;
    rdf:isDefinedBy <https://parliament.uk/ontologies/event/> . 

pev:Minutes rdf:type owl:Class ;
    rdfs:subClassOf pev:Document ;
    rdfs:label "Minutes"@en ;
    rdfs:comment "A type of document that captures what transpired during a meeting."@en ;
    rdf:isDefinedBy <https://parliament.uk/ontologies/event/> . 

pev:Itinerary rdf:type owl:Class ;
    rdfs:subClassOf pev:Document ;
    rdfs:label "Itinerary"@en ;
    rdfs:comment "A type of document setting out the schedule of a visit."@en ;
    rdf:isDefinedBy <https://parliament.uk/ontologies/event/> . 

pev:Transcript rdf:type owl:Class ;
    rdfs:subClassOf pev:Document ;
    rdfs:label "Transcript"@en ;
    rdfs:comment "A type of document that captures what was said during an evidence session."@en ;
    rdf:isDefinedBy <https://parliament.uk/ontologies/event/> . 

pev:Member rdf:type owl:Class ;
    rdfs:label "Member"@en ;
    rdfs:comment "A current or former Member of a House."@en ;
    rdf:isDefinedBy <https://parliament.uk/ontologies/event/> .        



#######  data properties ##### 	
    
pev:cancelledAt rdf:type owl:DatatypeProperty ;
    rdfs:label "cancelledAt"@en ;
    rdfs:comment "The time at which an event was cancelled."@en ;
    rdfs:domain pev:CalendarEvent ;
    rdfs:range xsd:dateTime ;
    rdf:isDefinedBy <https://parliament.uk/ontologies/event/> .  
    
pev:isPublic rdf:type owl:DatatypeProperty ;
    rdfs:label "isPublic"@en ;
    rdfs:comment "Whether members of the public are permitted to attend the event."@en ;
    rdfs:domain pev:CalendarEvent ;
    rdfs:range xsd:boolean ;
    rdf:isDefinedBy <https://parliament.uk/ontologies/event/> .    
    
pev:ordinality rdf:type owl:DatatypeProperty ;
    rdfs:label "ordinality"@en ;
    rdfs:comment "The position of a child event in its parent event."@en ;
    rdfs:domain pev:CalendarEvent ;
    rdfs:range xsd:integer ;
    rdf:isDefinedBy <https://parliament.uk/ontologies/event/> .    


#######  object properties ##### 	

pev:hasParentEvent rdf:type owl:ObjectProperty ;
	rdfs:label "hasParentEvent"@en ;
	rdfs:comment "Allows an event to be nested inside another event. e.g. a visit may contain a meeting which may contain an evidence session."@en ;
	rdfs:domain pev:Event ;
	rdfs:range pev:Event ;
	rdf:isDefinedBy <https://parliament.uk/ontologies/event/> .
	
pev:visitScheduling rdf:type owl:ObjectProperty ;
	rdfs:label "visitScheduling"@en ;
	rdfs:comment "Relates a visit to a calendar event. This allows an event to be created and annotated in advance of being scheduled."@en ;
	rdfs:domain pev:Visit ;
	rdfs:range pev:CalendarEvent ;
	rdf:isDefinedBy <https://parliament.uk/ontologies/event/> .
	
pev:meetingScheduling rdf:type owl:ObjectProperty ;
	rdfs:label "meetingScheduling"@en ;
	rdfs:comment "Relates a meeting to a calendar event. This allows a meeting to be created and annotated in advance of being scheduled."@en ;
	rdfs:domain pev:Meeting ;
	rdfs:range pev:CalendarEvent ;
	rdf:isDefinedBy <https://parliament.uk/ontologies/event/> .

pev:businessItemScheduling rdf:type owl:ObjectProperty ;
	rdfs:label "businessItemScheduling"@en ;
	rdfs:comment "Relates a business item to a calendar event. This allows a business item to be created and annotated in advance of being scheduled."@en ;
	rdfs:domain pev:BusinessItem ;
	rdfs:range pev:CalendarEvent ;
	rdf:isDefinedBy <https://parliament.uk/ontologies/event/> .
    
pev:chairedBy rdf:type owl:ObjectProperty ;
    rdfs:label "chairedBy"@en ;
    rdfs:comment "Relates a calendar event to the Member of Parliament chairing it."@en ;
    rdfs:domain pev:CalendarEvent ;
    rdfs:range pev:Member ;
    rdf:isDefinedBy <https://parliament.uk/ontologies/event/> .  
    
pev:hasBusinessItemType rdf:type owl:ObjectProperty ;
    rdfs:label "hasBusinessItemType"@en ;
    rdfs:comment "Relates a business item to the type of business item it is."@en ;
    rdfs:domain pev:BusinessItem ;
    rdfs:range pev:BusinessItemType ;
    rdf:isDefinedBy <https://parliament.uk/ontologies/event/> . 
    
pev:offersEvidence rdf:type owl:ObjectProperty ;
    rdfs:label "offersEvidence"@en ;
    rdfs:comment "Relates a piece of oral evidence (a single witness) to the evidence session in which it was given."@en ;
    rdfs:domain pev:OralEvidence ;
    rdfs:range pev:EvidenceSession ;
    rdf:isDefinedBy <https://parliament.uk/ontologies/event/> . 
        
pev:hasTranscript rdf:type owl:ObjectProperty ;
    rdfs:label "hasTranscript"@en ;
    rdfs:comment "Relates an evidence session to the transcript that captures what was said during that session."@en ;
    rdfs:domain pev:EvidenceSession ;
    rdfs:range pev:Transcript ;
    rdf:isDefinedBy <https://parliament.uk/ontologies/event/> . 
    
pev:hasMinutes rdf:type owl:ObjectProperty ;
    rdfs:label "hasMinutes"@en ;
    rdfs:comment "Relates a meeting to the minutes of that meeting."@en ;
    rdfs:domain pev:Meeting ;
    rdfs:range pev:Minutes ;
    rdf:isDefinedBy <https://parliament.uk/ontologies/event/> .
    
pev:hasMeetingType rdf:type owl:ObjectProperty ;
    rdfs:label "hasMeetingType"@en ;
    rdfs:comment "Relates a meeting to the type of meeting it is."@en ;
    rdfs:domain pev:Meeting ;
    rdfs:range pev:MeetingType ;
    rdf:isDefinedBy <https://parliament.uk/ontologies/event/> .
    
pev:hasVisitType rdf:type owl:ObjectProperty ;
    rdfs:label "hasVisitType"@en ;
    rdfs:comment "Relates a visit to the type of visit it is."@en ;
    rdfs:domain pev:Visit ;
    rdfs:range pev:VisitType ;
    rdf:isDefinedBy <https://parliament.uk/ontologies/event/> . 
    
pev:hasItinerary rdf:type owl:ObjectProperty ;
    rdfs:label "hasItinerary"@en ;
    rdfs:comment "Relates a visit to the itinerary of that visit."@en ;
    rdfs:domain pev:Visit ;
    rdfs:range pev:Itinerary ;
    rdf:isDefinedBy <https://parliament.uk/ontologies/event/> . 
    
pev:takesPlaceIn rdf:type owl:ObjectProperty ;
    rdfs:label "takesPlaceIn"@en ;
    rdfs:comment "Relates a calendar event to the place the event happens in."@en ;
    rdfs:domain pev:CalendarEvent ;
    rdfs:range pev:Place ;
    rdf:isDefinedBy <https://parliament.uk/ontologies/event/> . 
    
pev:hasAttendee rdf:type owl:ObjectProperty ;
    rdfs:label "hasAttendee"@en ;
    rdfs:comment "Relates a calendar event to an attendance."@en ;
    rdfs:domain pev:CalendarEvent ;
    rdfs:range pev:Attendance ;
    rdf:isDefinedBy <https://parliament.uk/ontologies/event/> . 
    
pev:attendanceInCapacity rdf:type owl:ObjectProperty ;
    rdfs:label "attendanceInCapacity"@en ;
    rdfs:comment "Relates an attendance to the capacity in which a person attends is attending."@en ;
    rdfs:domain pev:Attendance ;
    rdfs:range pev:Incumbency ;
    rdf:isDefinedBy <https://parliament.uk/ontologies/event/> . 
    
pev:attendedBy rdf:type owl:ObjectProperty ;
    rdfs:label "attendedBy"@en ;
    rdfs:comment "Relates an attendance to the person attending."@en ;
    rdfs:domain pev:Attendance ;
    rdfs:range pev:Person ;
    rdf:isDefinedBy <https://parliament.uk/ontologies/event/> .                                                
	
		