@prefix parea: <http://parliament.uk/ontologies/geographic-area/> . 
@prefix xsd: <http://www.w3.org/2001/XMLSchema#> . 
@prefix rdf: <http://www.w3.org/1999/02/22-rdf-syntax-ns#> .
@prefix dcterms: <http://purl.org/dc/terms/> .
@prefix owl:     <http://www.w3.org/2002/07/owl#> .
@prefix rdfs:    <http://www.w3.org/2000/01/rdf-schema#> .
@prefix foaf:	<http://xmlns.com/foaf/0.1/> .

<http://parliament.uk/ontologies/geographic-area/> 
    rdf:type owl:Ontology ;
    dcterms:title "Geographic area ontology"@en ;
    dcterms:created "2021-09-28"^^xsd:date ;
	dcterms:rights "Open Parliament Licence v3.0"@en ;
    dcterms:description "A model describing geographic areas in the UK - being constituency areas, local authority areas, countries, and statistical regions within England - and the containment relationships between such areas."@en ;
	foaf:depiction <https://ukparliament.github.io/ontologies/geographic-area/geographic-area-period.svg> ;
	foaf:maker
		[ foaf:name "Carl Baker" ],
		[ foaf:name "Robert Brook"; foaf:homepage <https://robert-brook.com/> ],
		[ foaf:name "Neil Johnston" ],
		[ foaf:name "Ned Morrell" ],
		[ foaf:name "Mark Sandford" ],
		[ foaf:name "Michael Smethurst"; foaf:homepage <http://smethur.st/> ],
		[ foaf:name "Anya Somerville" ] .


#######  Classes #####

parea:GeographicArea rdf:type owl:Class ;
	rdfs:label "Geographic area"@en ;
	rdfs:comment "A named area of geography."@en ;
	rdfs:isDefinedBy <http://parliament.uk/ontologies/geographic-area/> .
	
parea:GeographicAreaDefinedByStatute rdf:type owl:Class ;
	rdfs:subClassOf parea:GeographicArea ;
	rdfs:label "Geographic area defined by statute"@en ;
	rdfs:comment "A geographic area defined by an Act of Parliament or a made statutory instrument."@en ;
	rdfs:isDefinedBy <http://parliament.uk/ontologies/geographic-area/> .
	
parea:ConstituencyArea rdf:type owl:Class ;
	rdfs:subClassOf parea:GeographicAreaDefinedByStatute ;
	rdfs:label "Constituency area"@en ;
	rdfs:comment "An area within which members of a constituency group are registered to vote. Constituency areas bounding constituency groups represented in the House of Commons are proposed in a boundary review by the Boundary Commissions and established by statute."@en ;
	rdfs:isDefinedBy <http://parliament.uk/ontologies/geographic-area/> .
	
parea:UpperTierLocalAuthorityArea rdf:type owl:Class ;
	rdfs:subClassOf parea:GeographicAreaDefinedByStatute ;
	rdfs:label "Upper tier local authority area"@en ;
	rdfs:comment "The geographic area in which an upper tier local authority may exercise its powers."@en ;
	rdfs:isDefinedBy <http://parliament.uk/ontologies/geographic-area/> .

parea:LowerTierLocalAuthorityArea rdf:type owl:Class ;
	rdfs:subClassOf parea:GeographicAreaDefinedByStatute ;
	rdfs:label "Lower tier local authority area"@en ;
	rdfs:comment "The geographic area in which a lower tier local authority may exercise its powers."@en ;
	rdfs:isDefinedBy <http://parliament.uk/ontologies/geographic-area/> .

parea:CombinedAuthorityArea rdf:type owl:Class ;
	rdfs:subClassOf parea:GeographicAreaDefinedByStatute ;
	rdfs:label "Combined authority area"@en ;
	rdfs:comment "The geographic area in which a combined authority or combined county authority may exercise its powers. A combined authority may be created in England under powers set out in the Local Democracy, Economic Development and Construction Act 2009. A combined county authority may be created in England under powers set out in the Levelling-up and Regeneration Act 2023."@en ;
	rdfs:isDefinedBy <http://parliament.uk/ontologies/geographic-area/> .
	
parea:EnglishRegion rdf:type owl:Class ;
	rdfs:subClassOf parea:GeographicArea ;
	rdfs:label "English region"@en ;
	rdfs:comment "A statistical region in England, formerly known as a government office region, being an International Territorial Level (ITL) 1 unit, formerly known as a NUTS 1 unit."@en ;
	rdfs:isDefinedBy <http://parliament.uk/ontologies/geographic-area/> .
	
parea:Country rdf:type owl:Class ;
	rdfs:subClassOf parea:GeographicArea ;
	rdfs:label "Country"@en ;
	rdfs:comment "A country in the United Kingdom."@en ;
	rdfs:isDefinedBy <http://parliament.uk/ontologies/geographic-area/> .
	
parea:BoundarySet rdf:type owl:Class ;
	rdfs:label "Boundary set"@en ;
	rdfs:comment "A boundary set defining UK Parliament constituency areas, as proposed in a boundary review by the Boundary Commissions and established by statute."@en ;
	rdfs:isDefinedBy <http://parliament.uk/ontologies/geographic-area/> .

parea:StatutoryThing rdf:type owl:Class ;
	rdfs:label "Statutory thing"@en ;
	rdfs:comment "A statutory thing, for example: an Act of Parliament or a made statutory instrument."@en ;
	rdfs:isDefinedBy <http://parliament.uk/ontologies/geographic-area/> .
	
parea:ConstituencyAreaType rdf:type owl:Class ;
	rdfs:label "Constituency area type"@en ;
	rdfs:comment "The type of a constituency area, being either county, borough or burgh."@en ;
	rdfs:isDefinedBy <http://parliament.uk/ontologies/geographic-area/> .
	
	
	
#######  Object properties ##### 

parea:whollyContainedBy rdf:type owl:ObjectProperty ;
	rdfs:label "Wholly contained by"@en ;
	rdfs:comment "Relates a geographic area to the geographic area it is wholly contained by. A constituency area may be wholly contained by a lower tier local authority area, by an upper tier local authority area, or by neither. A constituency area in England is wholly contained by an English region. A constituency area is wholly contained by a country. A lower tier local authority area may be wholly contained by a constituency area. A lower tier local authority area is wholly contained by an upper tier local authority area, except where the lower tier local authority area is also the upper tier local authority area. An upper tier local authority area may be wholly contained by a constituency area. As at November 2024, an upper tier local authority area is wholly contained by a combined authority area, where a combined authority area exists. An upper tier local authority area in England is wholly contained by an English region. An upper tier local authority area is wholly contained by a country. A combined authority area may be wholly contained by an English region. A combined authority area is wholly contained by the country of England. An English region is wholly contained by the country of England."@en ;
	rdfs:domain parea:GeographicArea ;
	rdfs:range parea:GeographicArea ;
	rdfs:isDefinedBy <http://parliament.uk/ontologies/geographic-area/> .

parea:partlyContainedBy rdf:type owl:ObjectProperty ;
	rdfs:label "Partly contained by"@en ;
	rdfs:comment "Relates a geographic area to a geographic area it is partly contained by. A constituency area may be partly contained by a lower tier local authority area, by an upper tier local authority area, or by neither. A lower tier local authority area or an upper tier local authority area may be partly contained by a constituency area. The Local Democracy, Economic Development and Construction Act 2009 does not preclude an upper tier local authority area being partly contained by a combined authority area. As at November 2024, no upper tier local authority area is partly contained by a combined authority area."@en ;
	rdfs:domain parea:GeographicArea ;
	rdfs:range parea:GeographicArea ;
	rdfs:isDefinedBy <http://parliament.uk/ontologies/geographic-area/> .

parea:definedWithin rdf:type owl:ObjectProperty ;
	rdfs:label "Defined within"@en ;
	rdfs:comment "Relates a constituency area to the boundary set which defines that area. A constituency area is defined by one boundary set. A boundary set defines one or more constituency areas."@en ;
	rdfs:domain parea:ConstituencyArea ;
	rdfs:range parea:BoundarySet ;
	rdfs:isDefinedBy <http://parliament.uk/ontologies/geographic-area/> .

parea:definedBy rdf:type owl:ObjectProperty ;
	rdfs:label "Defined by"@en ;
	rdfs:comment "Relates a geographic area defined by statute to the statutory thing it was defined by. A geographic area defined by statute is defined by one statutory thing. A statutory thing may define one or more geographic areas, or none."@en ;
	rdfs:domain parea:GeographicAreaDefinedByStatute ;
	rdfs:range parea:StatutoryThing ;
	rdfs:isDefinedBy <http://parliament.uk/ontologies/geographic-area/> .
	
parea:boundarySetEstablishedBy rdf:type owl:ObjectProperty ;
	rdfs:label "Boundary set established by"@en ;
	rdfs:comment "Relates a boundary set to the statutory thing, or things, which established that boundary set. A boundary set may be established by one or more statutory things, for example: the 2010 boundary set in Wales being established by a single Order in Council and the 1955 boundary set in Wales being established by three Orders in Council. A statutory thing may establish one or more boundary sets, or none, for example: the Parliamentary Constituencies and Assembly Electoral Regions (Wales) Order 2006 establishing the 2010 boundary set in Wales and the Parliamentary Constituencies Order 2023 establishing boundary sets in England, Wales, Northern Ireland and Scotland."@en ;
	rdfs:domain parea:BoundarySet ;
	rdfs:range parea:StatutoryThing ;
	rdfs:isDefinedBy <http://parliament.uk/ontologies/geographic-area/> .

parea:isAlsoUpperTierLocalAuthorityArea rdf:type owl:ObjectProperty ;
	rdfs:label "Is also upper tier local authority area"@en ;
	rdfs:comment "Relates a lower tier local authority area to an upper tier local authority area where the lower tier local authority area is also the upper tier local authority area."@en ;
	rdfs:domain parea:LowerTierLocalAuthorityArea ;
	rdfs:range parea:UpperTierLocalAuthorityArea ;
	rdfs:isDefinedBy <http://parliament.uk/ontologies/geographic-area/> .
	
parea:appliesTo rdf:type owl:ObjectProperty ;
	rdfs:label "Applies to"@en ;
	rdfs:comment "Relates a boundary set to the country to which that boundary set applies. A boundary set applies to one country. A country may have one or more boundary sets over time. A country has one boundary set at any one time."@en ;
	rdfs:domain parea:BoundarySet ;
	rdfs:range parea:Country ;
	rdfs:isDefinedBy <http://parliament.uk/ontologies/geographic-area/> .
	
parea:hasConstituencyAreaType rdf:type owl:ObjectProperty ;
	rdfs:label "Has constituency area type"@en ;
	rdfs:comment "Relates a constituency area to the type of that constituency area. A constituency area has one type."@en ;
	rdfs:domain parea:ConstituencyArea ;
	rdfs:range parea:ConstituencyAreaType ;
	rdfs:isDefinedBy <http://parliament.uk/ontologies/geographic-area/> .
	
	
	
#######  Data properties ##### 

parea:geometry rdf:type owl:DatatypeProperty ;
	rdfs:label "Geometry"@en ;
	rdfs:comment "Relates a geographic area to the geometry describing the boundaries of that area."@en ;
	rdfs:domain parea:GeographicArea ;
	rdfs:range rdfs:Literal ;
	rdfs:isDefinedBy <http://parliament.uk/ontologies/geographic-area/> .