@prefix ppb: <https://parliament.uk/ontologies/political-bloc/> . 
@prefix xsd: <http://www.w3.org/2001/XMLSchema#> . 
@prefix rdf: <http://www.w3.org/1999/02/22-rdf-syntax-ns#> .
@prefix dcterms: <http://purl.org/dc/terms/> .
@prefix owl:     <http://www.w3.org/2002/07/owl#> .
@prefix rdfs:    <http://www.w3.org/2000/01/rdf-schema#> .

<https://parliament.uk/ontologies/political-bloc/> 
    rdf:type owl:Ontology ;
    dcterms:title "Political bloc ontology"@en ;
    dcterms:created "14/06/2017"^^xsd:date ;
	dcterms:rights "Open Parliament Licence v3.0"@en ;
    dcterms:description "Political bloc ontology for UK Parliament. Extends and specialises the agency model to describe memberships and whippings to politic parties and affiliations to politic blocs."@en .


#######  Classes ##### 	

ppb:Pact rdf:type owl:Class ;
	rdfs:label "Pact"@en ;
	rdfs:comment "A formal agreement between two or more political parties."@en ;
	rdf:isDefinedBy <https://parliament.uk/ontologies/political-bloc/> .
	
ppb:Sistership rdf:type owl:Class ;
	rdfs:label "Sistership"@en ;
	rdfs:comment "A relationship between parties with ideologically similar positions who have agreed to co-operate."@en ;
	rdf:isDefinedBy <https://parliament.uk/ontologies/political-bloc/> .
	
ppb:Party rdf:type owl:Class ;
	rdfs:subClassOf ppb:PoliticalBloc ;
	rdfs:label "Party"@en ;
	rdfs:comment "An organised political group."@en ;
	rdf:isDefinedBy <https://parliament.uk/ontologies/political-bloc/> .
	
ppb:PoliticalBloc rdf:type owl:Class ;
	rdfs:label "PoliticalBloc"@en ;
	rdfs:comment "A group of members. This might be a political party such as Labour or Conservative. Or might be a different type of grouping such as Bishops or Crossbenchers in the House of Lords."@en ;
	rdf:isDefinedBy <https://parliament.uk/ontologies/political-bloc/> .
	
ppb:Affiliation rdf:type owl:Class ;
	rdfs:label "Affiliation"@en ;
	rdfs:comment "A person or group's affiliation to a political bloc between between two dates. Could be used to describe affiliations to non-political party blocs. e.g. Crossbenchers and bishops in the House of Lords. Could also be used to describe members having an affiliation to the Co-operative Party whilst being whipped to Labour."@en ;
	rdf:isDefinedBy <https://parliament.uk/ontologies/political-bloc/> .
	
ppb:Whipping rdf:type owl:Class ;
	rdfs:subClassOf ppb:Affiliation ;
	rdfs:label "Whipping"@en ;
	rdfs:comment "A member of a legislature being whipped to a political party between two dates. A member accepting a whip agrees to vote mainly in line with the party they're whipped to. The whip may be withdrawn by the party or rejected by the member."@en ;
	rdf:isDefinedBy <https://parliament.uk/ontologies/political-bloc/> .
	
ppb:Member rdf:type owl:Class ;
	rdfs:subClassOf ppb:Person ;
	rdfs:label "Member"@en ;
	rdfs:comment "A current or former member of a house."@en ;
	rdf:isDefinedBy <https://parliament.uk/ontologies/political-bloc/> .
	

	
##### Object properties ####


ppb:hasPact rdf:type owl:ObjectProperty ;
	rdfs:label "hasPact"@en ;
	rdfs:comment "Relates a party to the pact it's part of."@en ;
	rdfs:domain ppb:Party ;
	rdfs:range ppb:Pact ;
	rdf:isDefinedBy <https://parliament.uk/ontologies/political-bloc/> .
	
ppb:hasSistership rdf:type owl:ObjectProperty ;
	rdfs:label "hasSistership"@en ;
	rdfs:comment "Relates a party to a sistership it's part of."@en ;
	rdfs:domain ppb:Party ;
	rdfs:range ppb:Sistership ;
	rdf:isDefinedBy <https://parliament.uk/ontologies/political-bloc/> .
	
ppb:affiliatedToPoliticalBloc rdf:type owl:ObjectProperty ;
	rdfs:label "affiliatedToPoliticalBloc"@en ;
	rdfs:comment "Relates an affiliation to a political bloc. e.g. covers the affiliation of a crossbencher to the crossbench bloc in the House of Lords. "@en ;
	rdfs:domain ppb:Affiliation ;
	rdfs:range ppb:PoliticalBloc ;
	rdf:isDefinedBy <https://parliament.uk/ontologies/political-bloc/> .
	
ppb:whippingTo rdf:type owl:ObjectProperty ;
	rdfs:label "whippingTo"@en ;
	rdfs:comment "Relates a whipping to a political party."@en ;
	rdfs:domain ppb:Whipping ;
	rdfs:range ppb:Party ;
	rdf:isDefinedBy <https://parliament.uk/ontologies/political-bloc/> .
	
ppb:hasWhipping rdf:type owl:ObjectProperty ;
	rdfs:label "hasWhipping"@en ;
	rdfs:comment "Relates a member to a whipping."@en ;
	rdfs:domain ppb:Member ;
	rdfs:range ppb:Whipping ;
	rdf:isDefinedBy <https://parliament.uk/ontologies/political-bloc/> .
				
	
##### Data properties ####	
			

						