@prefix ppaper: <http://parliament.uk/ontologies/parliamentary-paper/> . 
@prefix xsd: <http://www.w3.org/2001/XMLSchema#> . 
@prefix rdf: <http://www.w3.org/1999/02/22-rdf-syntax-ns#> .
@prefix dcterms: <http://purl.org/dc/terms/> .
@prefix owl:     <http://www.w3.org/2002/07/owl#> .
@prefix rdfs:    <http://www.w3.org/2000/01/rdf-schema#> .
@prefix foaf:	<http://xmlns.com/foaf/0.1/> .

<http://parliament.uk/ontologies/parliamentary-paper/> 
    rdf:type owl:Ontology ;
    dcterms:title "Parliamentary paper ontology"@en ;
    dcterms:created "2022-07-11"^^xsd:date ;
	dcterms:rights "Open Parliament Licence v3.0"@en ;
    dcterms:description "A model describing parliamentary papers, their types and their presence in bundles and in series."@en ;
	foaf:depiction <https://ukparliament.github.io/ontologies/parliamentary-paper/parliamentary-paper.svg> ;
	foaf:maker
		[ foaf:name "Jayne Bosworth" ],
		[ foaf:name "Robert Brook"; foaf:homepage <https://robert-brook.com/> ],
		[ foaf:name "Corie Chambers" ],
		[ foaf:name "Helen Creeke" ],
		[ foaf:name "Kath Kavanagh" ],
		[ foaf:name "Ned Morrell" ],
		[ foaf:name "Robi Quigley" ],
		[ foaf:name "Michael Smethurst"; foaf:homepage <http://smethur.st/> ],
		[ foaf:name "Anya Somerville" ].
		
		
		
#######  Classes ##### 	

ppaper:ParliamentaryPaperWork rdf:type owl:Class ;
	rdfs:label "Parliamentary paper work"@en ;
	rdfs:comment "A parliamentary paper as a single intellectual work, as defined in the Functional Requirements for Bibliographic Records specification."@en ;
	rdfs:isDefinedBy <http://parliament.uk/ontologies/parliamentary-paper/> .
	
ppaper:ParliamentaryPaperExpression rdf:type owl:Class ;
	rdfs:label "Parliamentary paper expression"@en ;
	rdfs:comment "A parliamentary paper made available to a House, being an expression of parliamentary paper work."@en ;
	rdfs:isDefinedBy <http://parliament.uk/ontologies/parliamentary-paper/> .
	
ppaper:PaperBundle rdf:type owl:Class ;
	rdfs:label "Paper bundle"@en ;
	rdfs:comment "A group of related parliamentary papers, called a bundle, for example: a bundle containing a statutory instrument paper and a related explanatory memorandum."@en ;
	rdfs:isDefinedBy <http://parliament.uk/ontologies/parliamentary-paper/> .
	
ppaper:PaperType rdf:type owl:Class ;
	rdfs:label "Paper type"@en ;
	rdfs:comment "The type of a paper, for example: bill, statutory instrument, petition or statement of annual accounts."@en ;
	rdfs:isDefinedBy <http://parliament.uk/ontologies/parliamentary-paper/> .
	
ppaper:PaperSeriesItem rdf:type owl:Class ;
	rdfs:label "Paper series item"@en ;
	rdfs:comment "A parliamentary paper, as it exists as part of a paper series. A parliamentary paper forming part of a series has a number within that series."@en ;
	rdfs:isDefinedBy <http://parliament.uk/ontologies/parliamentary-paper/> .
	
ppaper:PaperSeries rdf:type owl:Class ;
	rdfs:label "Paper series"@en ;
	rdfs:comment "A series of parliamentary papers, for example: the Treaty Series."@en ;
	rdfs:isDefinedBy <http://parliament.uk/ontologies/parliamentary-paper/> .
	
ppaper:Session rdf:type owl:Class ;
	rdfs:label "Session"@en ;
	rdfs:comment "A period during which Parliament is able to conduct business on days of its choosing. A session is within a Parliament period. The first session of a Parliament begins on the same day as the Parliament period and ends on a day named in a subsequent prorogation proclamation. Subsequent sessions within the Parliament period begin and end on dates named in subsequent prorogation proclamations. The final session of a Parliament ends either with prorogation followed by dissolution or with dissolution. Session periods are the same for both Houses."@en ;
	rdfs:isDefinedBy <http://parliament.uk/ontologies/parliamentary-paper/> .
	
				

#######  Object properties ##### 
	
ppaper:expressionOf rdf:type owl:ObjectProperty ;
	rdfs:label "Expression of"@en ;
	rdfs:comment "Relates a parliamentary paper expression to the work that paper is an expression of. A parliamentary paper expression is an expression of one parliamentary paper work. A parliamentary paper work is expressed as one or more parliamentary papers."@en ;
	rdfs:domain ppaper:ParliamentaryPaperExpression ;
	rdfs:range ppaper:ParliamentaryPaperWork ;
	rdfs:isDefinedBy <http://parliament.uk/ontologies/parliamentary-paper/> .
	
ppaper:formsPartOf rdf:type owl:ObjectProperty ;
	rdfs:label "Forms part of"@en ;
	rdfs:comment "Relates a parliamentary paper expression to the paper bundle it forms part of. A parliamentary paper expression may belong to one or more paper bundles, or none. For example: a single explanatory memorandum may form part of more than one bundle."@en ;
	rdfs:domain ppaper:ParliamentaryPaperExpression ;
	rdfs:range ppaper:PaperBundle ;
	rdfs:isDefinedBy <http://parliament.uk/ontologies/parliamentary-paper/> .

ppaper:hasType rdf:type owl:ObjectProperty ;
	rdfs:label "Has type"@en ;
	rdfs:comment "Relates a parliamentary paper expression to the type of that paper. A parliamentary paper expression may have one or more types, or none."@en ;
	rdfs:domain ppaper:ParliamentaryPaperExpression ;
	rdfs:range ppaper:PaperType ;
	rdfs:isDefinedBy <http://parliament.uk/ontologies/parliamentary-paper/> .

ppaper:paperTypeParent rdf:type owl:ObjectProperty ;
	rdfs:label "Paper type parent"@en ;
	rdfs:comment "Relates one paper type to another in a parent-child relationship. A paper type may have one or more parent paper types, or none. A paper type may have one or more child paper types, or none."@en ;
	rdfs:domain ppaper:PaperType ;
	rdfs:range ppaper:PaperType ;
	rdfs:isDefinedBy <http://parliament.uk/ontologies/parliamentary-paper/> .

ppaper:asSeriesitem rdf:type owl:ObjectProperty ;
	rdfs:label "As series item"@en ;
	rdfs:comment "Relates a parliamentary paper expression to the existence of that paper in a series. A paper series item refers to one parliamentary paper expression. A parliamentary paper expression may exist as an item in one or more series, or none."@en ;
	rdfs:domain ppaper:ParliamentaryPaperExpression ;
	rdfs:range ppaper:PaperSeriesItem ;
	rdfs:isDefinedBy <http://parliament.uk/ontologies/parliamentary-paper/> .

ppaper:inSeries rdf:type owl:ObjectProperty ;
	rdfs:label "In series"@en ;
	rdfs:comment "Relates the existence of a parliamentary paper as an item in a series to the series that the item forms part of. A paper series item forms part of one paper series."@en ;
	rdfs:domain ppaper:PaperSeriesItem ;
	rdfs:range ppaper:PaperSeries ;
	rdfs:isDefinedBy <http://parliament.uk/ontologies/parliamentary-paper/> .

ppaper:paperSeriesParent rdf:type owl:ObjectProperty ;
	rdfs:label "Paper series parent"@en ;
	rdfs:comment "Relates a paper series to its parent paper series. A paper series may have one parent paper series, or none. A paper series may have one or more child paper series, or none, for example: the Treaty Series of in force treaties is a child series of the Command Papers series."@en ;
	rdfs:domain ppaper:PaperSeries ;
	rdfs:range ppaper:PaperSeries ;
	rdfs:isDefinedBy <http://parliament.uk/ontologies/parliamentary-paper/> .

ppaper:paperSeriesFollows rdf:type owl:ObjectProperty ;
	rdfs:label "Paper series follows"@en ;
	rdfs:comment "Relates a paper series to its preceding series. A paper series may follow one series, or none. A paper series may be followed by one series, or none, for example: the series of statutory instruments made in 2022 follows the series of statutory instruments made in 2021."@en ;
	rdfs:domain ppaper:PaperSeries ;
	rdfs:range ppaper:PaperSeries ;
	rdfs:isDefinedBy <http://parliament.uk/ontologies/parliamentary-paper/> .

ppaper:belongsTo rdf:type owl:ObjectProperty ;
	rdfs:label "Belongs to"@en ;
	rdfs:comment "Relates a paper series to the session that series belongs to. A paper series may belong to one session, or none, for example: the series of House of Commons papers belonging to the session in which papers in that series are made available."@en ;
	rdfs:domain ppaper:PaperSeries ;
	rdfs:range ppaper:Session ;
	rdfs:isDefinedBy <http://parliament.uk/ontologies/parliamentary-paper/> .

	
	
#######  Data properties ##### 

ppaper:prefix rdf:type owl:DatatypeProperty ;
	rdfs:label "Prefix"@en ;
	rdfs:comment "Relates a paper series to the prefix which is combined with a paper series item identifier to form the 'number' of a parliamentary paper as an item in that series."@en ;
	rdfs:domain ppaper:PaperSeries ;
	rdfs:range rdfs:Literal ;
	rdfs:isDefinedBy <http://parliament.uk/ontologies/parliamentary-paper/> .
	
ppaper:hasPrivilege rdf:type owl:DatatypeProperty ;
	rdfs:label "Has privilege"@en ;
	rdfs:comment "Used to record if parliamentary papers being items in a series indicates that those papers have parliamentary privilege."@en ;
	rdfs:domain ppaper:PaperSeries ;
	rdfs:range xsd:boolean ;
	rdfs:isDefinedBy <http://parliament.uk/ontologies/parliamentary-paper/> .
	
ppaper:authoredOn rdf:type owl:DatatypeProperty ;
	rdfs:label "Authored on"@en ;
	rdfs:comment "Relates a parliamentary paper expression to the date that paper was authored on."@en ;
	rdfs:domain ppaper:ParliamentaryPaperExpression ;
	rdfs:range xsd:date ;
	rdfs:isDefinedBy <http://parliament.uk/ontologies/parliamentary-paper/> .
	
ppaper:copyrightStatement rdf:type owl:DatatypeProperty ;
	rdfs:label "Copyright statement"@en ;
	rdfs:comment "Relates a parliamentary paper expression to a statement containing the copyright description for that paper."@en ;
	rdfs:domain ppaper:ParliamentaryPaperExpression ;
	rdfs:range rdf:langString ;
	rdfs:isDefinedBy <http://parliament.uk/ontologies/parliamentary-paper/> .
	
ppaper:pageCount rdf:type owl:DatatypeProperty ;
	rdfs:label "Page count"@en ;
	rdfs:comment "Relates a parliamentary paper expression to its page count."@en ;
	rdfs:domain ppaper:ParliamentaryPaperExpression ;
	rdfs:range xsd:integer ;
	rdfs:isDefinedBy <http://parliament.uk/ontologies/parliamentary-paper/> .
	
ppaper:containsStatistics rdf:type owl:DatatypeProperty ;
	rdfs:label "Contains statistics"@en ;
	rdfs:comment "Used to record if a parliamentary paper expression contains statistics."@en ;
	rdfs:domain ppaper:ParliamentaryPaperExpression ;
	rdfs:range xsd:boolean ;
	rdfs:isDefinedBy <http://parliament.uk/ontologies/parliamentary-paper/> .