@prefix phm: <http://parliament.uk/ontologies/house-membership/> . 
@prefix xsd: <http://www.w3.org/2001/XMLSchema#> . 
@prefix rdf: <http://www.w3.org/1999/02/22-rdf-syntax-ns#> .
@prefix dcterms: <http://purl.org/dc/terms/> .
@prefix owl:     <http://www.w3.org/2002/07/owl#> .
@prefix rdfs:    <http://www.w3.org/2000/01/rdf-schema#> .
@prefix foaf:	<http://xmlns.com/foaf/0.1/> .

<http://parliament.uk/ontologies/house-membership/> 
    rdf:type owl:Ontology ;
    dcterms:title "House membership ontology"@en ;
    dcterms:created "2016-11-08"^^xsd:date ;
	dcterms:rights "Open Parliament Licence v3.0"@en ;
    dcterms:description "A model describing the occupation by a person of a seat in a House, by means of an incumbency over a period of time."@en ;
	foaf:depiction <https://ukparliament.github.io/ontologies/house-membership/house-membership.svg> ;
	foaf:maker
		[ foaf:name "Robert Brook"; foaf:homepage <https://robert-brook.com/> ],
		[ foaf:name "Ned Morrell" ],
		[ foaf:name "Anna Murphy" ],
		[ foaf:name "Michael Smethurst"; foaf:homepage <http://smethur.st/> ],
	    [ foaf:name "Anya Somerville" ].


#######  Classes ##### 	

phm:House rdf:type owl:Class ;
	rdfs:label "House"@en ;
	rdfs:comment "A parliamentary House, for example: the House of Lords."@en ;
	rdfs:isDefinedBy <http://parliament.uk/ontologies/house-membership/> .
	
phm:HouseSeat rdf:type owl:Class ;
	rdfs:label "House seat"@en ;
	rdfs:comment "A seat as a position in a House, rather than as a physical seat or constituency."@en ;
	rdfs:isDefinedBy <http://parliament.uk/ontologies/house-membership/> .
	
phm:SeatIncumbency rdf:type owl:Class ;
	rdfs:label "Seat incumbency"@en ;
	rdfs:comment "The occupation of a seat in a House by a person, for a period of time. A person may have only one seat incumbency at any one time, or none.  A person may have more than one seat incumbency over time. A seat incumbency is of one person."@en ;
	rdfs:isDefinedBy <http://parliament.uk/ontologies/house-membership/> .
	
phm:Person rdf:type owl:Class ;
	rdfs:label "Person"@en ;
	rdfs:comment "A person."@en ;
	rdfs:isDefinedBy <http://parliament.uk/ontologies/house-membership/> .
	
phm:HouseSeatType rdf:type owl:Class ;
	rdfs:label "House seat type"@en ;
	rdfs:comment "The type of a House seat, for example: seats in the House of Commons allocated by means of the first past the post electoral system, seats in the House of Lords allocated to hereditary peers, life peers, excepted hereditary peers or Lords Spiritual."@en ;
	rdfs:isDefinedBy <http://parliament.uk/ontologies/house-membership/> .
	
phm:HouseSeatEndReason rdf:type owl:Class ;
	rdfs:label "House Seat End reason"@en ;
	rdfs:comment "A reason for the ending of a House seat, for example: in the House of Commons, a seat may end by means of a constituency boundary change; in the House of Lords the passing of the House of Lords Act 1999 led to the expulsion of hereditary peers and the ending of their seats."@en ;
	rdfs:isDefinedBy <http://parliament.uk/ontologies/house-membership/> .

phm:HouseSeatEnablingThing rdf:type owl:Class ;
	rdfs:label "House seat enabling thing"@en ;
	rdfs:comment "The existence of a thing which enables a House seat to exist, for example: the existence of a constituency enabling a House seat to exist in the House of Commons; the existence of a life peerage enabling a House seat to exist in the House of Lords."@en ;
	rdfs:isDefinedBy <http://parliament.uk/ontologies/house-membership/> .
	
phm:SeatIncumbencyEndReason rdf:type owl:Class ;
	rdfs:label "Seat incumbency end reason"@en ;
	rdfs:comment "A reason for the ending of a seat incumbency, for example: the death of the Member holding that seat incumbency, the Member holding that seat incumbency no longer having membership of the House of Commons by means of appointment to a Crown Office, or the expulsion of the Member holding that seat incumbency from the House of Lords."@en ;
	rdfs:seeAlso <https://ukparliament.github.io/ontologies/house-membership/end-reasons/> ;
	rdfs:isDefinedBy <http://parliament.uk/ontologies/house-membership/> .
	
phm:SeatIncumbencyInterruptionPeriod rdf:type owl:Class ;
	rdfs:label "Seat incumbency interruption period"@en ;
	rdfs:comment "A period of interruption to a seat incumbency."@en ;
	rdfs:isDefinedBy <http://parliament.uk/ontologies/house-membership/> .
	
phm:Suspension rdf:type owl:Class ;
	rdfs:subClassOf phm:SeatIncumbencyInterruptionPeriod ;
	rdfs:label "Suspension"@en ;
	rdfs:comment "A period of time during which a Member of a House is suspended from taking part in the business of that House."@en ;
	rdfs:isDefinedBy <http://parliament.uk/ontologies/house-membership/> .
	
phm:LeaveOfAbsence rdf:type owl:Class ;
	rdfs:subClassOf  phm:SeatIncumbencyInterruptionPeriod ;
	rdfs:label "Leave of absence"@en ;
	rdfs:comment "A period of absence from a House notified in advance by the Member, during which the Member does not take part in the business of the House."@en ;
	rdfs:isDefinedBy <http://parliament.uk/ontologies/house-membership/> .
	
phm:HouseOfLordsDisqualification rdf:type owl:Class ;
	rdfs:subClassOf  phm:SeatIncumbencyInterruptionPeriod ;
	rdfs:label "House of Lords disqualification"@en ;
	rdfs:comment "A period of time during which a Member of a House of Lords is disqualified from taking part in the business of that House."@en ;
	rdfs:isDefinedBy <http://parliament.uk/ontologies/house-membership/> .
	
phm:HouseOfLordsDisqualificationType rdf:type owl:Class ;
	rdfs:label "House of Lords disqualification type"@en ;
	rdfs:comment "The type of disqualification of a disqualified Member of the House of Lords, for example: on the grounds of holding judicial office or being bankrupt."@en ;
	rdfs:isDefinedBy <http://parliament.uk/ontologies/house-membership/> .
	
phm:SeatIncumbencyEnablingThing rdf:type owl:Class ;
	rdfs:label "Seat incumbency enabling thing"@en ;
	rdfs:comment "The existence of a thing which enables a person to be incumbent in a House seat, for example: the winning of an election in a constituency represented in the House of Commons enabling a seat incumbency to exist in the House of Commons, or the holding of a life peerage enabling a seat incumbency to exist in the House of Lords.
"@en ;
	rdfs:isDefinedBy <http://parliament.uk/ontologies/house-membership/> .
	
phm:SwearingIn rdf:type owl:Class ;
	rdfs:label "Swearing in"@en ;
	rdfs:comment "The act of taking an oath, or making a solemn affirmation, of allegiance to the Crown by a Member of either House."@en ;
	rdfs:isDefinedBy <http://parliament.uk/ontologies/house-membership/> .
	
phm:ParliamentPeriod rdf:type owl:Class ;
	rdfs:label "Parliament period"@en ;
	rdfs:comment "The time period of a single Parliament between the date of its first assembly after a general election and its dissolution. A Parliament period contains contiguous session and prorogation periods. During a parliament period Parliament is either in session or prorogued. The start date of a Parliament may be changed by subsequent proclamations. A Parliament ends at the next dissolution. While the Fixed-term Parliaments Act 2011 was in force, the date of dissolution was determined by that Act or was named in a proclamation following a vote in Parliament for an early general election. The next Parliament began on the date named in the proclamation issued following a dissolution. Before the Fixed-term Parliaments Act 2011 came into force and after that Act was repealed by the Dissolution and Calling of Parliament Act 2022, the date of dissolution is fixed by proclamation. The dissolution proclamation also names the date for Parliament to reassemble. Parliament periods are the same across both Houses. Parliaments are numbered ordinally from the first Parliament of the United Kingdom, sitting in 1801."@en ;
	rdfs:isDefinedBy <http://parliament.uk/ontologies/house-membership/> .
	






	# edited to here
	
##### Object properties ####

phm:hasSeatIncumbencyInterruption rdf:type owl:ObjectProperty ;
	rdfs:label "Has seat incumbency interruption"@en ;
	rdfs:comment "Relates a seat incumbency to an interruption of that incumbency. An incumbency may be interrupted one or more times, or none. A seat incumbency interruption is of one seat incumbency."@en ;
	rdfs:domain phm:SeatIncumbency ;
	rdfs:range phm:SeatIncumbencyInterruption ;
	rdfs:isDefinedBy <http://parliament.uk/ontologies/house-membership/> .	

phm:inHouse rdf:type owl:ObjectProperty ;
	rdfs:label "In House"@en ;
	rdfs:comment "Relates a seat in a House to the House that the seat is in. A seat is in one House. "@en ;
	rdfs:domain phm:HouseSeat;
	rdfs:range phm:House ;
	rdfs:isDefinedBy <http://parliament.uk/ontologies/house-membership/> .
	
phm:inHouseSeat rdf:type owl:ObjectProperty ;
	rdfs:label "In House seat"@en ;
	rdfs:comment "Relates a seat incumbency to the House seat that the incumbency is in. A seat incumbency is in one seat. At any one time, a House seat has one incumbency or is unoccupied. A House seat may have more than one incumbency over time."@en ;
	rdfs:domain phm:SeatIncumbency ;
	rdfs:range phm:HouseSeat ;
	rdfs:isDefinedBy <http://parliament.uk/ontologies/house-membership/> .
	
phm:hasIncumbent rdf:type owl:ObjectProperty ;
	rdfs:label "Has incumbent"@en ;
	rdfs:comment "Relates a seat incumbency to a person. A seat incumbency is held by one person.  At any one time, a person may be incumbent in one seat, or none. A person may have many incumbencies in the same or different seats over time."@en ;
	rdfs:domain phm:SeatIncumbency ;
	rdfs:range phm:Person ;
	rdfs:isDefinedBy <http://parliament.uk/ontologies/house-membership/> .
	
phm:hasHouseSeatType rdf:type owl:ObjectProperty ;
	rdfs:label "Has House seat type"@en ;
	rdfs:comment "Relates a seat in a House to a seat type. A House seat is of one type."@en ;
	rdfs:domain phm:HouseSeat ;
	rdfs:range phm:HouseSeatType ;
	rdfs:isDefinedBy <http://parliament.uk/ontologies/house-membership/> .
	
phm:seatIncumbencyEndReason rdf:type owl:ObjectProperty ;
	rdfs:label "Seat incumbency end reason"@en ;
	rdfs:comment "Relates a seat incumbency to the reason for that incumbency ending. A seat incumbency may have one end reason, or none."@en ;
	rdfs:domain phm:SeatIncumbency ;
	rdfs:range phm:SeatIncumbencyEndReason ;
	rdfs:isDefinedBy <http://parliament.uk/ontologies/house-membership/> .
	
phm:houseSeatEndReason rdf:type owl:ObjectProperty ;
	rdfs:label "House seat end reason"@en ;
	rdfs:comment "Relates a House seat to the reason for that seat ending. A House seat may have one end reason, or none."@en ;
	rdfs:domain phm:HouseSeat ;
	rdfs:range phm:EndReason ;
	rdfs:isDefinedBy <http://parliament.uk/ontologies/house-membership/> .
	
phm:inParliamentPeriod rdf:type owl:ObjectProperty ;
	rdfs:label "In Parliament period"@en ;
	rdfs:comment "Relates a seat incumbency in the House of Commons to the Parliament period containing that incumbency. Seat incumbencies in the House of Commons are related to one Parliament period. Seat incumbencies in the House of Lords are not related to a Parliament period: Members of the Lords are considered to be Members across dissolution periods."@en ;
	rdfs:domain phm:SeatIncumbency ;
	rdfs:range phm:ParliamentPeriod ;
	rdfs:isDefinedBy <http://parliament.uk/ontologies/house-membership/> .
	
phm:hasHouseOfLordsDisqualificationType rdf:type owl:ObjectProperty ;
	rdfs:label "Has House of Lords disqualification type"@en ;
	rdfs:comment "Relates a disqualification to the type of that disqualification. A disqualification is of one type."@en ;
	rdfs:domain phm:HouseOfLordsDisqualification ;
	rdfs:range phm:HouseOfLordsDisqualificationType ;
	rdfs:isDefinedBy <http://parliament.uk/ontologies/house-membership/> .

phm:houseSeatEnabledBy rdf:type owl:ObjectProperty ;
	rdfs:label "House seat enabled by"@en ;
	rdfs:comment "Relates a House seat to the thing enabling the existence of that seat, for example: a peerage, a constituency or a named bishopric."@en ;
	rdfs:domain phm:HouseSeat ;
	rdfs:range phm:HouseSeatEnablingThing ;
	rdfs:isDefinedBy <http://parliament.uk/ontologies/house-membership/> .

phm:seatIncumbencyEnabledBy rdf:type owl:ObjectProperty ;
	rdfs:label "Seat incumbency enabled by"@en ;
	rdfs:comment "Relates a seat incumbency to the thing enabling the existence of that incumbency, for example: the holding of a peerage, the winning of a constituency election or an incumbency in a named bishopric."@en ;
	rdfs:domain phm:SeatIncumbency ;
	rdfs:range phm:SeatIncumbencyEnablingThing ;
	rdfs:isDefinedBy <http://parliament.uk/ontologies/house-membership/> .
				
	
##### Data properties ####	
			
phm:swearingInOrder rdf:type owl:DatatypeProperty ;
	rdfs:label "Swearing in order"@en ;
	rdfs:comment "Used to record the place in the order in which Members take an oath or make an affirmation at the beginning of a new Parliament or following a by-election. Swearing in order may be used in determining the longest serving member of a House, known as the Father or Mother of the House."@en ;
	rdfs:domain phm:SeatIncumbency ;
	rdfs:range xsd:integer ;
	rdfs:isDefinedBy <http://parliament.uk/ontologies/house-membership/> .
	
phm:intendsToStandDown rdf:type owl:DatatypeProperty ;
	rdfs:label "Intends to stand down"@en ;
	rdfs:comment "Used to record if a Member of the House of Commons has announced that they intend to stand down at the next election."@en ;
	rdfs:domain phm:SeatIncumbency ;
	rdfs:range xsd:boolean ;
	rdfs:isDefinedBy <http://parliament.uk/ontologies/house-membership/> .
						