@prefix ppsa: <http://parliament.uk/ontologies/procedure-step-annotation/> . 
@prefix xsd: <http://www.w3.org/2001/XMLSchema#> . 
@prefix rdf: <http://www.w3.org/1999/02/22-rdf-syntax-ns#> .
@prefix dcterms: <http://purl.org/dc/terms/> .
@prefix owl:     <http://www.w3.org/2002/07/owl#> .
@prefix rdfs:    <http://www.w3.org/2000/01/rdf-schema#> .
@prefix foaf:	<http://xmlns.com/foaf/0.1/> .

<http://parliament.uk/ontologies/procedure-step-annotation/> 
    rdf:type owl:Ontology ;
    dcterms:title "Procedure step ontology"@en ;
    dcterms:created "2019-04-16"^^xsd:date ;
	dcterms:rights "Open Parliament Licence v3.0"@en ;
    dcterms:description "A model describing annotations added to event steps in the procedure model by the Indexing and Data Management Section of the House of Commons Library. Annotations are used to describe how an event step is actualised."@en ;
	foaf:depiction <https://ukparliament.github.io/ontologies/procedure-step-annotation/procedure-step-annotation.svg> ;
	foaf:maker
	    [ foaf:name "Jayne Bosworth" ],
		[ foaf:name "Robert Brook"; foaf:homepage <https://robert-brook.com/> ],
		[ foaf:name "Michael Smethurst"; foaf:homepage <http://smethur.st/> ],
	    [ foaf:name "Anya Somerville" ] .


#######  Classes ##### 	

ppsa:EventStep rdf:type owl:Class ;
	rdfs:label "Event step"@en ;
	rdfs:comment "A procedural step of type event, being the notion of a event happening in the House of Commons, the House of Lords, bicamerally, in a devolved legislature or external to Parliament and the devolved legislatures."@en ;
	rdfs:isDefinedBy <http://parliament.uk/ontologies/procedure-step-annotation/> .
	
ppsa:Publication rdf:type owl:Class ;
	rdfs:label "Publication"@en ;
	rdfs:comment "A publication."@en ;
	rdfs:isDefinedBy <http://parliament.uk/ontologies/procedure-step-annotation/> .
	
	
	
##### Object properties ####

ppsa:actualiseWith rdf:type owl:ObjectProperty ;
	rdfs:label "Actualise with"@en ;
	rdfs:comment "Relates an event step to an event step where steps may be actualised together."@en ;
	rdfs:domain ppsa:EventStep ;
	rdfs:range ppsa:EventStep ;
	rdfs:isDefinedBy <http://parliament.uk/ontologies/procedure-step-annotation/> .

ppsa:source rdf:type owl:ObjectProperty ;
	rdfs:label "Source"@en ;
	rdfs:comment "Relates an event step to the publication which is the source of information for that event actualising the event step."@en ;
	rdfs:domain ppsa:EventStep ;
	rdfs:range ppsa:Publication ;
	rdfs:isDefinedBy <http://parliament.uk/ontologies/procedure-step-annotation/> .
	
	
	
##### Data properties ####	
	
ppsa:linkNote rdf:type owl:DatatypeProperty ;
	rdfs:label "Link note"@en ;
	rdfs:comment "A note that describes where an event, actualising an event step, should link to in a publication."@en ;
	rdfs:domain ppsa:EventStep ;
	rdfs:range rdf:langString ;
	rdfs:isDefinedBy <http://parliament.uk/ontologies/procedure-step-annotation/> .
	
ppsa:dateNote rdf:type owl:DatatypeProperty ;
	rdfs:label "Date note"@en ;
	rdfs:comment "A note that describes the date to use when actualising an event step."@en ;
	rdfs:domain ppsa:EventStep ;
	rdfs:range rdf:langString ;
	rdfs:isDefinedBy <http://parliament.uk/ontologies/procedure-step-annotation/> .
						