@prefix ppsa: <http://parliament.uk/ontologies/procedure-step-annotation/> . 
@prefix xsd: <http://www.w3.org/2001/XMLSchema#> . 
@prefix rdf: <http://www.w3.org/1999/02/22-rdf-syntax-ns#> .
@prefix dcterms: <http://purl.org/dc/terms/> .
@prefix owl:     <http://www.w3.org/2002/07/owl#> .
@prefix rdfs:    <http://www.w3.org/2000/01/rdf-schema#> .
@prefix foaf:	<http://xmlns.com/foaf/0.1/> .

<http://parliament.uk/ontologies/procedure-step-annotation/> 
    rdf:type owl:Ontology ;
    dcterms:title "Procedure step ontology"@en ;
    dcterms:created "2019-04-16"^^xsd:date ;
	dcterms:rights "Open Parliament Licence v3.0"@en ;
    dcterms:description "A model describing annotations added to business steps in the procedure model by the Indexing and Data Management Section of the House of Commons Library. Annotations are used to describe how a business step is actualised."@en ;
	foaf:depiction <https://ukparliament.github.io/ontologies/procedure-step-annotation/procedure-step-annotation.svg> ;
	foaf:maker
	    [ foaf:name "Jayne Bosworth" ],
		[ foaf:name "Robert Brook"; foaf:homepage <https://robert-brook.com/> ],
		[ foaf:name "Michael Smethurst"; foaf:homepage <http://smethur.st/> ],
	    [ foaf:name "Anya Somerville" ] .


#######  Classes ##### 	

ppsa:BusinessStep rdf:type owl:Class ;
	rdfs:label "Business step"@en ;
	rdfs:comment "A step of type business. A business step describes a set of potential business items, for example: the potential for papers to be laid before the House of Commons. Potential business items described by a business step may take place inside or outside Parliament."@en ;
	rdfs:isDefinedBy <http://parliament.uk/ontologies/procedure-step-annotation/> .
	
ppsa:Publication rdf:type owl:Class ;
	rdfs:label "Publication"@en ;
	rdfs:comment "A publication."@en ;
	rdfs:isDefinedBy <http://parliament.uk/ontologies/procedure-step-annotation/> .
	
	
	
##### Object properties ####

ppsa:actualisesAlongside rdf:type owl:ObjectProperty ;
	rdfs:label "Actualised alongside"@en ;
	rdfs:comment "Relates a business step to another business step where the two steps may be actualised alongside each other as a single business item."@en ;
	rdfs:domain ppsa:BusinessStep ;
	rdfs:range ppsa:BusinessStep ;
	rdfs:isDefinedBy <http://parliament.uk/ontologies/procedure-step-annotation/> .

ppsa:source rdf:type owl:ObjectProperty ;
	rdfs:label "Source"@en ;
	rdfs:comment "Relates a business step to the publication which is the source of information for the business item actualising that business step."@en ;
	rdfs:domain ppsa:BusinessStep ;
	rdfs:range ppsa:Publication ;
	rdfs:isDefinedBy <http://parliament.uk/ontologies/procedure-step-annotation/> .
	
	
	
##### Data properties ####	
	
ppsa:linkNote rdf:type owl:DatatypeProperty ;
	rdfs:label "Link note"@en ;
	rdfs:comment "A note describing the nature of the link that should be added to a business item actualising a business step. For example: a business item actualising a business step describing the putting of a question in the House of Commons should link to the corresponding business item recorded in Votes and Proceedings."@en ;
	rdfs:domain ppsa:BusinessStep ;
	rdfs:range rdf:langString ;
	rdfs:isDefinedBy <http://parliament.uk/ontologies/procedure-step-annotation/> .
	
ppsa:dateNote rdf:type owl:DatatypeProperty ;
	rdfs:label "Date note"@en ;
	rdfs:comment "A note describing the nature of the date that should be added to a business item actualising a business step. For example: a business item actualising a business step describing committee consideration should use the date that the committee met, rather than the date on which the committee report was published."@en ;
	rdfs:domain ppsa:BusinessStep ;
	rdfs:range rdf:langString ;
	rdfs:isDefinedBy <http://parliament.uk/ontologies/procedure-step-annotation/> .
						