@prefix ppsa: <http://parliament.uk/ontologies/procedure-step-annotation/> . 
@prefix xsd: <http://www.w3.org/2001/XMLSchema#> . 
@prefix rdf: <http://www.w3.org/1999/02/22-rdf-syntax-ns#> .
@prefix dcterms: <http://purl.org/dc/terms/> .
@prefix owl:     <http://www.w3.org/2002/07/owl#> .
@prefix rdfs:    <http://www.w3.org/2000/01/rdf-schema#> .
@prefix foaf:	<http://xmlns.com/foaf/0.1/> .

<http://parliament.uk/ontologies/procedure-step-annotation/> 
    rdf:type owl:Ontology ;
    dcterms:title "Procedure step ontology"@en ;
    dcterms:created "2019-04-16"^^xsd:date ;
	dcterms:rights "Open Parliament Licence v3.0"@en ;
    dcterms:description "Ontology allowing annotation of procedure steps by the Indexing and Data Management Section in the House of Commons Library. Allows us to capture how and when procedure steps are actualised."@en ;
	foaf:depiction <https://ukparliament.github.io/ontologies/procedure-step-annotation/procedure-step-annotation.png> ;
	foaf:maker
		[ foaf:name "Michael Smethurst"; foaf:homepage <http://smethur.st/> ],
	    [ foaf:name "Anya Somerville" ].


#######  Classes ##### 	

ppsa:BusinessStep rdf:type owl:Class ;
	rdfs:label "Business step"@en ;
	rdfs:comment "A business step is a step that can be actualised by a business item."@en ;
	rdfs:isDefinedBy <http://parliament.uk/ontologies/procedure-step-annotation/> .
	
ppsa:Publication rdf:type owl:Class ;
	rdfs:label "Publication"@en ;
	rdfs:comment "An online publication."@en ;
	rdfs:isDefinedBy <http://parliament.uk/ontologies/procedure-step-annotation/> .
	

	

	
##### Object properties ####


ppsa:actualiseAlongside rdf:type owl:ObjectProperty ;
	rdfs:label "Actualise alongside"@en ;
	rdfs:comment "Relates a business step to a business step where steps are commonly actualised together."@en ;
	rdfs:domain ppsa:BusinessStep ;
	rdfs:range ppsa:BusinessStep ;
	rdfs:isDefinedBy <http://parliament.uk/ontologies/procedure-step-annotation/> .

ppsa:source rdf:type owl:ObjectProperty ;
	rdfs:label "Source"@en ;
	rdfs:comment "Relates a business step to the publication which is the authoritative source of information for that step."@en ;
	rdfs:domain ppsa:BusinessStep ;
	rdfs:range ppsa:Publication ;
	rdfs:isDefinedBy <http://parliament.uk/ontologies/procedure-step-annotation/> .
	

				
	
##### Data properties ####	

ppsa:scopeNote rdf:type owl:DatatypeProperty ;
	rdfs:label "Scope note"@en ;
	rdfs:comment "A note that clarifies the rules around actualising a business step."@en ;
	rdfs:domain ppsa:BusinessStep ;
	rdfs:range rdf:langString ;
	rdfs:isDefinedBy <http://parliament.uk/ontologies/procedure-step-annotation/> .
	
ppsa:linkNote rdf:type owl:DatatypeProperty ;
	rdfs:label "Link note"@en ;
	rdfs:comment "A note that clarifies where a business item should link to in a publication."@en ;
	rdfs:domain ppsa:BusinessStep ;
	rdfs:range rdf:langString ;
	rdfs:isDefinedBy <http://parliament.uk/ontologies/procedure-step-annotation/> .
	
ppsa:dateNote rdf:type owl:DatatypeProperty ;
	rdfs:label "Date note"@en ;
	rdfs:comment "A note that clarifies the date to use when actualising a business step."@en ;
	rdfs:domain ppsa:BusinessStep ;
	rdfs:range rdf:langString ;
	rdfs:isDefinedBy <http://parliament.uk/ontologies/procedure-step-annotation/> .
						