@prefix pl: <http://parliament.uk/ontologies/laying/> . 
@prefix xsd: <http://www.w3.org/2001/XMLSchema#> . 
@prefix rdf: <http://www.w3.org/1999/02/22-rdf-syntax-ns#> .
@prefix dcterms: <http://purl.org/dc/terms/> .
@prefix owl:     <http://www.w3.org/2002/07/owl#> .
@prefix rdfs:    <http://www.w3.org/2000/01/rdf-schema#> .
@prefix foaf:	<http://xmlns.com/foaf/0.1/> .

<http://parliament.uk/ontologies/laying/> 
    rdf:type owl:Ontology ;
    dcterms:title "Laying ontology"@en ;
    dcterms:created "2018-02-06"^^xsd:date ;
	dcterms:rights "Open Parliament Licence v3.0"@en ;
    dcterms:description "A model describing the laying of papers into a House and the authorities those papers are laid under."@en ;
	foaf:depiction <https://ukparliament.github.io/ontologies/laying/laying.svg> ;
	foaf:maker 
		[ foaf:name "Jayne Bosworth" ],
		[ foaf:name "Robert Brook"; foaf:homepage <https://robert-brook.com/> ],
		[ foaf:name "Jack Dent" ],
		[ foaf:name "Mike Hennessy" ],
		[ foaf:name "Matt Korris" ],
		[ foaf:name "Stephen McGinness" ],
		[ foaf:name "Ned Morrell" ],
		[ foaf:name "Michael Smethurst"; foaf:homepage <http://smethur.st/> ],
		[ foaf:name "Anya Somerville" ].


#######  Classes #####
	
pl:MakingAvailable rdf:type owl:Class ;
	rdfs:label "Making available"@en ;
	rdfs:comment "The act of making a thing available to a House or to a House by means of its Library."@en ;
	rdfs:isDefinedBy <http://parliament.uk/ontologies/laying/> .

pl:MadeAvailableThing rdf:type owl:Class ;
	rdfs:label "Made available thing"@en ;
	rdfs:comment "A thing made available to a House or to a House by means of its Library."@en ;
	rdfs:isDefinedBy <http://parliament.uk/ontologies/laying/> .
	
pl:PaperExpression rdf:type owl:Class ;
	rdfs:label "Paper expression"@en ;
	rdfs:comment "A paper made available to a House, being an expression of a paper work."@en ;
	rdfs:isDefinedBy <http://parliament.uk/ontologies/laying/> .
	
pl:Laying rdf:type owl:Class ;
	rdfs:subClassOf pl:MakingAvailable ;
	rdfs:label "Laying"@en ;
	rdfs:comment "The act of making a paper available to a House under a laying authority. Papers are made available to a House on being accepted by the Journal Office of that House."@en ;
	rdfs:isDefinedBy <http://parliament.uk/ontologies/laying/> .
	
pl:LaidPaper rdf:type owl:Class ;
	rdfs:subClassOf pl:MadeAvailableThing ;
	rdfs:subClassOf pl:PaperExpression ;
	rdfs:label "Laid paper"@en ;
	rdfs:comment "A paper having been laid before a House."@en ;
	rdfs:isDefinedBy <http://parliament.uk/ontologies/laying/> .

pl:LayingAuthorityCitation rdf:type owl:Class ;
	rdfs:label "Laying authority citation"@en ;
	rdfs:comment "A citation of the authority under which a paper is laid, for example: a section of legislation, a standing order or a resolution giving authorisation for that laying."@en ;
	rdfs:isDefinedBy <http://parliament.uk/ontologies/laying/> .

pl:LayingAuthorityType rdf:type owl:Class ;
	rdfs:label "Laying authority type"@en ;
	rdfs:comment "The type of an authority under which a paper is laid. A paper may be laid under prerogative powers and said to be laid 'by command'. A paper laid in order to comply with legislation may be said to be laid 'by Act'. A paper may be laid in order to comply with standing orders, or with an opposed or unopposed return motion."@en ;
	rdfs:isDefinedBy <http://parliament.uk/ontologies/laying/> .
	
	

#######  Object properties ##### 
	
pl:hasLayingAuthorityCitation rdf:type owl:ObjectProperty ;
	rdfs:label "Has laying authority citation"@en ;
	rdfs:comment "Relates an act of laying a paper to the citation of the authority under which that paper is laid. The laying of a paper has one authority citation, or none."@en ;
	rdfs:domain pl:Laying ;
	rdfs:range pl:LayingAuthorityCitation ;
	rdfs:isDefinedBy <http://parliament.uk/ontologies/laying/> .
	
pl:hasLayingAuthorityType rdf:type owl:ObjectProperty ;
	rdfs:label "Has laying authority type"@en ;
	rdfs:comment "Relates a laying to the type of the authority under which that laying is made. A laying has one laying authority type."@en ;
	rdfs:domain pl:Laying ;
	rdfs:range pl:LayingAuthorityType ;
	rdfs:isDefinedBy <http://parliament.uk/ontologies/laying/> .
	
pl:parentLayingAuthorityType rdf:type owl:ObjectProperty ;
	rdfs:label "Parent laying authority type"@en ;
	rdfs:comment "Relates a laying authority type to the parent of that laying authority type, for example: a laying authority type of 'by Act' having a parent laying authority type of 'by Statute'. A laying authority type may have one parent laying authority type, or none. A laying authority type may have one or more child laying authority types, or none."@en ;
	rdfs:domain pl:LayingAuthorityType ;
	rdfs:range pl:LayingAuthorityType ;
	rdfs:isDefinedBy <http://parliament.uk/ontologies/laying/> .
	
pl:resultsIn rdf:type owl:ObjectProperty ;
	rdfs:label "Results in"@en ;
	rdfs:comment "Relates an act of laying a paper to that paper having been laid. An act of laying is of one or more laid papers. A laid paper is the result of one act of laying."@en ;
	rdfs:domain pl:Laying ;
	rdfs:range pl:LaidPaper ;
	rdfs:isDefinedBy <http://parliament.uk/ontologies/laying/> .

				

#######  Data properties #####

pl:isAuditorCertified rdf:type owl:DatatypeProperty ;
	rdfs:label "Is auditor certified"@en ;
	rdfs:comment "Used to record whether a laid paper has been certified by an auditor."@en ;
	rdfs:domain pl:LaidPaper ;
	rdfs:range xsd:boolean ;
	rdfs:isDefinedBy <http://parliament.uk/ontologies/laying/> .