@prefix del: <http://parliament.uk/ontologies/delegation/> . 
@prefix xsd: <http://www.w3.org/2001/XMLSchema#> . 
@prefix rdf: <http://www.w3.org/1999/02/22-rdf-syntax-ns#> .
@prefix dcterms: <http://purl.org/dc/terms/> .
@prefix owl:     <http://www.w3.org/2002/07/owl#> .
@prefix rdfs:    <http://www.w3.org/2000/01/rdf-schema#> .
@prefix foaf:	<http://xmlns.com/foaf/0.1/> .

<http://parliament.uk/ontologies/delegation/> 
    rdf:type owl:Ontology ;
    dcterms:title "Delegation ontology"@en ;
    dcterms:created "2023-03-01"^^xsd:date ;
	dcterms:rights "Open Parliament Licence v3.0"@en ;
    dcterms:description "A model describing the enabling of secondary legislation."@en ;
	foaf:depiction <https://ukparliament.github.io/ontologies/delegation/delegation.svg> ;
	foaf:maker
		[ foaf:name "David Beamish" ],
		[ foaf:name "Robert Brook"; foaf:homepage <https://robert-brook.com/> ],
		[ foaf:name "Nerys Davies" ],
		[ foaf:name "Jack Dent" ],
		[ foaf:name "Samu Lang" ],
		[ foaf:name "Lucinda Maer" ],
		[ foaf:name "Silver Oliver" ],
		[ foaf:name "John Sheridan" ],
		[ foaf:name "Michael Smethurst"; foaf:homepage <http://smethur.st/> ],
	    [ foaf:name "Claire Searle" ],
	    [ foaf:name "Anya Somerville" ],
	    [ foaf:name "Jayne Sunley" ],
	    [ foaf:name "Matthew Waddington" ],
		[ foaf:name "Jane White" ].


#######  Classes #####

del:PaperWork rdf:type owl:Class ;
	rdfs:label "Paper work"@en ;
	rdfs:comment "A paper as a single intellectual work, as defined in the Functional Requirements for Bibliographic Records specification."@en ;
	rdfs:isDefinedBy <http://parliament.uk/ontologies/delegation/> .

del:LegislativeThing rdf:type owl:Class ;
	rdfs:label "Legislative thing"@en ;
	rdfs:comment "A legislative thing, for example: an Act of Parliament or a made statutory instrument."@en ;
	rdfs:isDefinedBy <http://parliament.uk/ontologies/delegation/> .
	
del:ActOfParliament rdf:type owl:Class ;
	rdfs:subClassOf del:LegislativeThing ;
	rdfs:label "Act of Parliament"@en ;
	rdfs:comment "An Act of Parliament creates, amends or repeals legislation. An Act is a Bill having been passed by Parliament and been given Royal Assent. Acts of Parliament which are in force comprise statute law."@en ;
	rdfs:isDefinedBy <http://parliament.uk/ontologies/delegation/> .
	
del:EnabledThing rdf:type owl:Class ;
	rdfs:subClassOf del:PaperWork ;
	rdfs:label "Enabled thing"@en ;
	rdfs:comment "A thing resulting from a Minister exercising or intending to exercise a power conferred by a legislative thing."@en ;
	rdfs:isDefinedBy <http://parliament.uk/ontologies/delegation/> .

del:PublishedDraftUnderEUWA2018Work rdf:type owl:Class ;
	rdfs:subClassOf del:EnabledThing ;
	rdfs:label "Published draft under the European Union (Withdrawal) Act 2018 work"@en ;
	rdfs:comment "A draft published under the duties laid out in paragraph 14 of schedule 8 of the European Union (Withdrawal) Act 2018. A Minister has a duty to publish such a draft 28 joint sitting days before the laying of an instrument intending to amend or revoke subordinate legislation under section 2(2) of the European Communities Act 1972, including subordinate legislation implementing EU directives."@en ;
	rdfs:isDefinedBy <http://parliament.uk/ontologies/delegation/> .
	
del:ProposedDraftRemedialOrderWork rdf:type owl:Class ;
	rdfs:subClassOf del:EnabledThing ;
	rdfs:label "Proposed draft remedial order work"@en ;
	rdfs:comment "A proposal for a draft remedial order. Under paragraph 3(1) of schedule 2 of the Human Rights Act 1998, the Minister has a duty to lay before Parliament 'a document which contains a draft of the proposed order'. This document must lay before Parliament for a period of 60 sitting days, beginning with the day on which it was laid."@en ;
	rdfs:isDefinedBy <http://parliament.uk/ontologies/delegation/> .

del:ProposedNegativeStatutoryInstrumentWork rdf:type owl:Class ;
	rdfs:subClassOf del:EnabledThing ;
	rdfs:label "Proposed negative statutory instrument work"@en ;
	rdfs:comment "A regulation made under a power or powers set out in clause 7, 8 or 9 of the European Union (Withdrawal) Act 2018, or under schedule 5 of the Future Relationship Act 2020, which government ministers propose be laid under the negative procedure. Sifting committees of either House may recommend that any subsequent statutory instrument or instruments be laid under the affirmative procedure."@en ;
	rdfs:isDefinedBy <http://parliament.uk/ontologies/delegation/> .

del:StatutoryInstrumentSubjectToParliamentaryProcedureWork rdf:type owl:Class ;
	rdfs:subClassOf del:EnabledThing ;
	rdfs:label "Statutory instrument subject to parliamentary procedure work"@en ;
	rdfs:comment "Statutory instruments subject to parliamentary procedure according to duties set out in legislation."@en ;
	rdfs:isDefinedBy <http://parliament.uk/ontologies/delegation/> .

del:DraftStatutoryInstrumentSubjectToParliamentaryProcedureWork rdf:type owl:Class ;
	rdfs:subClassOf del:StatutoryInstrumentSubjectToParliamentaryProcedureWork ;
	rdfs:label "Draft statutory instrument subject to parliamentary procedure work"@en ;
	rdfs:comment "An instrument laid in draft before Parliament subject to either a negative, affirmative or super affirmative procedure. An instrument under the draft negative procedure may be made into law, if not objected to within the scrutiny period. An instrument under the draft affirmative procedure may be made into law, having been approved by Parliament. An instrument under the draft super affirmative procedure may be made into law, having been approved by Parliament within the approval period."@en ;
	rdfs:isDefinedBy <http://parliament.uk/ontologies/delegation/> .

del:MadeStatutoryInstrumentSubjectToParliamentaryProcedureWork rdf:type owl:Class ;
	rdfs:subClassOf del:StatutoryInstrumentSubjectToParliamentaryProcedureWork ;
	rdfs:subClassOf del:LegislativeThing ;
	rdfs:label "Made statutory instrument subject to parliamentary procedure work"@en ;
	rdfs:comment "Statutory instruments as signed into law before being laid into Parliament. Made statutory instruments laid before Parliament are subject to a negative, affirmative or super affirmative procedure, or none. An instrument under the made negative procedure remains law unless objected to within the scrutiny period. An instrument under the made affirmative procedure or made super affirmative procedure remains law if approved by Parliament within the approval period."@en ;
	rdfs:isDefinedBy <http://parliament.uk/ontologies/delegation/> .



##### Object properties ####

del:enabledBy rdf:type owl:ObjectProperty ;
	rdfs:label "Enabled by"@en ;
	rdfs:comment "Relates an enabled thing to the legislative thing under which it was made or under which it is intended to be made. An enabled thing may be enabled by one or more legislative things. A legislative thing may enable one or more enabled things, or none."@en ;
	rdfs:domain del:EnabledThing ;
	rdfs:range del:LegislativeThing ;
	rdfs:isDefinedBy <http://parliament.uk/ontologies/delegation/> .
	
del:precededBy rdf:type owl:ObjectProperty ;
	rdfs:label "Preceded by"@en ;
	rdfs:comment "Relates an enabled thing to the enabled thing which preceded it. An enabled thing may be preceded by one or more enabled things, or by none. An enabled thing may precede one or more enabled things, or none. For example: a statutory instrument being preceded by a proposed negative statutory instrument."@en ;
	rdfs:domain del:EnabledThing ;
	rdfs:range del:EnabledThing ;
	rdfs:isDefinedBy <http://parliament.uk/ontologies/delegation/> .
	
del:replacedBy rdf:type owl:ObjectProperty ;
	rdfs:label "Replaced by"@en ;
	rdfs:comment "Relates a paper work to the paper work it is replaced by. A paper work may be replaced by one paper work, or none. A paper work being replaced is always replaced by a paper work of the same type. A paper work may replace one paper work, or none. For example: a draft statutory instrument replacing another draft statutory instrument, a proposed negative statutory instrument replacing another proposed negative statutory instrument or a treaty replacing another treaty. Made instruments cannot be replaced, only revoked."@en ;
	rdfs:domain del:PaperWork ;
	rdfs:range del:PaperWork ;
	rdfs:isDefinedBy <http://parliament.uk/ontologies/delegation/> ."
	
del:whollyRevokedBy rdf:type owl:ObjectProperty ;
	rdfs:label "Wholly revoked by"@en ;
	rdfs:comment "Relates a made statutory instrument subject to parliamentary procedure to the made statutory instrument it is wholly revoked by. A made statutory instrument can be wholly revoked by one made statutory instrument, or none. A made statutory instrument can wholly revoke one or more made statutory instruments, or none. 'Wholly revoked by' is populated for made statutory instruments revoked whilst still before Parliament. Revoking secondary legislation has an effect similar to repealing primary legislation. Wholly revoking a made statutory instrument removes that made statutory instrument from the statute book on the date it is revoked."@en ;
	rdfs:domain del:MadeStatutoryInstrumentSubjectToParliamentaryProcedureWork ;
	rdfs:range del:MadeStatutoryInstrumentSubjectToParliamentaryProcedureWork ;
	rdfs:isDefinedBy <http://parliament.uk/ontologies/delegation/> .
	
					
	
##### Data properties ####
	
del:madeDate rdf:type owl:DatatypeProperty ;
	rdfs:label "Made date"@en ;
	rdfs:comment "The date on which a statutory instrument is made by the person having the power to make it."@en ;
	rdfs:domain del:MadeStatutoryInstrumentSubjectToParliamentaryProcedureWork ;
	rdfs:range xsd:date ;
	rdfs:isDefinedBy <http://parliament.uk/ontologies/delegation/> .
	
del:comingIntoForceDate rdf:type owl:DatatypeProperty ;
	rdfs:label "Coming into force date"@en ;
	rdfs:comment "The date on which a statutory instrument comes into force. Schedules within an instrument may come into force on different dates. Coming into force details would be given in a coming into force note where no single coming into force date is given."@en ;
	rdfs:domain del:StatutoryInstrumentSubjectToParliamentaryProcedureWork ;
	rdfs:range xsd:date ;
	rdfs:isDefinedBy <http://parliament.uk/ontologies/delegation/> .
	
del:comingIntoForceNote rdf:type owl:DatatypeProperty ;
	rdfs:label "Coming into force note"@en ;
	rdfs:comment "A coming into force note sets out details of the commencement of provisions or effects forming part or parts of an instrument, or the instrument as a whole."@en ;
	rdfs:domain del:StatutoryInstrumentSubjectToParliamentaryProcedureWork ;
	rdfs:range rdf:langString ;
	rdfs:isDefinedBy <http://parliament.uk/ontologies/delegation/> .

del:chapterNumber rdf:type owl:DatatypeProperty ;
	rdfs:label "Chapter number"@en ;
	rdfs:comment "The identifier in a year part of an Act of Parliament number, for example, '12' in '1986 c. 12'."@en ;
	rdfs:domain del:ActOfParliament ;
	rdfs:range rdfs:Literal ;
	rdfs:isDefinedBy <http://parliament.uk/ontologies/delegation/> .

del:actYear rdf:type owl:DatatypeProperty ;
	rdfs:label "Act year"@en ;
	rdfs:comment "The year part of an Act of Parliament number, for example, '1986' in '1986 c. 12'. The Act year is the year in which Royal Assent was given."@en ;
	rdfs:domain del:ActOfParliament ;
	rdfs:range rdfs:Literal ;
	rdfs:isDefinedBy <http://parliament.uk/ontologies/delegation/> .

del:royalAssentOn rdf:type owl:DatatypeProperty ;
	rdfs:label "Royal Assent on"@en ;
	rdfs:comment "The date on which Royal Assent was given, as recorded by legislation.gov.uk. This may differ from the date recorded by Parliament if Royal Assent is given after midnight on a sitting day."@en ;
	rdfs:domain del:ActOfParliament ;
	rdfs:range xsd:date ;
	rdfs:isDefinedBy <http://parliament.uk/ontologies/delegation/> .

del:longTitle rdf:type owl:DatatypeProperty ;
	rdfs:label "Long title"@en ;
	rdfs:comment "The title of an Act, setting out in general terms its purpose or scope."@en ;
	rdfs:domain del:ActOfParliament ;
	rdfs:range rdf:langString ;
	rdfs:isDefinedBy <http://parliament.uk/ontologies/delegation/> .
