@prefix pso: <http://parliament.uk/ontologies/standing-order/> . 
@prefix xsd: <http://www.w3.org/2001/XMLSchema#> . 
@prefix rdf: <http://www.w3.org/1999/02/22-rdf-syntax-ns#> .
@prefix dcterms: <http://purl.org/dc/terms/> .
@prefix owl:     <http://www.w3.org/2002/07/owl#> .
@prefix rdfs:    <http://www.w3.org/2000/01/rdf-schema#> .
@prefix foaf:	<http://xmlns.com/foaf/0.1/> .

<http://parliament.uk/ontologies/standing-order/> 
    rdf:type owl:Ontology ;
    dcterms:title "Standing order ontology"@en ;
    dcterms:created "2020-12-07"^^xsd:date ;
	dcterms:rights "Open Parliament Licence v3.0"@en ;
    dcterms:description "A model describing standing orders of legislatures and changes to standing orders over time."@en;
	foaf:depiction <https://ukparliament.github.io/ontologies/standing-order/standing-order.svg> ;
	foaf:maker
		[ foaf:name "David Beamish" ],
		[ foaf:name "Robert Brook"; foaf:homepage <https://robert-brook.com/> ],
		[ foaf:name "Paul Evans" ],
		[ foaf:name "Thomas Fleming"; foaf:homepage <https://tgfleming.wordpress.com/> ],
		[ foaf:name "Niels D. Goet"; foaf:homepage <https://ngoet.com/> ],
		[ foaf:name "James Jefferies"; foaf:homepage <https://jamesjefferies.com/> ],
		[ foaf:name "Ned Morrell" ],
		[ foaf:name "Michael Smethurst"; foaf:homepage <http://smethur.st/> ],
		[ foaf:name "Anya Somerville" ],
	    [ foaf:name "Radoslaw Zubek"; foaf:homepage <https://radoslawzubek.com/> ].


#######  Classes #####

pso:Legislature rdf:type owl:Class ;
	rdfs:label "Legislature"@en ;
	rdfs:comment "A legislature, being either the UK Parliament or a devolved legislature."@en ;
	rdfs:isDefinedBy <http://parliament.uk/ontologies/standing-order/> .

pso:House rdf:type owl:Class ;
	rdfs:label "House"@en ;
	rdfs:comment "A parliamentary House, for example: the House of Lords."@en ;
	rdfs:isDefinedBy <http://parliament.uk/ontologies/standing-order/> .

pso:BusinessExtent rdf:type owl:Class ;
	rdfs:label "Business extent"@en ;
	rdfs:comment "The extent of business covered by a set of standing orders being, for example: public business or private business."@en ;
	rdfs:isDefinedBy <http://parliament.uk/ontologies/standing-order/> .
	
pso:RevisionSet rdf:type owl:Class ;
	rdfs:label "Revision set"@en ;
	rdfs:comment "A set of standing orders, as they exist at the time of revision of one or more of those orders."@en ;
	rdfs:isDefinedBy <http://parliament.uk/ontologies/standing-order/> .
	
pso:RevisionSetSection rdf:type owl:Class ;
	rdfs:label "Revision set section"@en ;
	rdfs:comment "A grouping of orders under the same title in a revision set."@en ;
	rdfs:isDefinedBy <http://parliament.uk/ontologies/standing-order/> .
	
pso:OrderVersion rdf:type owl:Class ;
	rdfs:label "Order version"@en ;
	rdfs:comment "A version of a standing order contained by a section of a revision set."@en ;
	rdfs:isDefinedBy <http://parliament.uk/ontologies/standing-order/> .
	
pso:Order rdf:type owl:Class ;
	rdfs:label "Order"@en ;
	rdfs:comment "A standing order with its associated intent, as a single intellectual work, as defined in the Functional Requirements for Bibliographic Records specification."@en ;
	rdfs:isDefinedBy <http://parliament.uk/ontologies/standing-order/> .
	
pso:FragmentVersion rdf:type owl:Class ;
	rdfs:label "Fragment version"@en ;
	rdfs:comment "A version of a fragment of a standing order, contained by a revision set."@en ;
	rdfs:isDefinedBy <http://parliament.uk/ontologies/standing-order/> .

pso:Fragment rdf:type owl:Class ;
	rdfs:label "Fragment"@en ;
	rdfs:comment "A fragment of a standing order with its associated intent, as a single intellectual work, as defined in the Functional Requirements for Bibliographic Records specification."@en ;
	rdfs:isDefinedBy <http://parliament.uk/ontologies/standing-order/> .
	
pso:Revision rdf:type owl:Class ;
	rdfs:label "Revision"@en ;
	rdfs:comment "A change to the text of a standing order fragment."@en ;
	rdfs:isDefinedBy <http://parliament.uk/ontologies/standing-order/> .

pso:SuspensionPeriod rdf:type owl:Class ;
	rdfs:label "Suspension period"@en ;
	rdfs:comment "A suspension period is the time during which one or more standing orders are suspended. A suspension period has a start date and, where specified, an end date. Some suspensions do not specify an end date, for example: the suspension of House of Lords Standing Order 10(6) (Hereditary peers: by-elections) pending a further report from the Procedure and Privileges Committee. An order may be 'suspended, for a period' or 'dispensed with, for a purpose'. The suspension period class covers suspensions, not dispensations."@en ;
	rdfs:isDefinedBy <http://parliament.uk/ontologies/standing-order/> .



#######  Object properties ##### 

pso:inLegislature rdf:type owl:ObjectProperty ;
	rdfs:label "In legislature"@en ;
	rdfs:comment "Relates a House to the legislature it forms part of, for example: the House of Commons forming part of the UK Parliament. A House forms part of one legislature."@en ;
	rdfs:domain pso:House ;
	rdfs:range pso:Legislature ;
	rdfs:isDefinedBy <http://parliament.uk/ontologies/standing-order/> .
	
pso:issuedByHouse rdf:type owl:ObjectProperty ;
	rdfs:label "Issued by House"@en ;
	rdfs:comment "Relates a revision set to the House that revision set is issued by. A revision set may be issued by one House, or none."@en ;
	rdfs:domain pso:RevisionSet ;
	rdfs:range pso:House ;
	rdfs:isDefinedBy <http://parliament.uk/ontologies/standing-order/> .
	
pso:issuedByLegislature rdf:type owl:ObjectProperty ;
	rdfs:label "Issued by legislature"@en ;
	rdfs:comment "Relates a revision set to the legislature that revision set is issued by. A revision set may be issued by one legislature, or none."@en ;
	rdfs:domain pso:RevisionSet ;
	rdfs:range pso:Legislature ;
	rdfs:isDefinedBy <http://parliament.uk/ontologies/standing-order/> .
	
pso:revisionSetCoversBusinessExtent rdf:type owl:ObjectProperty ;
	rdfs:label "Revision set covers business extent"@en ;
	rdfs:comment "Relates a revision set to the business extent which that revision set covers. A revision set covers one business extent."@en ;
	rdfs:domain pso:RevisionSet ;
	rdfs:range pso:BusinessExtent ;
	rdfs:isDefinedBy <http://parliament.uk/ontologies/standing-order/> .

pso:revisionSetSectionContainedBy rdf:type owl:ObjectProperty ;
	rdfs:label "Revision set section contained by"@en ;
	rdfs:comment "Relates a revision set section to the revision set it is contained by. A revision set section is contained by one revision set."@en ;
	rdfs:domain pso:RevisionSetSection ;
	rdfs:range pso:RevisionSet ;
	rdfs:isDefinedBy <http://parliament.uk/ontologies/standing-order/> .
	
pso:orderVersionContainedBy rdf:type owl:ObjectProperty ;
	rdfs:label "Order version contained by"@en ;
	rdfs:comment "Relates an order version to the section of a revision set it is contained by. An order version is contained by one revision set section."@en ;
	rdfs:domain pso:OrderVersion ;
	rdfs:range pso:RevisionSetSection ;
	rdfs:isDefinedBy <http://parliament.uk/ontologies/standing-order/> .
	
pso:fragmentVersionContainedBy rdf:type owl:ObjectProperty ;
	rdfs:label "Fragment version contained by"@en ;
	rdfs:comment "Relates a fragment version to the revision set it is contained by. A fragment version is contained by one revision set."@en ;
	rdfs:domain pso:FragmentVersion ;
	rdfs:range pso:RevisionSet ;
	rdfs:isDefinedBy <http://parliament.uk/ontologies/standing-order/> .
	
pso:formsPartOf rdf:type owl:ObjectProperty ;
	rdfs:label "Forms part of"@en ;
	rdfs:comment "Relates a fragment version to the order version it forms part of. A fragment version forms part of one order version."@en ;
	rdfs:domain pso:FragmentVersion ;
	rdfs:range pso:OrderVersion ;
	rdfs:isDefinedBy <http://parliament.uk/ontologies/standing-order/> .
	
pso:revisionFrom rdf:type owl:ObjectProperty ;
	rdfs:label "Revision from"@en ;
	rdfs:comment "Relates a revision to the fragment version being revised. A revision is from one fragment version."@en ;
	rdfs:domain pso:Revision ;
	rdfs:range pso:FragmentVersion ;
	rdfs:isDefinedBy <http://parliament.uk/ontologies/standing-order/> .

pso:revisionTo rdf:type owl:ObjectProperty ;
	rdfs:label "Revision to"@en ;
	rdfs:comment "Relates a revision to the fragment version resulting from the revision. A revision is to one fragment version."@en ;
	rdfs:domain pso:Revision ;
	rdfs:range pso:FragmentVersion ;
	rdfs:isDefinedBy <http://parliament.uk/ontologies/standing-order/> .
	
pso:orderOfHouse rdf:type owl:ObjectProperty ;
	rdfs:label "Order of House"@en ;
	rdfs:comment "Relates an order to the House of which it is an order. An order is of one House, or none."@en ;
	rdfs:domain pso:Order ;
	rdfs:range pso:House ;
	rdfs:isDefinedBy <http://parliament.uk/ontologies/standing-order/> .
	
pso:orderOfLegislature rdf:type owl:ObjectProperty ;
	rdfs:label "Order of legislature"@en ;
	rdfs:comment "Relates an order to the legislature of which it is an order. An order is of one legislature, or none."@en ;
	rdfs:domain pso:Order ;
	rdfs:range pso:Legislature ;
	rdfs:isDefinedBy <http://parliament.uk/ontologies/standing-order/> .
	
pso:versionOfOrder rdf:type owl:ObjectProperty ;
	rdfs:label "Version of order"@en ;
	rdfs:comment "Relates an order version to the order it is a version of. An order version is a version of one order."@en ;
	rdfs:domain pso:OrderVersion ;
	rdfs:range pso:Order ;
	rdfs:isDefinedBy <http://parliament.uk/ontologies/standing-order/> .

pso:versionOfFragment rdf:type owl:ObjectProperty ;
	rdfs:label "Version of fragment"@en ;
	rdfs:comment "Relates a fragment version to the fragment it is a version of. A fragment version is a version of one fragment."@en ;
	rdfs:domain pso:FragmentVersion ;
	rdfs:range pso:Fragment ;
	rdfs:isDefinedBy <http://parliament.uk/ontologies/standing-order/> .

pso:suspensionPeriodOfOrder rdf:type owl:ObjectProperty ;
	rdfs:label "Suspension period of order"@en ;
	rdfs:comment "Relates a suspension period to the order or orders that are suspended for that period. A suspension period applies to one or more orders."@en ;
	rdfs:domain pso:SuspensionPeriod ;
	rdfs:range pso:Order ;
	rdfs:isDefinedBy <http://parliament.uk/ontologies/standing-order/> .
	
	
	
#######  Data properties ##### 

pso:text rdf:type owl:DatatypeProperty ;
	rdfs:label "Text"@en ;
	rdfs:comment "Relates a fragment version to the text content of that fragment version."@en ;
	rdfs:domain pso:FragmentVersion ;
	rdfs:range rdf:langString ;
	rdfs:isDefinedBy <http://parliament.uk/ontologies/standing-order/> .
	
pso:paragraphNumber rdf:type owl:DatatypeProperty ;
	rdfs:label "Paragraph number"@en ;
	rdfs:comment "Relates an order version to the paragraph number for that order version, for example: '7' in '(7) The Member presiding may not vote in any ballot'. An order version has one paragraph number, or none."@en ;
	rdfs:domain pso:OrderVersion ;
	rdfs:range rdfs:Literal ;
	rdfs:isDefinedBy <http://parliament.uk/ontologies/standing-order/> .
	
pso:subParagraphNumber rdf:type owl:DatatypeProperty ;
	rdfs:label "Sub-paragraph number"@en ;
	rdfs:comment "Relates an order version to the sub-paragraph number for that order version, for example: 'c' in '(c) on Thursdays beginning at 1.30 pm and continuing for up to three hours'. An order version has one sub-paragraph number, or none."@en ;
	rdfs:domain pso:OrderVersion ;
	rdfs:range rdfs:Literal ;
	rdfs:isDefinedBy <http://parliament.uk/ontologies/standing-order/> .
	
pso:subSubParagraphNumber rdf:type owl:DatatypeProperty ;
	rdfs:label "Sub-sub-paragraph number"@en ;
	rdfs:comment "Relates an order version to the sub-sub-paragraph number for that order version, for example: 'ii' in '(ii) in Westminster Hall, at the commencement of proceedings'. An order version has one sub-sub-paragraph number, or none."@en ;
	rdfs:domain pso:OrderVersion ;
	rdfs:range rdfs:Literal ;
	rdfs:isDefinedBy <http://parliament.uk/ontologies/standing-order/> .

pso:isMajorRevision rdf:type owl:DatatypeProperty ;
	rdfs:label "Is major revision"@en ;
	rdfs:comment "Records if the revision is considered to be major: a TRUE value indicates a change of wording to the text content, a FALSE value indicates a change in casing with no change of wording."@en ;
	rdfs:domain pso:Revision ;
	rdfs:range xsd:boolean ;
	rdfs:isDefinedBy <http://parliament.uk/ontologies/standing-order/> .