@prefix pso: <http://parliament.uk/ontologies/standing-order/> . 
@prefix xsd: <http://www.w3.org/2001/XMLSchema#> . 
@prefix rdf: <http://www.w3.org/1999/02/22-rdf-syntax-ns#> .
@prefix dcterms: <http://purl.org/dc/terms/> .
@prefix owl:     <http://www.w3.org/2002/07/owl#> .
@prefix rdfs:    <http://www.w3.org/2000/01/rdf-schema#> .
@prefix foaf:	<http://xmlns.com/foaf/0.1/> .

<http://parliament.uk/ontologies/standing-order/> 
    rdf:type owl:Ontology ;
    dcterms:title "Standing order ontology"@en ;
    dcterms:created "2020-12-07"^^xsd:date ;
	dcterms:rights "Open Parliament Licence v3.0"@en ;
    dcterms:description "A model describing standing orders for both Houses of Parliament, establishing persistent identification of orders and fragments of orders."@en;
	foaf:depiction <https://ukparliament.github.io/ontologies/standing-order/standing-order.svg> ;
	foaf:maker
		[ foaf:name "David Beamish" ],
		[ foaf:name "Robert Brook"; foaf:homepage <https://robert-brook.com/> ],
		[ foaf:name "Paul Evans" ],
		[ foaf:name "Thomas Fleming"; foaf:homepage <https://tgfleming.wordpress.com/> ],
		[ foaf:name "Niels D. Goet"; foaf:homepage <https://ngoet.com/> ],
		[ foaf:name "Michael Smethurst"; foaf:homepage <http://smethur.st/> ],
		[ foaf:name "Anya Somerville" ],
	    [ foaf:name "Radoslaw Zubek"; foaf:homepage <https://radoslawzubek.com/> ].


#######  Classes #####

pso:Legislature rdf:type owl:Class ;
	rdfs:label "Legislature"@en ;
	rdfs:comment "A legislature, being either the UK Parliament or a devolved legislature."@en ;
	rdfs:isDefinedBy <http://parliament.uk/ontologies/standing-order/> .

pso:House rdf:type owl:Class ;
	rdfs:label "House"@en ;
	rdfs:comment "A parliamentary House, for example: the House of Lords."@en ;
	rdfs:isDefinedBy <http://parliament.uk/ontologies/standing-order/> .

pso:BusinessExtent rdf:type owl:Class ;
	rdfs:label "Business extent"@en ;
	rdfs:comment "Sets out the extent of business covered by a standing order as public business or private business."@en ;
	rdfs:isDefinedBy <http://parliament.uk/ontologies/standing-order/> .
	
pso:RevisionSet rdf:type owl:Class ;
	rdfs:label "Revision set"@en ;
	rdfs:comment "A set of sections, containing orders, as they exist at the time of revision of one or more orders."@en ;
	rdfs:isDefinedBy <http://parliament.uk/ontologies/standing-order/> .
	
pso:RevisionSetSection rdf:type owl:Class ;
	rdfs:label "Revision set section"@en ;
	rdfs:comment "A grouping of orders in a revision set."@en ;
	rdfs:isDefinedBy <http://parliament.uk/ontologies/standing-order/> .
	
pso:OrderVersion rdf:type owl:Class ;
	rdfs:label "Order version"@en ;
	rdfs:comment "A version of an order contained by a section of a revision set."@en ;
	rdfs:isDefinedBy <http://parliament.uk/ontologies/standing-order/> .
	
pso:Order rdf:type owl:Class ;
	rdfs:label "Order"@en ;
	rdfs:comment "An order is an FRBR-style work level item, wrapping different manifestations - described as versions - over time. It represents a platonic entity and associated intent."@en ;
	rdfs:isDefinedBy <http://parliament.uk/ontologies/standing-order/> .

pso:FragmentVersion rdf:type owl:Class ;
	rdfs:label "Fragment version"@en ;
	rdfs:comment "A version of a fragment of a standing order, contained by a revision set."@en ;
	rdfs:isDefinedBy <http://parliament.uk/ontologies/standing-order/> .

pso:Fragment rdf:type owl:Class ;
	rdfs:label "Fragment"@en ;
	rdfs:comment "A fragment is an FRBR-style work level item, wrapping different manifestations - described as fragment versions - over time. It represents a platonic entity and associated intent."@en ;
	rdfs:isDefinedBy <http://parliament.uk/ontologies/standing-order/> .

pso:Revision rdf:type owl:Class ;
	rdfs:label "Revision"@en ;
	rdfs:comment "A revision is a change to the text of a standing order fragment."@en ;
	rdfs:isDefinedBy <http://parliament.uk/ontologies/standing-order/> .

pso:SuspensionPeriod rdf:type owl:Class ;
	rdfs:label "Suspension period"@en ;
	rdfs:comment "A suspension period is the time during which one or more standing orders, or fragments of standing orders, are suspended. A suspension period has a start date and, where specified, an end date. These dates are set out in the utility model. Some suspensions do not specify an end date, for example: the suspension of House of Lords Standing Order 10(6) (Hereditary peers: by-elections) pending a further report from the Procedure and Privileges Committee. An order or fragment may be 'suspended, for a period' or 'dispensed with, for a purpose'. Orders and fragments may be dispensed with on a case by case basis: in the House of Commons this is usually indicated by the presence of 'notwithstanding' in the text of the motion. The suspension period class only covers suspensions and does not cover cases where standing orders are dispensed with. The procedure maps have steps which express the dispensing of standing orders."@en ;
	rdfs:isDefinedBy <http://parliament.uk/ontologies/standing-order/> .



#######  Object properties ##### 

pso:inLegislature rdf:type owl:ObjectProperty ;
	rdfs:label "In legislature"@en ;
	rdfs:comment "Relates a House to the Legislature it forms part of. This is only used to relate the House of Commons and the House of Lords to the UK Parliament, devolved legislatures being unicameral."@en ;
	rdfs:domain pso:House ;
	rdfs:range pso:Legislature ;
	rdfs:isDefinedBy <http://parliament.uk/ontologies/standing-order/> .

pso:issuedByHouse rdf:type owl:ObjectProperty ;
	rdfs:label "Issued by House"@en ;
	rdfs:comment "Relates a revision set to the House it is issued by. A revision set may be issued by one House, or none."@en ;
	rdfs:domain pso:RevisionSet ;
	rdfs:range pso:House ;
	rdfs:isDefinedBy <http://parliament.uk/ontologies/standing-order/> .
	
pso:issuedByLegislature rdf:type owl:ObjectProperty ;
	rdfs:label "Issued by legislature"@en ;
	rdfs:comment "Relates a revision set to the legislature it is issued by. A revision set may be issued by one legislature, or none."@en ;
	rdfs:domain pso:RevisionSet ;
	rdfs:range pso:Legislature ;
	rdfs:isDefinedBy <http://parliament.uk/ontologies/standing-order/> .
	
pso:revisionSetCoversBusinessExtent rdf:type owl:ObjectProperty ;
	rdfs:label "Revision set covers business extent"@en ;
	rdfs:comment "Relates a revision set to the business extent which that set covers."@en ;
	rdfs:domain pso:RevisionSet ;
	rdfs:range pso:BusinessExtent ;
	rdfs:isDefinedBy <http://parliament.uk/ontologies/standing-order/> .

pso:revisionSetSectionContainedBy rdf:type owl:ObjectProperty ;
	rdfs:label "Revision set section contained by"@en ;
	rdfs:comment "Relates a revision set section to the revision set it is contained by."@en ;
	rdfs:domain pso:RevisionSetSection ;
	rdfs:range pso:RevisionSet ;
	rdfs:isDefinedBy <http://parliament.uk/ontologies/standing-order/> .
	
pso:orderVersionContainedBy rdf:type owl:ObjectProperty ;
	rdfs:label "Order version contained by"@en ;
	rdfs:comment "Relates an order version to the section of a revision set it is contained by."@en ;
	rdfs:domain pso:OrderVersion ;
	rdfs:range pso:RevisionSetSection ;
	rdfs:isDefinedBy <http://parliament.uk/ontologies/standing-order/> .
	
pso:fragmentVersionContainedBy rdf:type owl:ObjectProperty ;
	rdfs:label "Fragment version contained by"@en ;
	rdfs:comment "Relates a fragment version to the revision set it is contained by."@en ;
	rdfs:domain pso:FragmentVersion ;
	rdfs:range pso:RevisionSet ;
	rdfs:isDefinedBy <http://parliament.uk/ontologies/standing-order/> .
	
pso:containedBy rdf:type owl:ObjectProperty ;
	rdfs:label "Contained by"@en ;
	rdfs:comment "Relates a fragment version to the order version it is contained by."@en ;
	rdfs:domain pso:FragmentVersion ;
	rdfs:range pso:OrderVersion ;
	rdfs:isDefinedBy <http://parliament.uk/ontologies/standing-order/> .

pso:revisionFrom rdf:type owl:ObjectProperty ;
	rdfs:label "Revision from"@en ;
	rdfs:comment "Relates a revision to the fragment version being revised."@en ;
	rdfs:domain pso:Revision ;
	rdfs:range pso:FragmentVersion ;
	rdfs:isDefinedBy <http://parliament.uk/ontologies/standing-order/> .

pso:revisionTo rdf:type owl:ObjectProperty ;
	rdfs:label "Revision to"@en ;
	rdfs:comment "Relates a revision to the fragment version resulting from the revision."@en ;
	rdfs:domain pso:Revision ;
	rdfs:range pso:FragmentVersion ;
	rdfs:isDefinedBy <http://parliament.uk/ontologies/standing-order/> .

pso:orderedByHouse rdf:type owl:ObjectProperty ;
	rdfs:label "Ordered by House"@en ;
	rdfs:comment "Relates an order to the House by which it was ordered."@en ;
	rdfs:domain pso:Order ;
	rdfs:range pso:House ;
	rdfs:isDefinedBy <http://parliament.uk/ontologies/standing-order/> .
	
pso:orderedByLegislature rdf:type owl:ObjectProperty ;
	rdfs:label "Ordered by legislature"@en ;
	rdfs:comment "Relates an order to the legislature by which it was ordered."@en ;
	rdfs:domain pso:Order ;
	rdfs:range pso:Legislature ;
	rdfs:isDefinedBy <http://parliament.uk/ontologies/standing-order/> .
	
pso:versionOfOrder rdf:type owl:ObjectProperty ;
	rdfs:label "Version of order"@en ;
	rdfs:comment "Relates an order version to the order it is a version of."@en ;
	rdfs:domain pso:OrderVersion ;
	rdfs:range pso:Order ;
	rdfs:isDefinedBy <http://parliament.uk/ontologies/standing-order/> .

pso:versionOfFragment rdf:type owl:ObjectProperty ;
	rdfs:label "Version of fragment"@en ;
	rdfs:comment "Relates a fragment version to the fragment it is a version of."@en ;
	rdfs:domain pso:FragmentVersion ;
	rdfs:range pso:Fragment ;
	rdfs:isDefinedBy <http://parliament.uk/ontologies/standing-order/> .

pso:suspensionPeriodOfOrder rdf:type owl:ObjectProperty ;
	rdfs:label "Suspension period of order"@en ;
	rdfs:comment "Relates a suspension period to the order that is suspended for that period."@en ;
	rdfs:domain pso:SuspensionPeriod ;
	rdfs:range pso:Order ;
	rdfs:isDefinedBy <http://parliament.uk/ontologies/standing-order/> .
	
pso:suspensionPeriodOfFragment rdf:type owl:ObjectProperty ;
	rdfs:label "Suspension period of fragment"@en ;
	rdfs:comment "Relates a suspension period to the fragment that is suspended for that period."@en ;
	rdfs:domain pso:SuspensionPeriod ;
	rdfs:range pso:Fragment ;
	rdfs:isDefinedBy <http://parliament.uk/ontologies/standing-order/> .
	
				

#######  Data properties ##### 

pso:revisedOn rdf:type owl:DatatypeProperty ;
	rdfs:label "Revised on"@en ;
	rdfs:comment "Relates a revision set to the date on which one or more orders contained by the revision set were revised."@en ;
	rdfs:domain pso:RevisionSet ;
	rdfs:range xsd:date ;
	rdfs:isDefinedBy <http://parliament.uk/ontologies/standing-order/> .
	
pso:revisionSetOrdinality rdf:type owl:DatatypeProperty ;
	rdfs:label "Revision set ordinality"@en ;
	rdfs:comment "Relates a revision set to its position in the list of revision sets. Allows more than one revision set to occur on the same calendar day."@en ;
	rdfs:domain pso:RevisionSet ;
	rdfs:range xsd:integer ;
	rdfs:isDefinedBy <http://parliament.uk/ontologies/standing-order/> .
	
pso:text rdf:type owl:DatatypeProperty ;
	rdfs:label "Text"@en ;
	rdfs:comment "Relates a fragment version to the text content of that fragment version."@en ;
	rdfs:domain pso:FragmentVersion ;
	rdfs:range rdf:langString ;
	rdfs:isDefinedBy <http://parliament.uk/ontologies/standing-order/> .
	
pso:paragraphNumber rdf:type owl:DatatypeProperty ;
	rdfs:label "Paragraph number"@en ;
	rdfs:comment "Relates an order version to the paragraph number for that order version, for example: '7' in 'The Member presiding may not vote in any ballot'. An order version has one paragraph number, or none."@en ;
	rdfs:domain pso:OrderVersion ;
	rdfs:range rdfs:Literal ;
	rdfs:isDefinedBy <http://parliament.uk/ontologies/standing-order/> .
	
pso:subParagraphNumber rdf:type owl:DatatypeProperty ;
	rdfs:label "Sub-paragraph number"@en ;
	rdfs:comment "Relates an order version to the sub-paragraph number for that order version, for example: 'c' in '(c) on Thursdays beginning at 1.30 pm and continuing for up to three hours'. An order version has one sub-paragraph number, or none."@en ;
	rdfs:domain pso:OrderVersion ;
	rdfs:range rdfs:Literal ;
	rdfs:isDefinedBy <http://parliament.uk/ontologies/standing-order/> .
	
pso:subSubParagraphNumber rdf:type owl:DatatypeProperty ;
	rdfs:label "Sub-sub-paragraph number"@en ;
	rdfs:comment "Relates an order version to the sub-sub-paragraph number for that order version, for example: 'ii' in '(ii) in Westminster Hall, at the commencement of proceedings'. An order version has one sub-sub-paragraph number, or none."@en ;
	rdfs:domain pso:OrderVersion ;
	rdfs:range rdfs:Literal ;
	rdfs:isDefinedBy <http://parliament.uk/ontologies/standing-order/> .
	
pso:fragmentVersionOrdinality rdf:type owl:DatatypeProperty ;
	rdfs:label "Fragment version ordinality"@en ;
	rdfs:comment "Relates a fragment version to the position of that fragment version in the list of fragment versions contained by a revision set."@en ;
	rdfs:domain pso:FragmentVersion ;
	rdfs:range xsd:integer ;
	rdfs:isDefinedBy <http://parliament.uk/ontologies/standing-order/> .

pso:isMajorRevision rdf:type owl:DatatypeProperty ;
	rdfs:label "Is major revision"@en ;
	rdfs:comment "Relates a revision to boolean describing if the revision is major: a FALSE value indicates only a change of case to the text content, a TRUE value indicates a major revision involving a change of wording to the text content."@en ;
	rdfs:domain pso:Revision ;
	rdfs:range xsd:boolean ;
	rdfs:isDefinedBy <http://parliament.uk/ontologies/standing-order/> .