@prefix ps: <https://parliament.uk/ontologies/submission/> . 
@prefix xsd: <http://www.w3.org/2001/XMLSchema#> . 
@prefix rdf: <http://www.w3.org/1999/02/22-rdf-syntax-ns#> .
@prefix dcterms: <http://purl.org/dc/terms/> .
@prefix owl:     <http://www.w3.org/2002/07/owl#> .
@prefix rdfs:    <http://www.w3.org/2000/01/rdf-schema#> .

<https://parliament.uk/ontologies/submission/> 
    rdf:type owl:Ontology ;
    dcterms:title "Submission ontology"@en ;
    dcterms:created "29/08/2017"^^xsd:date ;
	dcterms:rights "Open Parliament Licence v3.0"@en ;
    dcterms:description "Ontology to describe calls from Parliament for submission of evidence and resulting submissions."@en .


#######  Classes ##### 	

ps:Event rdf:type owl:Class ;
	rdfs:label "Event"@en ;
	rdfs:comment "An event. A thing that happens over a time interval."@en ;
	rdf:isDefinedBy <https://parliament.uk/ontologies/submission/> .
	
ps:CalendarEvent rdf:type owl:Class ;
	rdfs:label "CalendarEvent"@en ;
	rdfs:comment "A planned or arranged event in a place."@en ;
	rdf:isDefinedBy <https://parliament.uk/ontologies/submission/> .
	
ps:Call rdf:type owl:Class ;
	rdfs:subClassOf ps:Event ;
	rdfs:label "Call"@en ;
	rdfs:comment "A call by a committee or committees conducting an inquiry for written evidence, oral evidence, papers or records."@en ;
	rdf:isDefinedBy <https://parliament.uk/ontologies/submission/> .

ps:CallForOralEvidence rdf:type owl:Class ;
	rdfs:subClassOf ps:Call ;
	rdfs:label "CallForOralEvidence"@en ;
	rdfs:comment "A call by a committee or committees conducting an inquiry for a named witness to provide oral evidence."@en ;
	rdf:isDefinedBy <https://parliament.uk/ontologies/submission/> .

ps:Compelled rdf:type owl:Class ;
	rdfs:subClassOf ps:CallForOralEvidence ;
	rdfs:label "Compelled"@en ;
	rdfs:comment "A call by a committee or committees conducting an inquiry compelling a named witness to provide oral evidence."@en ;
	rdf:isDefinedBy <https://parliament.uk/ontologies/submission/> .

ps:CallForPapers rdf:type owl:Class ;
	rdfs:subClassOf ps:Call ;
	rdfs:label "CallForPapers"@en ;
	rdfs:comment "A call by a committee or committees conducting an inquiry for a named individual or organisation to provide papers. Papers are understood to be documents that the individual or organisation are unlikely to possess but would be able to compile."@en ;
	rdf:isDefinedBy <https://parliament.uk/ontologies/submission/> .

ps:CallForRecords rdf:type owl:Class ;
	rdfs:subClassOf ps:Call ;
	rdfs:label "CallForRecords"@en ;
	rdfs:comment "A call by a committee or committees conducting an inquiry for a named individual or organisation to provide records. Records are understood to be documents that the individual or organisation are known to possess."@en ;
	rdf:isDefinedBy <https://parliament.uk/ontologies/submission/> .

ps:CallForEvidence rdf:type owl:Class ;
	rdfs:subClassOf ps:Call ;
	rdfs:label "CallForEvidence"@en ;
	rdfs:comment "An open call by a committee or committees conducting an inquiry for members of the public or organisations to provide written evidence. Sometimes referred to as a call for written submissions."@en ;
	rdf:isDefinedBy <https://parliament.uk/ontologies/submission/> .

ps:Contribution rdf:type owl:Class ;
	rdfs:label "Contribution"@en ;
	rdfs:comment "A contribution by an individual or organisation to a committee inquiry. This might be in the form of written evidence, oral evidence, papers or records."@en ;
	rdf:isDefinedBy <https://parliament.uk/ontologies/submission/> .

ps:Person rdf:type owl:Class ;
	rdfs:label "Person"@en ;
	rdfs:comment "A person."@en ;
	rdf:isDefinedBy <https://parliament.uk/ontologies/submission/> .

ps:Document rdf:type owl:Class ;
	rdfs:label "Document"@en ;
	rdfs:comment "A document."@en ;
	rdf:isDefinedBy <https://parliament.uk/ontologies/submission/> .

ps:Focus rdf:type owl:Class ;
	rdfs:label "Focus"@en ;
	rdfs:comment "A focus area for a contribution. Borrowed from the formal body ontology to identify the subject area or areas covered by a contribution."@en ;
	rdf:isDefinedBy <https://parliament.uk/ontologies/submission/> .

ps:Incumbency rdf:type owl:Class ;
	rdfs:label "Incumbency"@en ;
	rdfs:comment "A position held by a person for a period of time e.g. Philip Hammond occupying the position of Foreign Secretary between two dates."@en ;
	rdf:isDefinedBy <https://parliament.uk/ontologies/submission/> .
	

	

	
##### Object properties ####


ps:compelledToAttend rdf:type owl:ObjectProperty ;
	rdfs:label "compelledToAttend"@en ;
	rdfs:comment "Relates a compelled call for oral evidence to a calendar event where the witness is expected to be heard."@en ;
	rdfs:domain ps:Compelled ;
	rdfs:range ps:CalendarEvent ;
	rdf:isDefinedBy <https://parliament.uk/ontologies/submission/> .
	
ps:callForOralEvidence rdf:type owl:ObjectProperty ;
	rdfs:label "callForOralEvidence"@en ;
	rdfs:comment "Relates a call for oral evidence to a contribution made in response to that call."@en ;
	rdfs:domain ps:CallForOralEvidence ;
	rdfs:range ps:Contribution ;
	rdf:isDefinedBy <https://parliament.uk/ontologies/submission/> .
	
ps:callForPapers rdf:type owl:ObjectProperty ;
	rdfs:label "callForPapers"@en ;
	rdfs:comment "Relates a call for papers to a contribution made in response to that call."@en ;
	rdfs:domain ps:CallForPapers ;
	rdfs:range ps:Contribution ;
	rdf:isDefinedBy <https://parliament.uk/ontologies/submission/> .
	
ps:callForRecords rdf:type owl:ObjectProperty ;
	rdfs:label "callForRecords"@en ;
	rdfs:comment "Relates a call for records to a contribution made in response to that call."@en ;
	rdfs:domain ps:CallForRecords ;
	rdfs:range ps:Contribution ;
	rdf:isDefinedBy <https://parliament.uk/ontologies/submission/> .
	
ps:respondsToCall rdf:type owl:ObjectProperty ;
	rdfs:label "respondsToCall"@en ;
	rdfs:comment "Relates any type of contribution to the call it is submitted in response to."@en ;
	rdfs:domain ps:Contribution ;
	rdfs:range ps:Call ;
	rdf:isDefinedBy <https://parliament.uk/ontologies/submission/> .
	
ps:makesContribution rdf:type owl:ObjectProperty ;
	rdfs:label "makesContribution"@en ;
	rdfs:comment "Relates a person making a contribution to their contribution."@en ;
	rdfs:domain ps:Person ;
	rdfs:range ps:Contribution ;
	rdf:isDefinedBy <https://parliament.uk/ontologies/submission/> .
	
ps:contributes rdf:type owl:ObjectProperty ;
	rdfs:label "contributes"@en ;
	rdfs:comment "Relates a contribution to a document contributed."@en ;
	rdfs:domain ps:Contribution ;
	rdfs:range ps:Document ;
	rdf:isDefinedBy <https://parliament.uk/ontologies/submission/> .
	
ps:focusOfContribution rdf:type owl:ObjectProperty ;
	rdfs:label "focusOfContribution"@en ;
	rdfs:comment "Relates a contribution to its focus (subject) area(s)."@en ;
	rdfs:domain ps:Contribution ;
	rdfs:range ps:Focus ;
	rdf:isDefinedBy <https://parliament.uk/ontologies/submission/> .
	
ps:inCapacity rdf:type owl:ObjectProperty ;
	rdfs:label "inCapacity"@en ;
	rdfs:comment "Relates a contribution to the incumbency of the person making the contribution e.g. a person making a contribution in their capacity of holding a CEO position of an organisation."@en ;
	rdfs:domain ps:Contribution ;
	rdfs:range ps:Incumbency ;
	rdf:isDefinedBy <https://parliament.uk/ontologies/submission/> .
	

				
	
##### Data properties ####	

ps:callDescription rdf:type owl:DatatypeProperty ;
	rdfs:label "callDescription"@en ;
	rdfs:comment "Relates any type of call to its descriptive text."@en ;
	rdfs:domain ps:Call ;
	rdfs:range rdf:langString ;
	rdf:isDefinedBy <https://parliament.uk/ontologies/submission/> .	

ps:calledAt rdf:type owl:DatatypeProperty ;
	rdfs:label "calledAt"@en ;
	rdfs:comment "The date time at which a call is made."@en ;
	rdfs:domain ps:Call ;
	rdfs:range xsd:dateTime ;
	rdf:isDefinedBy <https://parliament.uk/ontologies/submission/> .	

ps:callEnds rdf:type owl:DatatypeProperty ;
	rdfs:label "callEnds"@en ;
	rdfs:comment "The date time at which a call ends."@en ;
	rdfs:domain ps:Call ;
	rdfs:range xsd:dateTime ;
	rdf:isDefinedBy <https://parliament.uk/ontologies/submission/> .	
						