@prefix pgo: <https://parliament.uk/ontologies/government-organisation/> . 
@prefix xsd: <http://www.w3.org/2001/XMLSchema#> . 
@prefix rdf: <http://www.w3.org/1999/02/22-rdf-syntax-ns#> .
@prefix dcterms: <http://purl.org/dc/terms/> .
@prefix owl:     <http://www.w3.org/2002/07/owl#> .
@prefix rdfs:    <http://www.w3.org/2000/01/rdf-schema#> .

<https://parliament.uk/ontologies/government-organisation/> 
    rdf:type owl:Ontology ;
    dcterms:title "Government organisation ontology"@en ;
    dcterms:created "29/09/2017"^^xsd:date ;
	dcterms:rights "Open Parliament Licence v3.0"@en ;
    dcterms:description "Government organisation ontology for UK Parliament"@en .


#######  Classes ##### 	

pgo:Incumbency rdf:type owl:Class ;
	rdfs:label "Incumbency"@en ;
	rdfs:comment "A position held by a person for a period of time. e.g. Philip Hammond occupying the position of Foreign Secretary between two dates."@en ;
	rdf:isDefinedBy <https://parliament.uk/ontologies/government-organisation/> .
	
pgo:Position rdf:type owl:Class ;
	rdfs:label "Position"@en ;
	rdfs:comment "A position in a group that persists over time which can be occupied by different people at different times e.g. many people have been Foreign Secretary."@en ;
	rdf:isDefinedBy <https://parliament.uk/ontologies/government-organisation/> .
	
pgo:Group rdf:type owl:Class ;
	rdfs:label "Group"@en ;
	rdfs:comment "A group of people or a group of groups or a group of people and groups."@en ;
	rdf:isDefinedBy <https://parliament.uk/ontologies/government-organisation/> .
	
pgo:GovernmentIncumbency rdf:type owl:Class ;
	rdfs:subClassOf pgo:Incumbency ;
	rdfs:label "GovernmentIncumbency"@en ;
	rdfs:comment "An incumbency of a person in a government position. This is a specialisation of an incumbency from the agency ontology."@en ;
	rdf:isDefinedBy <https://parliament.uk/ontologies/government-organisation/> .

pgo:GovernmentPosition rdf:type owl:Class ;
	rdfs:subClassOf pgo:Position ;
	rdfs:label "GovernmentPosition"@en ;
	rdfs:comment "A position (job) in a government organisation. Note that not all government positions are in government organisations. e.g. Minister without Portfolio is a position outside any department, agency or public body. This is a specialisation of a position from the agency ontology."@en ;
	rdf:isDefinedBy <https://parliament.uk/ontologies/government-organisation/> .
	
pgo:AttendsCabinet rdf:type owl:Class ;
	rdfs:label "AttendsCabinet"@en ;
	rdfs:comment "Used to determine if the person incumbent in a government position is able to attend cabinet. Possible values are always, never and when required."@en ;
	rdf:isDefinedBy <https://parliament.uk/ontologies/government-organisation/> .

pgo:GovernmentRank rdf:type owl:Class ;
	rdfs:label "GovernmentRank"@en ;
	rdfs:comment "A packaging of ways to describe the rank of a government position. Different bodies have different ways to describe these."@en ;
	rdf:isDefinedBy <https://parliament.uk/ontologies/government-organisation/> .

pgo:GovernmentOrganisation rdf:type owl:Class ;
	rdfs:subClassOf pgo:Group ;
	rdfs:label "GovernmentOrganisation"@en ;
	rdfs:comment "Government departments, agencies and public bodies which have responsibility for a specific sector of public administration. Is a specialised type of group."@en ;
	rdf:isDefinedBy <https://parliament.uk/ontologies/government-organisation/> .
	
#######  Object properties ##### 

pgo:attendsCabinet rdf:type owl:ObjectProperty ;
	rdfs:label "attendsCabinet"@en ;
	rdfs:comment "Relates a government position to cabinet attendance."@en ;
	rdfs:domain pgo:GovernmentPosition ;
	rdfs:range pgo:AttendsCabinet ;
	rdf:isDefinedBy <https://parliament.uk/ontologies/government-organisation/> .	

pgo:hasRank rdf:type owl:ObjectProperty ;
	rdfs:label "hasRank"@en ;
	rdfs:comment "Relates a government position to assorted ways of describing rank."@en ;
	rdfs:domain pgo:GovernmentPosition ;
	rdfs:range pgo:GovernmentRank ;
	rdf:isDefinedBy <https://parliament.uk/ontologies/government-organisation/> .

#######  Data properties ##### 

pgo:isPaid rdf:type owl:DatatypeProperty ;
	rdfs:label "isPaid"@en ;
	rdfs:comment "Used to describe whether an incumbency is paid or not."@en ;
	rdfs:domain pgo:GovernmentIncumbency ;
	rdfs:range xsd:boolean ;
	rdf:isDefinedBy <https://parliament.uk/ontologies/government-organisation/> .

pgo:cabinetRank rdf:type owl:DatatypeProperty ;
	rdfs:label "cabinetRank"@en ;
	rdfs:comment "Used to capture how the government ranks assorted positions in the cabinet. e.g. whether the Foreign Secretary is ranked above or below the Health Secretary."@en ;
	rdfs:domain pgo:GovernmentPosition ;
	rdfs:range xsd:integer ;
	rdf:isDefinedBy <https://parliament.uk/ontologies/government-organisation/> .

pgo:paidToAttendCabinet rdf:type owl:DatatypeProperty ;
	rdfs:label "paidToAttendCabinet"@en ;
	rdfs:comment "Used to determine whether a government position is paid to attend cabinet or not."@en ;
	rdfs:domain pgo:GovernmentPosition ;
	rdfs:range xsd:boolean ;
	rdf:isDefinedBy <https://parliament.uk/ontologies/government-organisation/> .

pgo:isLayingPosition rdf:type owl:DatatypeProperty ;
	rdfs:label "isLayingPosition"@en ;
	rdfs:comment "Used to determine if a government position has the authority to lay papers into Parliament."@en ;
	rdfs:domain pgo:GovernmentPosition ;
	rdfs:range xsd:boolean ;
	rdf:isDefinedBy <https://parliament.uk/ontologies/government-organisation/> .

pgo:ministerialRank rdf:type owl:DatatypeProperty ;
	rdfs:label "ministerialRank"@en ;
	rdfs:comment ""@en ;
	rdfs:domain pgo:GovernmentRank ;
	rdfs:range xsd:integer ;
	rdf:isDefinedBy <https://parliament.uk/ontologies/government-organisation/> .

pgo:statsRank rdf:type owl:DatatypeProperty ;
	rdfs:label "statsRank"@en ;
	rdfs:comment ""@en ;
	rdfs:domain pgo:GovernmentRank ;
	rdfs:range rdf:langString ;
	rdf:isDefinedBy <https://parliament.uk/ontologies/government-organisation/> .

pgo:clerksRank rdf:type owl:DatatypeProperty ;
	rdfs:label "clerksRank"@en ;
	rdfs:comment ""@en ;
	rdfs:domain pgo:GovernmentRank ;
	rdfs:range rdf:langString ;
	rdf:isDefinedBy <https://parliament.uk/ontologies/government-organisation/> .

pgo:orderRank rdf:type owl:DatatypeProperty ;
	rdfs:label "orderRank"@en ;
	rdfs:comment ""@en ;
	rdfs:domain pgo:GovernmentRank ;
	rdfs:range xsd:integer ;
	rdf:isDefinedBy <https://parliament.uk/ontologies/government-organisation/> .
	
pgo:governmentSortOrder rdf:type owl:DatatypeProperty ;
	rdfs:label "governmentSortOrder"@en ;
	rdfs:comment "Used to determine how the government chooses to order government organisations. e.g. whether they choose to rank the Foreign Office higher than the Department of Health."@en ;
	rdfs:domain pgo:GovernmentOrganisation ;
	rdfs:range xsd:integer ;
	rdf:isDefinedBy <https://parliament.uk/ontologies/government-organisation/> .
	
pgo:oppositionSortOrder rdf:type owl:DatatypeProperty ;
	rdfs:label "oppositionSortOrder"@en ;
	rdfs:comment "Used to determine how the official opposition chooses to order government organisations. e.g. whether they choose to rank the Foreign Office higher than the Department of Health."@en ;
	rdfs:domain pgo:GovernmentOrganisation ;
	rdfs:range xsd:integer ;
	rdf:isDefinedBy <https://parliament.uk/ontologies/government-organisation/> .