@prefix pcp: <http://parliament.uk/ontologies/contact-point/> . 
@prefix xsd: <http://www.w3.org/2001/XMLSchema#> . 
@prefix rdf: <http://www.w3.org/1999/02/22-rdf-syntax-ns#> .
@prefix dcterms: <http://purl.org/dc/terms/> .
@prefix owl:     <http://www.w3.org/2002/07/owl#> .
@prefix rdfs:    <http://www.w3.org/2000/01/rdf-schema#> .
@prefix foaf:	<http://xmlns.com/foaf/0.1/> .

<http://parliament.uk/ontologies/contact-point/> 
    rdf:type owl:Ontology ;
    dcterms:title "Contact point ontology"@en ;
    dcterms:created "2017-01-27"^^xsd:date ;
	dcterms:rights "Open Parliament Licence v3.0"@en ;
    dcterms:description ""@en ;
    dcterms:description "A model describing contact points for contactable things."@en ;
	foaf:depiction <https://ukparliament.github.io/ontologies/contact-point/contact-point.svg> ;
	foaf:maker
		[ foaf:name "Robert Brook"; foaf:homepage <https://robert-brook.com/> ],
		[ foaf:name "Ned Morrell" ],
		[ foaf:name "Michael Smethurst"; foaf:homepage <https://smethur.st/> ].


#######  Classes #####

pcp:ContactableThing rdf:type owl:Class ;
	rdfs:label "Contactable thing"@en ;
	rdfs:comment "A thing that can be contacted. This is a group or a person in the context of their role in or their membership of a group."@en ;
	rdfs:isDefinedBy <http://parliament.uk/ontologies/contact-point/> .
	
pcp:ContactPoint rdf:type owl:Class ;
	rdfs:label "Contact point"@en ;
	rdfs:comment "One or more means of contact for a contactable thing, for example: a contact point having a postal address."@en ;
	rdfs:isDefinedBy <http://parliament.uk/ontologies/contact-point/> .
	
pcp:OnlineAccount rdf:type owl:Class ;
	rdfs:label "Online account"@en ;
	rdfs:comment "A online account, for example: an online account for the UK Parliament on X."@en ;
	rdfs:isDefinedBy <http://parliament.uk/ontologies/contact-point/> .
	
pcp:OnlineAccountProvider rdf:type owl:Class ;
	rdfs:label "Online account provider"@en ;
	rdfs:comment "A provider of online accounts, for example: X."@en ;
	rdfs:isDefinedBy <http://parliament.uk/ontologies/contact-point/> .
	
pcp:PostalAddress rdf:type owl:Class ;
	rdfs:label "Postal address"@en ;
	rdfs:comment "A postal address."@en ;
	rdfs:isDefinedBy <http://parliament.uk/ontologies/contact-point/> .
	
	
	
#######  Object properties ##### 

pcp:hasContactPoint rdf:type owl:ObjectProperty ;
	rdfs:label "Has contact point"@en ;
	rdfs:comment "Relates a contactable thing to a contact point. A contactable thing may have one or more contact points. A contact point is for one contactable thing."@en ;
	rdfs:domain pcp:ContactableThing ;
	rdfs:range pcp:ContactPoint ;
	rdfs:isDefinedBy <http://parliament.uk/ontologies/contact-point/> .
	
pcp:hasOnlineAccount rdf:type owl:ObjectProperty ;
	rdfs:label "Has online account"@en ;
	rdfs:comment "Relates a contact point to an online account. A contact point may have one or more online accounts, or none."@en ;
	rdfs:domain pcp:ContactPoint ;
	rdfs:range pcp:OnlineAccount ;
	rdfs:isDefinedBy <http://parliament.uk/ontologies/contact-point/> .
	
pcp:hasProvider rdf:type owl:ObjectProperty ;
	rdfs:label "Has provider"@en ;
	rdfs:comment "Relates an online account to the provider of that account. An online account has one provider."@en ;
	rdfs:domain pcp:OnlineAccount ;
	rdfs:range pcp:OnlineAccountProvider ;
	rdfs:isDefinedBy <http://parliament.uk/ontologies/contact-point/> .
	
pcp:hasPostalAddress rdf:type owl:ObjectProperty ;
	rdfs:label "Has postal address"@en ;
	rdfs:comment "Relates a contact point to its postal address. A contact point has one or more postal addresses or none."@en ;
	rdfs:domain pcp:ContactPoint ;
	rdfs:range pcp:PostalAddress ;
	rdfs:isDefinedBy <http://parliament.uk/ontologies/contact-point/> .
				

#######  Data properties #####

pcp:accountName rdf:type owl:DatatypeProperty ;
	rdfs:label "Account name"@en ;
	rdfs:comment "Relates an online account to the name of that account. For example: UK Parliament having an account on X with the name @ukparliament."@en ;
	rdfs:domain pcp:OnlineAccount ;
	rdfs:range rdfs:Literal ;
	rdfs:isDefinedBy <http://parliament.uk/ontologies/contact-point/> .

pcp:accountURL rdf:type owl:DatatypeProperty ;
	rdfs:label "Account URL"@en ;
	rdfs:comment "Relates an online account to the URL of that account. For example: UK Parliament having an account on X with the URL https://x.com/ukparliament."@en ;
	rdfs:domain pcp:OnlineAccount ;
	rdfs:range rdfs:Literal ;
	rdfs:isDefinedBy <http://parliament.uk/ontologies/contact-point/> .
	
pcp:address rdf:type owl:DatatypeProperty ;
	rdfs:label "Address"@en ;
	rdfs:comment "Relates a postal address to the part of its address before its postcode. For example: '35-39 Market Street, Chorley'."@en ;
	rdfs:domain pcp:PostalAddress ;
	rdfs:range rdf:langString ;
	rdfs:isDefinedBy <http://parliament.uk/ontologies/contact-point/> .

pcp:postcode rdf:type owl:DatatypeProperty ;
	rdfs:label "Postcode"@en ;
	rdfs:comment "Relates a postal address to its postcode, for example: 'PR7 2SW'."@en ;
	rdfs:domain pcp:PostalAddress ;
	rdfs:range rdfs:Literal ;	
	rdfs:isDefinedBy <http://parliament.uk/ontologies/contact-point/> .

pcp:faxNumber rdf:type owl:DatatypeProperty ;
	rdfs:label "Fax number"@en ;
	rdfs:comment "Relates a contact point to its fax number."@en ;
	rdfs:domain pcp:ContactPoint ;
	rdfs:range rdfs:Literal ;
	rdfs:isDefinedBy <http://parliament.uk/ontologies/contact-point/> .
	
pcp:phoneNumber rdf:type owl:DatatypeProperty ;
	rdfs:label "Phone number"@en ;
	rdfs:comment "Relates a contact point to its phone number, for example: '01257 271555'."@en ;
	rdfs:domain pcp:ContactPoint ;
	rdfs:range rdfs:Literal ;
	rdfs:isDefinedBy <http://parliament.uk/ontologies/contact-point/> .
	
pcp:emailAddress rdf:type owl:DatatypeProperty ;
	rdfs:label "Email address"@en ;
	rdfs:comment "Relates a contact point to its email address, for example: 'lindsay.hoyle.mp@parliament.uk'."@en ;
	rdfs:domain pcp:ContactPoint ;
	rdfs:range rdfs:Literal ;
	rdfs:isDefinedBy <http://parliament.uk/ontologies/contact-point/> .
	
pcp:homepageURL rdf:type owl:DatatypeProperty ;
	rdfs:label "Homepage URL"@en ;
	rdfs:comment "Relates a contact point to an online homepage."@en ;
	rdfs:domain pcp:ContactPoint ;
	rdfs:range rdfs:Literal ;
	rdfs:isDefinedBy <http://parliament.uk/ontologies/contact-point/> .

pcp:contactFormURL rdf:type owl:DatatypeProperty ;
	rdfs:label "Contact form URL"@en ;
	rdfs:comment "Relates a contact point to the URL of a contact form."@en ;
	rdfs:domain pcp:ContactPoint ;
	rdfs:range rdfs:Literal ;
	rdfs:isDefinedBy <http://parliament.uk/ontologies/contact-point/> .
	
pcp:availabilityNote rdf:type owl:DatatypeProperty ;
	rdfs:label "Availability note"@en ;
	rdfs:comment "Relates a contact point to a note describing the availability of the contactable thing at that contact point. For example: a constituency office being contactable in working hours only."@en ;
	rdfs:domain pcp:ContactPoint ;
	rdfs:range rdf:langString ;
	rdfs:isDefinedBy <http://parliament.uk/ontologies/contact-point/> .