@prefix pe: <http://parliament.uk/ontologies/election/> .
@prefix xsd: <http://www.w3.org/2001/XMLSchema#> .
@prefix rdf: <http://www.w3.org/1999/02/22-rdf-syntax-ns#> .
@prefix dcterms: <http://purl.org/dc/terms/> .
@prefix owl:     <http://www.w3.org/2002/07/owl#> .
@prefix rdfs:    <http://www.w3.org/2000/01/rdf-schema#> .
@prefix foaf:	<http://xmlns.com/foaf/0.1/> .

<http://parliament.uk/ontologies/election/>
    rdf:type owl:Ontology ;
    dcterms:title "Election ontology"@en ;
    dcterms:created "2016-10-06"^^xsd:date ;
	dcterms:rights "Open Parliament Licence v3.0"@en ;
    dcterms:description "A model describing elections, for example: general elections, by-elections to the House of Commons, by-elections of excepted hereditary peers in the House of Lords and elections to positions including that of the Speaker of the House of Commons. The model describes the result of an election regardless of the process by which that election has been conducted, and covers election returns by the 'first past the post' system and those which follow other methods. Where applicable, the model is aligned with the Cabinet Office Election Result Data Standard."@en ;
	foaf:depiction  <https://ukparliament.github.io/ontologies/election/election.svg> ;
	foaf:maker
		[ foaf:name "Anna Buck" ],
		[ foaf:name "Robert Brook"; foaf:homepage <https://robert-brook.com/> ],
		[ foaf:name "Carl Baker" ],
		[ foaf:name "Emily Davis" ],
		[ foaf:name "Oli Hawkins"; foaf:homepage <https://olihawkins.com/> ],
		[ foaf:name "Neil Johnston" ],
		[ foaf:name "Ned Morrell" ],
		[ foaf:name "Sym Roe"; foaf:homepage <http://symroe.co.uk/> ],
		[ foaf:name "Michael Smethurst"; foaf:homepage <http://smethur.st/> ],
	    [ foaf:name "Anya Somerville" ].
	


#######  Classes #####

pe:Country rdf:type owl:Class ;
	rdfs:label "Country"@en ;
	rdfs:comment "A country, for example: Great Britain, England and Wales, Scotland, Ireland and Northern Ireland."@en ;
	rdfs:isDefinedBy <http://parliament.uk/ontologies/election/> .

pe:PoliticalPartyRegistration rdf:type owl:Class ;
	rdfs:label "Political party registration"@en ;
	rdfs:comment "The registration of a political party in a country by the Electoral Commission."@en ;
	rdfs:isDefinedBy <http://parliament.uk/ontologies/election/> .
	
pe:PoliticalParty rdf:type owl:Class ;
	rdfs:label "Political party"@en ;
	rdfs:comment "An organisation registered by the Electoral Commission as a political party."@en ;
	rdfs:isDefinedBy <http://parliament.uk/ontologies/election/> .
	
pe:Certification rdf:type owl:Class ;
	rdfs:label "Certification"@en ;
	rdfs:comment "A certification of a candidate by a political party to stand in an election on behalf of that party. A candidate may be certified by more than one party at one time, for example: by both the Labour party and the Co-operative Party."@en ;
	rdfs:isDefinedBy <http://parliament.uk/ontologies/election/> .
	
pe:Candidacy rdf:type owl:Class ;
	rdfs:label "Candidacy"@en ;
	rdfs:comment "A candidacy of a person standing in an election, for example: the candidacy of Philip Hammond standing as the Conservative Party candidate in Runnymede and Weybridge, at the 2015 General Election."@en ;
	rdfs:isDefinedBy <http://parliament.uk/ontologies/election/> .
	
pe:Person rdf:type owl:Class ;
	rdfs:label "Person"@en ;
	rdfs:comment "A person."@en ;
	rdfs:isDefinedBy <http://parliament.uk/ontologies/election/> .
	
pe:CandidacyResult rdf:type owl:Class ;
	rdfs:label "Candidacy result"@en ;
	rdfs:comment "The result of a candidacy in an election, for example: the winning candidacy of Philip Hammond as the Conservative Party candidate in Runnymede and Weybridge, at the 2015 General Election."@en ;
	rdfs:isDefinedBy <http://parliament.uk/ontologies/election/> .
	
pe:WinningCandidacyResult rdf:type owl:Class ;
	rdfs:subClassOf pe:CandidacyResult ;
	rdfs:label "Winning candidacy result"@en ;
	rdfs:comment "Used to record the winning candidacy in an election."@en ;
	rdfs:isDefinedBy <http://parliament.uk/ontologies/election/> .
	
pe:Election rdf:type owl:Class ;
	rdfs:label "Election"@en ;
	rdfs:comment "An election to elect a person or persons to a seat or position."@en ;
	rdfs:isDefinedBy <http://parliament.uk/ontologies/election/> .

pe:ParliamentPeriod rdf:type owl:Class ;
	rdfs:label "Parliament period"@en ;
	rdfs:comment "The time period of a single Parliament between the date of its first assembly after a general election and its dissolution. A Parliament period contains contiguous session and prorogation periods. During a parliament period Parliament is either in session or prorogued. The start date of a Parliament may be changed by subsequent proclamations. A Parliament ends at the next dissolution. While the Fixed-term Parliaments Act 2011 was in force, the date of dissolution was determined by that Act or was named in a proclamation following a vote in Parliament for an early general election. The next Parliament began on the date named in the proclamation issued following a dissolution. Before the Fixed-term Parliaments Act 2011 came into force and after that Act was repealed by the Dissolution and Calling of Parliament Act 2022, the date of dissolution is fixed by proclamation. The dissolution proclamation also names the date for Parliament to reassemble. Parliament periods are the same across both Houses. Parliaments are numbered ordinally from the first Parliament of the United Kingdom, sitting in 1801."@en ;
	rdfs:isDefinedBy <http://parliament.uk/ontologies/election/> .
	
pe:GeneralElection rdf:type owl:Class ;
	rdfs:label "General election"@en ;
	rdfs:comment "A set of elections to the House of Commons, held concurrently in all constituencies."@en ;
	rdfs:isDefinedBy <http://parliament.uk/ontologies/election/> .
	
pe:GeneralElectionInBoundarySet rdf:type owl:Class ;
	rdfs:label "General election in boundary set"@en ;
	rdfs:comment "Provides a means to describe the ordinality of a general election in a boundary set, for example: the 2010 general election being the first general election to take place in the England boundary set established in April 2010 and the second general election to take place in the Scotland boundary set established in April 2005."@en ;
	rdfs:isDefinedBy <http://parliament.uk/ontologies/election/> .
	
pe:BoundarySet rdf:type owl:Class ;
	rdfs:label "Boundary set"@en ;
	rdfs:comment "A boundary set defining UK Parliament constituency areas, as proposed in a boundary review by the Boundary Commissions and established by statute."@en ;
	rdfs:isDefinedBy <http://parliament.uk/ontologies/election/> .
	
pe:Electorate rdf:type owl:Class ;
	rdfs:label "Electorate"@en ;
	rdfs:comment "A group of people eligible to vote in an election called at a particular time, for example: the group of people eligible to vote in an election to the House of Commons, or members of the House of Commons voting for their Speaker."@en ;
	rdfs:isDefinedBy <http://parliament.uk/ontologies/election/> .
	
pe:ConstituencyGroup rdf:type owl:Class ;
	rdfs:label "Constituency group"@en ;
	rdfs:comment "A group of people represented by an election winner."@en ;
	rdfs:isDefinedBy <http://parliament.uk/ontologies/election/> .
	
pe:ConstituencyArea rdf:type owl:Class ;
	rdfs:label "Constituency area"@en ;
	rdfs:comment "An area within which members of a constituency group are registered to vote. Constituency areas bounding constituency groups represented in the House of Commons are proposed in a boundary review by the Boundary Commissions and established by statute."@en ;
	rdfs:isDefinedBy <http://parliament.uk/ontologies/election/> .
	
pe:ConstituencyGroupSet rdf:type owl:Class ;
	rdfs:label "Constituency group set"@en ;
	rdfs:comment "A set of constituency groups, established by statute."@en ;
	rdfs:isDefinedBy <http://parliament.uk/ontologies/election/> .

pe:StatutoryThing rdf:type owl:Class ;
	rdfs:label "Statutory thing"@en ;
	rdfs:comment "A statutory thing, for example: an Act of Parliament or a made statutory instrument."@en ;
	rdfs:isDefinedBy <http://parliament.uk/ontologies/election/> .



#######  Object properties #####

pe:registrationIn rdf:type owl:ObjectProperty ;
	rdfs:label "Registration in"@en ;
	rdfs:comment "Relates a political party registration to the country the registration is in. A political party registration is in one country."@en ;
	rdfs:domain pe:PoliticalPartyRegistration ;
	rdfs:range pe:Country  ;
	rdfs:isDefinedBy <http://parliament.uk/ontologies/election/> .
	
pe:registrationOf rdf:type owl:ObjectProperty ;
	rdfs:label "Registration of"@en ;
	rdfs:comment "Relates a political party registration to the political party being registered. A political party registration is of one political party. A political party may have one or more political party registrations over time and in different countries."@en ;
	rdfs:domain pe:PoliticalPartyRegistration ;
	rdfs:range pe:PoliticalParty ;
	rdfs:isDefinedBy <http://parliament.uk/ontologies/election/> .
	
pe:issuedBy rdf:type owl:ObjectProperty ;
	rdfs:label "Issued by"@en ;
	rdfs:comment "Relates a certification of a candidacy to the political party issuing that certification. A certification is issued by one political party."@en ;
	rdfs:domain pe:Certification ;
	rdfs:range pe:PoliticalParty  ;
	rdfs:isDefinedBy <http://parliament.uk/ontologies/election/> .

pe:adjunctTo rdf:type owl:ObjectProperty ;
	rdfs:label "Adjunct to"@en ;
	rdfs:comment "Relates a certification of a candidacy to another certification of the same candidacy to which the first certification is adjunct, for example: relating a Co-operative Party certification to a certification by the Labour party."@en ;
	rdfs:domain pe:Certification ;
	rdfs:range pe:Certification  ;
	rdfs:isDefinedBy <http://parliament.uk/ontologies/election/> .

pe:certificationOf rdf:type owl:ObjectProperty ;
	rdfs:label "Certification of"@en ;
	rdfs:comment "Relates a certification by a political party to the candidacy being certified. A certification is of one candidacy. A candidacy has one or more certifications, or none."@en ;
	rdfs:domain pe:Certification ;
	rdfs:range pe:Candidacy ;
	rdfs:isDefinedBy <http://parliament.uk/ontologies/election/> .
	
pe:isOfPerson rdf:type owl:ObjectProperty ;
	rdfs:label "Is of person"@en ;
	rdfs:comment "Relates a candidacy to a person being a candidate. A candidacy is of one recorded person, or none."@en ;
	rdfs:domain pe:Candidacy ;
	rdfs:range pe:Person ;
	rdfs:isDefinedBy <http://parliament.uk/ontologies/election/> .
	
pe:hasCandidacyResult rdf:type owl:ObjectProperty ;
	rdfs:label "Has candidacy result"@en ;
	rdfs:comment "Relates a candidacy in an election to the result of that candidacy. A candidacy has one candidacy result. A candidacy result is for one candidacy."@en ;
	rdfs:domain pe:Candidacy ;
	rdfs:range pe:CandidacyResult ;
	rdfs:isDefinedBy <http://parliament.uk/ontologies/election/> .
	
pe:inElection rdf:type owl:ObjectProperty ;
	rdfs:label "In election"@en ;
	rdfs:comment "Relates a candidacy to the election that candidacy is in. A candidacy is in one election."@en ;
	rdfs:domain pe:Candidacy ;
	rdfs:range pe:Election ;
	rdfs:isDefinedBy <http://parliament.uk/ontologies/election/> .

pe:intoParliamentPeriod rdf:type owl:ObjectProperty ;
	rdfs:label "Into Parliament period"@en ;
	rdfs:comment "Relates an election to the House of Commons to the Parliament period within which any resulting incumbency takes place. An election to the House of Commons is related to one Parliament period."@en ;
	rdfs:domain pe:Election ;
	rdfs:range pe:ParliamentPeriod ;
	rdfs:isDefinedBy <http://parliament.uk/ontologies/election/> .
	
pe:forParliamentPeriod rdf:type owl:ObjectProperty ;
	rdfs:label "For Parliament period"@en ;
	rdfs:comment "Relates a general election to the Parliament period for which the general election is called. A general election is related to one Parliament period."@en ;
	rdfs:domain pe:GeneralElection ;
	rdfs:range pe:ParliamentPeriod ;
	rdfs:isDefinedBy <http://parliament.uk/ontologies/election/> .
	
pe:formsPartOfGeneralElection rdf:type owl:ObjectProperty ;
	rdfs:label "Forms part of general election"@en ;
	rdfs:comment "Relates a constituency election held as part of a general election to that general election. A constituency election is related to one general election, or none in the case of a by-election."@en ;
	rdfs:domain pe:Election ;
	rdfs:range pe:GeneralElection ;
	rdfs:isDefinedBy <http://parliament.uk/ontologies/election/> .
	
pe:forGeneralElection rdf:type owl:ObjectProperty ;
	rdfs:label "For general election"@en ;
	rdfs:comment "Relates a general election having ordinality in a boundary set to the general election having that ordinality."@en ;
	rdfs:domain pe:GeneralElectionInBoundarySet ;
	rdfs:range pe:GeneralElection  ;
	rdfs:isDefinedBy <http://parliament.uk/ontologies/election/> .
	
pe:inBoundarySet rdf:type owl:ObjectProperty ;
	rdfs:label "In boundary set"@en ;
	rdfs:comment "Relates a boundary set having general election ordinality to the boundary set."@en ;
	rdfs:domain pe:GeneralElectionInBoundarySet ;
	rdfs:range pe:BoundarySet  ;
	rdfs:isDefinedBy <http://parliament.uk/ontologies/election/> .

pe:forConstituencyGroup rdf:type owl:ObjectProperty ;
	rdfs:label "For constituency group"@en ;
	rdfs:comment "Relates an election to the constituency group represented by the winner of that election. An election is always for one constituency group."@en ;
	rdfs:domain pe:Election ;
	rdfs:range pe:ConstituencyGroup ;
	rdfs:isDefinedBy <http://parliament.uk/ontologies/election/> .

pe:hasElectorate rdf:type owl:ObjectProperty ;
	rdfs:label "Has electorate"@en ;
	rdfs:comment "Relates an election to the group of people eligible to vote in that election. An election has one electorate. The same group of people forming an electorate may be eligible to vote in one or more elections over time, or none."@en ;
	rdfs:domain pe:Election ;
	rdfs:range pe:Electorate ;
	rdfs:isDefinedBy <http://parliament.uk/ontologies/election/> .
	
pe:boundedBy rdf:type owl:ObjectProperty ;
	rdfs:label "Bounded by"@en ;
	rdfs:comment "Relates a constituency group to a geographic area. Some historical constituency groups had no defined geographical extent, for example: Oxford University. Since 1950, constituency groups represented in the House of Commons are within a constituency area. A new boundary set results in the creation of both a new constituency area and a new constituency group. A constituency group is bounded by one constituency area, or none. A constituency area bounds one constituency group."@en ;
	rdfs:domain pe:ConstituencyGroup ;
	rdfs:range pe:ConstituencyArea ;
	rdfs:isDefinedBy <http://parliament.uk/ontologies/election/> .
	
pe:formsPartOfConstituencyGroupSet rdf:type owl:ObjectProperty ;
	rdfs:label "Forms part of constituency group set"@en ;
	rdfs:comment "Relates a constituency group to the constituency group set of which it forms part. A constituency group forms part of one constituency group set."@en ;
	rdfs:domain pe:ConstituencyGroup ;
	rdfs:range pe:ConstituencyGroupSet ;
	rdfs:isDefinedBy <http://parliament.uk/ontologies/election/> .
	
pe:constituencyGroupSetInCountry rdf:type owl:ObjectProperty ;
	rdfs:label "Constituency group set in country"@en ;
	rdfs:comment "Relates a constituency group set to its country. A constituency group set is in one country. A country may have one or more constituency group sets over time."@en ;
	rdfs:domain pe:ConstituencyGroupSet ;
	rdfs:range pe:Country ;
	rdfs:isDefinedBy <http://parliament.uk/ontologies/election/> .
	
pe:establishedBy rdf:type owl:ObjectProperty ;
	rdfs:label "Established by"@en ;
	rdfs:comment "Relates a constituency group set to the statutory thing establishing that set. A constituency group set is established by one or more statutory things."@en ;
	rdfs:domain pe:ConstituencyGroupSet ;
	rdfs:range pe:StatutoryThing ;
	rdfs:isDefinedBy <http://parliament.uk/ontologies/election/> .



#######  Data properties #####

pe:registrationID rdf:type owl:DatatypeProperty ;
	rdfs:label "Registration ID"@en ;
	rdfs:comment "The ID of a political party registration. For example: 'PP103' being the registration ID of the Alliance party in Northern Ireland starting on 25 February 1999."@en ;
	rdfs:domain pe:PoliticalPartyRegistration ;
	rdfs:range rdfs:Literal ;
	rdfs:isDefinedBy <http://parliament.uk/ontologies/election/> .
	
pe:registeredPrimaryNameLastUpdatedOn rdf:type owl:DatatypeProperty ;
	rdfs:label "Registered primary name last updated on"@en ;
	rdfs:comment "The date on which the primary name of the political party as registered with the Electoral Commission was last updated."@en ;
	rdfs:domain pe:PoliticalPartyRegistration ;
	rdfs:range xsd:date ;
	rdfs:isDefinedBy <http://parliament.uk/ontologies/election/> .
	
pe:resultPosition rdf:type owl:DatatypeProperty ;
	rdfs:label "Result position"@en ;
	rdfs:comment "The ordinal position of the result of a candidacy in an election, for example: 1st or 2nd, recorded as 1 or 2."@en ;
	rdfs:domain pe:CandidacyResult ;
	rdfs:range xsd:integer ;
	rdfs:isDefinedBy <http://parliament.uk/ontologies/election/> .

pe:voteCount rdf:type owl:DatatypeProperty ;
	rdfs:label "Vote count"@en ;
	rdfs:comment "The number of valid votes recorded for a candidacy."@en ;
	rdfs:domain pe:CandidacyResult ;
	rdfs:range xsd:integer ;
	rdfs:isDefinedBy <http://parliament.uk/ontologies/election/> .

pe:voteShare rdf:type owl:DatatypeProperty ;
	rdfs:label "Vote share"@en ;
	rdfs:comment "The calculated share of a vote won in an election by a candidacy as a percentage of the total valid votes. For example: Alex Baker receiving approximately 40.7% of the vote in the constituency of Aldershot in the 2019 general election."@en ;
	rdfs:domain pe:CandidacyResult ;
	rdfs:range xsd:decimal ;
	rdfs:isDefinedBy <http://parliament.uk/ontologies/election/> .
	
pe:voteChange rdf:type owl:DatatypeProperty ;
	rdfs:label "Vote change"@en ;
	rdfs:comment "The change in the vote share recorded for a candidacy in an election compared to the vote share for a candidacy in the same constituency at the previous general election, the previous candidacy either being certified by the same party - discounting any adjunct certification - or being of a candidate standing for re-election as the House of Commons Speaker, or being of the same person standing for re-election as an independent. The calculation of vote change does not take account of intervening by-elections. Where a constituency's boundary has changed since the last general election, the vote change figure is based on notional results, being projected results of the previous general election if that election had taken place according to new boundaries."@en ;
	rdfs:domain pe:CandidacyResult ;
	rdfs:range xsd:decimal ;
	rdfs:isDefinedBy <http://parliament.uk/ontologies/election/> .
	
pe:candidateGivenName rdf:type owl:DatatypeProperty ;
	rdfs:label "Candidate given name"@en ;
	rdfs:comment "The given name of the candidate as it appears on the ballot, for example: 'John' in 'John Smith'."@en ;
	rdfs:domain pe:Candidacy ;
	rdfs:range rdf:langString ;
	rdfs:isDefinedBy <http://parliament.uk/ontologies/election/> .

pe:candidateFamilyName rdf:type owl:DatatypeProperty ;
	rdfs:label "Candidate family name"@en ;
	rdfs:comment "The family name of the candidate as it appears on the ballot, for example: 'Smith' in 'John Smith'."@en ;
	rdfs:domain pe:Candidacy ;
	rdfs:range rdf:langString ;
	rdfs:isDefinedBy <http://parliament.uk/ontologies/election/> .
	
pe:asCommonsSpeaker rdf:type owl:DatatypeProperty ;
	rdfs:label "As Commons Speaker"@en ;
	rdfs:comment "Used to record if the candidacy is of the House of Commons Speaker standing for re-election to the House of Commons."@en ;
	rdfs:domain pe:Candidacy ;
	rdfs:range xsd:boolean ;
	rdfs:isDefinedBy <http://parliament.uk/ontologies/election/> .
	
pe:asIndependent rdf:type owl:DatatypeProperty ;
	rdfs:label "As independent"@en ;
	rdfs:comment "Used to record if the candidacy is of a person standing as an independent, not being certified by any political party."@en ;
	rdfs:domain pe:Candidacy ;
	rdfs:range xsd:boolean ;
	rdfs:isDefinedBy <http://parliament.uk/ontologies/election/> .
	
pe:isNotional rdf:type owl:DatatypeProperty ;
	rdfs:label "Is notional"@en ;
	rdfs:comment "Used to record if the results of a general election are notional. When a general election is contested on a new boundary set or boundary sets, notional results are calculated for the changed constituencies. Notional results are calculated as if the previous general election had been contested on the new boundaries. Notional winner and notional vote share are used to derive the party gain / hold and change in vote share information, respectively, at the subsequent general election."@en ;
	rdfs:domain pe:GeneralElection ;
	rdfs:range xsd:boolean ;
	rdfs:isDefinedBy <http://parliament.uk/ontologies/election/> .

pe:generalElectionPollingOn rdf:type owl:DatatypeProperty ;
	rdfs:label "General election polling on"@en ;
	rdfs:comment "The date on which polling takes place for all elections forming part of a general election."@en ;
	rdfs:domain pe:GeneralElection ;
	rdfs:range xsd:date ;
	rdfs:isDefinedBy <http://parliament.uk/ontologies/election/> .

pe:ordinality rdf:type owl:DatatypeProperty ;
	rdfs:label "Ordinality"@en ;
	rdfs:comment "The ordinality of a general election in a boundary set. For example: the 2010 general election is the first general election in the England boundary set established in April 2010, and the second general election in the Scotland boundary set established in April 2005."@en ;
	rdfs:domain pe:GeneralElectionInBoundarySet ;
	rdfs:range xsd:integer ;
	rdfs:isDefinedBy <http://parliament.uk/ontologies/election/> .

pe:electionPollingOn rdf:type owl:DatatypeProperty ;
	rdfs:label "Election polling on"@en ;
	rdfs:comment "The date on which polling takes place for an election."@en ;
	rdfs:domain pe:Election ;
	rdfs:range xsd:date ;
	rdfs:isDefinedBy <http://parliament.uk/ontologies/election/> .

pe:resultSummary rdf:type owl:DatatypeProperty ;
	rdfs:label "Result summary"@en ;
	rdfs:comment "Text summarising the result of an election in terms of a candidacy gaining or holding a constituency relative to a candidacy at the previous general election, the previous candidacy either being certified by the same party - discounting any adjunct certification, for example: 'Conservative gain from Labour Co-operative'; or being of a candidate standing for re-election as the House of Commons Speaker, for example: 'Speaker hold'; or being of a candidate standing for election as an independent and gaining the seat, for example: 'Independent gain from Labour'; or being of a candidate being re-elected as an independent having won the constituency as an independent at the previous general election, for example: 'Independent hold'. The result summary does not take account of intervening by-elections. Where a constituency's boundary has changed since the most recent general election, the result summary is based on notional results, being projected results of the previous general election if that election had taken place according to new boundaries."@en ;
	rdfs:domain pe:Election ;
	rdfs:range rdf:langString ;
	rdfs:isDefinedBy <http://parliament.uk/ontologies/election/> .
	
pe:majority rdf:type owl:DatatypeProperty ;
	rdfs:label "Majority"@en ;
	rdfs:comment "The difference between the number of valid votes cast for the winning candidate and the number of valid votes cast for the second-placed candidate."@en ;
	rdfs:domain pe:Election ;
	rdfs:range xsd:integer ;
	rdfs:isDefinedBy <http://parliament.uk/ontologies/election/> .

pe:validVoteCount rdf:type owl:DatatypeProperty ;
	rdfs:label "Valid vote count"@en ;
	rdfs:comment "The number of votes cast in an election excluding any declared invalid by the Returning Officer."@en ;
	rdfs:domain pe:Election ;
	rdfs:range xsd:integer ;
	rdfs:isDefinedBy <http://parliament.uk/ontologies/election/> .

pe:invalidVoteCount rdf:type owl:DatatypeProperty ;
	rdfs:label "Invalid vote count"@en ;
	rdfs:comment "The number of invalid votes - also called spoiled ballots - cast by an electorate in an election, for example: ballots on which votes are given for more candidates than the voter is entitled to vote for, ballots on which anything is written or marked by which the voter can be identified, or ballots which are unmarked or where a mark does not sufficiently identify the vote. The number of invalid votes may be included in a calculation of turnout. Turnout as calculated by the House of Commons Library - and generally in academic usage - is the total number of valid votes cast, divided by the size of the electorate. Turnout as calculated by a Returning Officer is the total number of votes cast, divided by the size of the electorate."@en ;
	rdfs:domain pe:Election ;
	rdfs:range xsd:integer ;
	rdfs:isDefinedBy <http://parliament.uk/ontologies/election/> .

pe:round rdf:type owl:DatatypeProperty ;
	rdfs:label "Round"@en ;
	rdfs:comment "The ordinal position of the round in an election having more than one round of voting, for example: 1st or 2nd, recorded as 1 or 2."@en ;
	rdfs:domain pe:Election ;
	rdfs:range xsd:integer ;
	rdfs:isDefinedBy <http://parliament.uk/ontologies/election/> .

pe:declarationTime rdf:type owl:DatatypeProperty ;
	rdfs:label "Declaration time"@en ;
	rdfs:comment "The date and time at which results were declared for an election, for example: the date and time of the declaration of the results in a constituency election, by the Returning Officer."@en ;
	rdfs:domain pe:Election ;
	rdfs:range xsd:dateTime ;
	rdfs:isDefinedBy <http://parliament.uk/ontologies/election/> .
	
pe:recordedSize rdf:type owl:DatatypeProperty ;
	rdfs:label "Recorded size"@en ;
	rdfs:comment "The number of people forming an electorate."@en ;
	rdfs:domain pe:Electorate ;
	rdfs:range xsd:integer ;
	rdfs:isDefinedBy <http://parliament.uk/ontologies/election/> .

pe:recordedOn rdf:type owl:DatatypeProperty ;
	rdfs:label "Recorded on"@en ;
	rdfs:comment "The date on which the size of an electorate was recorded."@en ;
	rdfs:domain pe:Electorate ;
	rdfs:range xsd:date ;
	rdfs:isDefinedBy <http://parliament.uk/ontologies/election/> .