@prefix ppr: <https://parliament.uk/ontologies/procedure/> . 
@prefix xsd: <http://www.w3.org/2001/XMLSchema#> . 
@prefix rdf: <http://www.w3.org/1999/02/22-rdf-syntax-ns#> .
@prefix dcterms: <http://purl.org/dc/terms/> .
@prefix owl:     <http://www.w3.org/2002/07/owl#> .
@prefix rdfs:    <http://www.w3.org/2000/01/rdf-schema#> .

<https://parliament.uk/ontologies/procedure/> 
    rdf:type owl:Ontology ;
    dcterms:title "Procedure ontology"@en ;
    dcterms:created "20/02/2018"^^xsd:date ;
	dcterms:rights "Open Parliament Licence v3.0"@en ;
    dcterms:description "Procedure ontology for UK Parliament. An abstract ontology for describing how process steps or stages can be combined into a procedure."@en .


#######  Classes #####

ppr:Step rdf:type owl:Class ;
	rdfs:label "Step"@en ;
	rdfs:comment "A step in a procedure e.g. consideration of a statutory instrument by the Joint Committee on Statutory Instruments. Steps may not be unique to a specific procedure e.g. the consideration described in the previous example happens in both the affirmative and negative statutory instrument procedure."@en ;
	rdf:isDefinedBy <https://parliament.uk/ontologies/procedure/> .
	
ppr:Route rdf:type owl:Class ;
	rdfs:label "Route"@en ;
	rdfs:comment "Ties a procedural step or steps to the subsequent step, according to the RouteType. Note that routes are time bound (borrowing startOn and endOn from the Core Ontology). This allows routes to change over time and adapt to changes in procedure. A route is activated once the business item(s) which actualise the preceding steps are completed. This can be taken to mean the step is 'completed'. Note that the RouteType 'precludes' can route a completed step to the same step. This has the effect of precluding any more instances of that step in the procedure e.g. in the made affirmative statutory instrument procedure the step 'cleared by the Joint Committee on Statutory Instruments' can happen only once. In other words, the actualisation of this step as a business item precludes any other instance of that step."@en ;
	rdf:isDefinedBy <https://parliament.uk/ontologies/procedure/> .
	
ppr:RouteType rdf:type owl:Class ;
	rdfs:label "RouteType"@en ;
	rdfs:comment "Route types are: causes, allows and precludes. A route of type 'causes' relates the route to a following step where completion of the preceding step(s) directly causes the route to trigger the next step i.e. the next step is inevitable. A route of type 'allows' relates the route to a following step where completion of the preceding step(s) allows the next step to happen, but does not cause it to happen i.e. the next step might happen but is not inevitable. A route of type 'precludes' relates a route to a step where completion of the preceding step(s) precludes that step from happening i.e. the next step can no longer happen."@en ;
	rdf:isDefinedBy <https://parliament.uk/ontologies/procedure/> .
	
ppr:House rdf:type owl:Class ;
	rdfs:label "House"@en ;
	rdfs:comment "A parliamentary House e.g. the House of Lords."@en ;
	rdf:isDefinedBy <https://parliament.uk/ontologies/procedure/> .
	
ppr:Procedure rdf:type owl:Class ;
	rdfs:label "Procedure"@en ;
	rdfs:comment "A parliamentary procedure in a particular House or Houses. An example might be the passage of a made affirmative statutory instrument in both Houses. Note that some procedures are House specific, but can involve things like a joint committee that cuts across the two Houses. In the latter case we consider it to be a single procedure."@en ;
	rdf:isDefinedBy <https://parliament.uk/ontologies/procedure/> .
	
ppr:BusinessItem rdf:type owl:Class ;
	rdfs:label "BusinessItem"@en ;
	rdfs:comment "An item of parliamentary business."@en ;
	rdf:isDefinedBy <https://parliament.uk/ontologies/procedure/> .
	
ppr:BusinessItem rdf:type owl:Class ;
	rdfs:label "BusinessItem"@en ;
	rdfs:comment "An item of parliamentary business. The business item might be scheduled for a time and place via a calendar business item (e.g. a second reading debate), or it might not yet be scheduled (e.g. an early day motion), or it might be an item of business that is never scheduled (e.g. a written question)."@en ;
	rdf:isDefinedBy <https://parliament.uk/ontologies/procedure/> .
	
ppr:CalendarBusinessItem rdf:type owl:Class ;
	rdfs:label "CalendarBusinessItem"@en ;
	rdfs:comment "Handles the scheduling of a parliamentary business item once it has been timetabled into a calendar. The calendar business item only handles the timetabling of day, time and location and does not describe the nature of the business item."@en ;
	rdf:isDefinedBy <https://parliament.uk/ontologies/procedure/> .
	
ppr:WorkPackage rdf:type owl:Class ;
	rdfs:label "WorkPackage"@en ;
	rdfs:comment "A package of work grouping together many individual business items e.g. the passage of a specific statutory instrument, or the passage of a specific public bill etc. Whereas a procedure (and its accompanying routes and steps) describes the process, the work package handles the application of that process for a specific instance."@en ;
	rdf:isDefinedBy <https://parliament.uk/ontologies/procedure/> .
	
#######  Object properties ##### 

ppr:belongsTo rdf:type owl:ObjectProperty ;
	rdfs:label "belongsTo"@en ;
	rdfs:comment "Relates an individual business item to the work package it is part of. Note that whilst a work package can contain many business items, a business item might relate to several work packages e.g. a meeting of the Joint Committee on Statutory Instruments might include business relating to many SI work packages with no distinct segmentation."@en ;
	rdfs:domain ppr:BusinessItem ;
	rdfs:range ppr:WorkPackage ;
	rdf:isDefinedBy <https://parliament.uk/ontologies/procedure/> .
	
ppr:calendarises rdf:type owl:ObjectProperty ;
	rdfs:label "calendarises"@en ;
	rdfs:comment "Relates a calendar business item to a business item. Note that an individual business item can be calendarised into multiple calendar business items e.g. a second reading of a Bill might take place over several days."@en ;
	rdfs:domain ppr:CalendarBusinessItem ;
	rdfs:range ppr:BusinessItem ;
	rdf:isDefinedBy <https://parliament.uk/ontologies/procedure/> .
	
ppr:subjectTo rdf:type owl:ObjectProperty ;
	rdfs:label "subjectTo"@en ;
	rdfs:comment "Relates a work package to the procedure it is subject to. A work package can only be subject to one procedure."@en ;
	rdfs:domain ppr:WorkPackage ;
	rdfs:range ppr:Procedure ;
	rdf:isDefinedBy <https://parliament.uk/ontologies/procedure/> .
	
ppr:actualises rdf:type owl:ObjectProperty ;
	rdfs:label "actualises"@en ;
	rdfs:comment "Relates a business item to a step in a procedure (via a route) e.g. relates the second reading of a specific public bill to the corresponding (conceptual) step in the procedure. Note that whilst a step might be actualised by several business items (in different work packages), a business item might actualise one or several steps e.g. there might be a calendarised business item on the order paper that includes a debate on a number of motions. This would actualise steps relating each of those motions."@en ;
	rdfs:domain ppr:BusinessItem ;
	rdfs:range ppr:Step ;
	rdf:isDefinedBy <https://parliament.uk/ontologies/procedure/> .

ppr:fromStep rdf:type owl:ObjectProperty ;
	rdfs:label "fromStep"@en ;
	rdfs:comment "Relates a route to a preceding step."@en ;
	rdfs:domain ppr:Route ;
	rdfs:range ppr:Step ;
	rdf:isDefinedBy <https://parliament.uk/ontologies/procedure/> .
	
ppr:toStep rdf:type owl:ObjectProperty ;
	rdfs:label "toStep"@en ;
	rdfs:comment "Relates a route to a potential following step. Note that the 'next' step might be precluded by the route type."@en ;
	rdfs:domain ppr:Route ;
	rdfs:range ppr:Step ;
	rdf:isDefinedBy <https://parliament.uk/ontologies/procedure/> .
	
ppr:hasRouteType rdf:type owl:ObjectProperty ;
	rdfs:label "hasRouteType"@en ;
	rdfs:comment "Relates a route to a route type. A route can have one only type."@en ;
	rdfs:domain ppr:Route ;
	rdfs:range ppr:RouteType ;
	rdf:isDefinedBy <https://parliament.uk/ontologies/procedure/> .
	
ppr:follows rdf:type owl:ObjectProperty ;
	rdfs:label "follows"@en ;
	rdfs:comment "Relates a procedure to a route. A route can belong to only one procedure."@en ;
	rdfs:domain ppr:Procedure ;
	rdfs:range ppr:Route ;
	rdf:isDefinedBy <https://parliament.uk/ontologies/procedure/> .
	
ppr:stepInHouse rdf:type owl:ObjectProperty ;
	rdfs:label "stepInHouse"@en ;
	rdfs:comment "Relates a step to one or both Houses."@en ;
	rdfs:domain ppr:Step ;
	rdfs:range ppr:House ;
	rdf:isDefinedBy <https://parliament.uk/ontologies/procedure/> .
		
ppr:procedureInHouse rdf:type owl:ObjectProperty ;
	rdfs:label "procedureInHouse"@en ;
	rdfs:comment "Relates a procedure to one or both Houses."@en ;
	rdfs:domain ppr:Procedure ;
	rdfs:range ppr:House ;
	rdf:isDefinedBy <https://parliament.uk/ontologies/procedure/> .