@prefix ppr: <http://parliament.uk/ontologies/procedure/> . 
@prefix xsd: <http://www.w3.org/2001/XMLSchema#> . 
@prefix rdf: <http://www.w3.org/1999/02/22-rdf-syntax-ns#> .
@prefix dcterms: <http://purl.org/dc/terms/> .
@prefix owl:     <http://www.w3.org/2002/07/owl#> .
@prefix rdfs:    <http://www.w3.org/2000/01/rdf-schema#> .
@prefix foaf:	<http://xmlns.com/foaf/0.1/> .

<http://parliament.uk/ontologies/procedure/> 
    rdf:type owl:Ontology ;
    dcterms:title "Procedure ontology"@en ;
    dcterms:created "2018-02-20"^^xsd:date ;
	dcterms:rights "Open Parliament Licence v3.0"@en ;
    dcterms:description "A process flow model used to describe parliamentary procedure as a set of steps connected by routes. A step is a waypoint in a process, a route is a direction between steps and a procedure is analogous to a map of all possible routes. The model also describes the package of work resulting from a bill or an instrument subject to a procedure."@en ;
	foaf:depiction <https://ukparliament.github.io/ontologies/procedure/procedure.svg> ;
	foaf:maker
		[ foaf:name "Chris Alcock" ],
		[ foaf:name "David Beamish" ],
		[ foaf:name "Robert Brook"; foaf:homepage <https://robert-brook.com/> ],
		[ foaf:name "Gordon Clarke" ],
		[ foaf:name "Jack Dent" ],
		[ foaf:name "Ayesha Khan" ],
		[ foaf:name "Samu Lang" ],
		[ foaf:name "Ned Morrell" ],
		[ foaf:name "Silver Oliver" ],
		[ foaf:name "Michael Smethurst"; foaf:homepage <http://smethur.st/> ],
	    [ foaf:name "Anya Somerville" ],
	    [ foaf:name "Dominic Stockbridge" ],
	    [ foaf:name "Jayne Bosworth" ],
		[ foaf:name "James Vinter" ],
		[ foaf:name "Jane White" ],
		[ foaf:name "Ben Woodhams" ].


#######  Classes #####

ppr:Event rdf:type owl:Class ;
	rdfs:label "Event"@en ;
	rdfs:comment "An event taking place inside or outside Parliament. For example: a second reading debate, the tabling of an early day motion, a laying of a paper or the making of a statutory instrument by a government minister."@en ;
	rdfs:isDefinedBy <http://parliament.uk/ontologies/procedure/> .

ppr:WorkPackage rdf:type owl:Class ;
	rdfs:label "Work package"@en ;
	rdfs:comment "A group of events occurring as part of a procedure or as determined by a committee, for example: business items considered during the passage of a Statutory Instrument or Public Bill, or during an inquiry by a Select Committee."@en ;
	rdfs:isDefinedBy <http://parliament.uk/ontologies/procedure/> .
	
ppr:ProceduralWorkPackage rdf:type owl:Class ;
	rdfs:subClassOf ppr:WorkPackage ;
	rdfs:label "Procedural work package"@en ;
	rdfs:comment "A group of events occurring as part of a procedure, for example: business items considered during the passage of a Statutory Instrument or Public Bill."@en ;
	rdfs:isDefinedBy <http://parliament.uk/ontologies/procedure/> .
	
ppr:PaperWork rdf:type owl:Class ;
	rdfs:label "Paper work"@en ;
	rdfs:comment "A paper as a single intellectual work, as defined in the Functional Requirements for Bibliographic Records specification."@en ;
	rdfs:isDefinedBy <http://parliament.uk/ontologies/procedure/> .
	
ppr:StepType rdf:type owl:Class ;
	rdfs:label "Step type"@en ;
	rdfs:comment "The type of a step being an event step, decision step, logical NOT step, logical AND step, logical OR step, arithmetic SUM step, arithmetic INCREMENT step, arithmetic EQUALS step, or summation step."@en ;
	rdfs:seeAlso <https://ukparliament.github.io/ontologies/procedure/maps/meta/design-notes/> ;
	rdfs:isDefinedBy <http://parliament.uk/ontologies/procedure/> .
	
ppr:Step rdf:type owl:Class ;
	rdfs:label "Step"@en ;
	rdfs:comment "A step having a type. Steps are joined by routes to form procedures. For example, within the SI procedures there exists a step named 'English Votes for English Laws (EVEL) consideration'. Steps may occur in more than one procedure. For example, all statutory instrument procedures include the EVEL consideration step by means of routes."@en ;
	rdfs:isDefinedBy <http://parliament.uk/ontologies/procedure/> .
	
ppr:EventStep rdf:type owl:Class ;
	rdfs:subClassOf ppr:Step ;
	rdfs:subClassOf ppr:CitingThing ;
	rdfs:label "Event step"@en ;
	rdfs:comment "A step of type event, being the abstract notion of an event happening inside or outside Parliament."@en ;
	rdfs:isDefinedBy <http://parliament.uk/ontologies/procedure/> .
	
ppr:CitingThing rdf:type owl:Class ;
	rdfs:label "Citing thing"@en ;
	rdfs:comment "A thing which may have a citation."@en ;
	rdfs:isDefinedBy <http://parliament.uk/ontologies/procedure/> .

ppr:Citation rdf:type owl:Class ;
	rdfs:label "Citation"@en ;
	rdfs:comment "A citation."@en ;
	rdfs:isDefinedBy <http://parliament.uk/ontologies/procedure/> .
	
ppr:CitedThingType rdf:type owl:Class ;
	rdfs:label "Cited thing type"@en ;
	rdfs:comment "The type of the thing being cited, for example: an Act of Parliament, a House of Commons public standing order or a Speaker's ruling."@en ;
	rdfs:isDefinedBy <http://parliament.uk/ontologies/procedure/> .
	
ppr:AvailableThing rdf:type owl:Class ;
	rdfs:subClassOf ppr:CitingThing ;
	rdfs:label "Available thing"@en ;
	rdfs:comment "A thing having periods of availability and unavailability."@en ;
	rdfs:isDefinedBy <http://parliament.uk/ontologies/procedure/> .
	
ppr:Availability rdf:type owl:Class ;
	rdfs:subClassOf ppr:CitingThing ;
	rdfs:label "Availability"@en ;
	rdfs:comment "The availability of a path - being a route or a clock - or a procedure over time. Availability may change as a result of a change to legislation, for example: the procedure for proposed negative statutory instruments laid under Section 8 of the European Union (Withdrawal) Act 2018 will remain open - as set out under the Act - until two years after completion day. The availability of a route may change as a result of a standing order being introduced, suspended or rescinded, for example: the standing orders setting out rules for English Votes for English Laws were first suspended, then rescinded. The availability of a route may change as a result of an order of a House in Parliament, for example: a formal proceeding may establish a new committee, creating a new route to a step for consideration by that committee. A thing, having been closed, may reopen."@en ;
	rdfs:isDefinedBy <http://parliament.uk/ontologies/procedure/> .

ppr:AvailabilityStatus rdf:type owl:Class ;
	rdfs:label "Availability status"@en ;
	rdfs:comment "The status of an availability, being either open or closed."@en ;
	rdfs:isDefinedBy <http://parliament.uk/ontologies/procedure/> .
	
ppr:Path rdf:type owl:Class ;
	rdfs:subClassOf ppr:AvailableThing ;
	rdfs:label "Path"@en ;
	rdfs:comment "A path is a link from one step to another step in a procedure."@en ;
	rdfs:isDefinedBy <http://parliament.uk/ontologies/procedure/> .
	
ppr:Route rdf:type owl:Class ;
	rdfs:subClassOf ppr:Path ;
	rdfs:label "Route"@en ;
	rdfs:comment "A path which may be traversed, taking inputs from event steps actualised by events in a work package, being processed by logical, arithmetic and decision steps, in order to determine the potential future states of all event steps in the procedure the work package is subject to."@en ;
	rdfs:isDefinedBy <http://parliament.uk/ontologies/procedure/> .

ppr:Clock rdf:type owl:Class ;
	rdfs:subClassOf ppr:Path ;
	rdfs:label "Clock"@en ;
	rdfs:comment "A clock sets out a number of days to be counted between a clock start step and a clock end step in a procedure. Within a work package, a clock is used to record the period of time between the date of the event actualising a clock start step and the date of the event actualising a clock end step. The period of time resulting from a clock is dependent on the start date of the clock, the day count of the clock and the calculation style. End dates of clocks in work packages currently before Parliament may change."@en ;
	rdfs:isDefinedBy <http://parliament.uk/ontologies/procedure/> .
	
ppr:Procedure rdf:type owl:Class ;
	rdfs:subClassOf ppr:AvailableThing ;
	rdfs:label "Procedure"@en ;
	rdfs:comment "A procedure in a legislature. For example, the passage of a made affirmative statutory instrument in both Houses. This procedure consists of business in a House, such as a division; business undertaken by both Houses jointly, such as consideration by a joint committee; processes applying to either House, such as a clock; and activities outside Parliament, such as the making of the statutory instrument."@en ;
	rdfs:isDefinedBy <http://parliament.uk/ontologies/procedure/> .
	
ppr:ProcedureCollection rdf:type owl:Class ;
	rdfs:label "Procedure collection"@en ;
	rdfs:comment "A collection of procedures, for example: the collection containing the Made Affirmative Remedial Order and Draft Affirmative Remedial Order procedures."@en ;
	rdfs:isDefinedBy <http://parliament.uk/ontologies/procedure/> .
	
ppr:CalculationStyle rdf:type owl:Class ;
	rdfs:label "Calculation style"@en ;
	rdfs:comment "A calculation style is used to record the form of a calculation based on the sitting days counted by a clock, for example: either House being sitting or adjourned for less than four days, both Houses sitting or being adjourned for less than four days, or the House of Commons sitting or being adjourned for less than four days. A calculation style may set out the definition of the first day to be counted."@en ;
	rdfs:seeAlso <https://api.parliament.uk/egg-timer/calculator/styles> ;
	rdfs:isDefinedBy <http://parliament.uk/ontologies/procedure/> .
	
	
							# edited to here
							
							
							
ppr:StepDisplayDepthInProcedure rdf:type owl:Class ;
	rdfs:label "Step display depth in procedure"@en ;
	rdfs:comment "The display depth of an event step in a procedure. An event or events may actualise two different steps in the same work package on the same day.
	
	
	
	Because we capture dates rather than times of events it is not possible to order events in a way that makes 'procedural sense', for example: we may show 'procedure concluded' before 'instrument approved'.
	
	
	
	
	This class records the display depth of each of those event steps, associating a number with each step in the procedure in order by the date of the business item, then by the display depth of the step in the procedure. Display depth in this context is not absolute across the procedure. The context of display depth is constrained to parts of a procedure map where procedure specifies that if X happens it must happen before Y but that Y may happen without X happening. A step with depth 8 may happen before a step with depth 7."@en ;
	rdfs:isDefinedBy <http://parliament.uk/ontologies/procedure/> .
	
	

	
ppr:Legislature rdf:type owl:Class ;
	rdfs:label "Legislature"@en ;
	rdfs:comment "A legislature, being either the UK Parliament or a devolved legislature."@en ;
	rdfs:isDefinedBy <http://parliament.uk/ontologies/procedure/> .
	
ppr:House rdf:type owl:Class ;
	rdfs:label "House"@en ;
	rdfs:comment "A parliamentary House, for example: the House of Lords."@en ;
	rdfs:isDefinedBy <http://parliament.uk/ontologies/procedure/> .
	
ppr:StepCollection rdf:type owl:Class ;
	rdfs:label "Step collection"@en ;
	rdfs:comment "A collection of steps. Step collections are used to collect steps of one type, for example: starting steps, concluding steps, website display steps, bill stage steps, or Member action steps. A step collection named 'Starting steps' collects steps which, when actualised in a work package, denote that that work package is considered to be started. A procedure may have one or more starting steps. A step collection named 'Concluding steps' collects steps which, when actualised in a work package, denote that that work package is considered to be concluded. A procedure may have one or more concluding steps. A step collection named 'Website visible steps' collects steps which are intended to be visible on a website work package page once actualised by a business item in that work package. A procedure may have one or more steps described as website visible. A step collection named 'Second reading', within the House of Commons, collects steps forming that stage in that House. A step collection named 'Member action steps' collects steps which are considered to be steps at which a Member is able to take an action. A procedure may have one or more steps considered to be Member action steps."@en ;
	rdfs:isDefinedBy <http://parliament.uk/ontologies/procedure/> .
	


#######  Object properties #####

ppr:formsPartOf rdf:type owl:ObjectProperty ;
	rdfs:label "Forms part of"@en ;
	rdfs:comment "Relates an event to the work package or work packages it forms part of. One or more events may form part of a work package. An event may form part of one or more work packages, for example: a meeting of the Joint Committee on Statutory Instruments may consider one or more SIs, each SI being the focus of a separate work package."@en ;
	rdfs:domain ppr:Event ;
	rdfs:range ppr:WorkPackage ;
	rdfs:isDefinedBy <http://parliament.uk/ontologies/procedure/> .

ppr:focus rdf:type owl:ObjectProperty ;
	rdfs:label "Focus"@en ;
	rdfs:comment "Relates a procedural work package to the focus of that work package, being a paper work. A procedural work package has focus on one paper work. A paper work may be the focus of one or more procedural work packages, or none."@en ;
	rdfs:domain ppr:ProceduralWorkPackage ;
	rdfs:range ppr:PaperWork ;
	rdfs:isDefinedBy <http://parliament.uk/ontologies/procedure/> .
	
ppr:actualises rdf:type owl:ObjectProperty ;
	rdfs:label "Actualises"@en ;
	rdfs:comment "Relates an event to the procedural step or steps being actualised. An event may actualise one or more steps, for example: the step for the putting of a question and the step for the outcome may be actualised by one event. A step may be actualised one or more times by events in separate work packages."@en ;
	rdfs:domain ppr:Event ;
	rdfs:range ppr:EventStep ;
	rdfs:isDefinedBy <http://parliament.uk/ontologies/procedure/> .

ppr:hasStepType rdf:type owl:ObjectProperty ;
	rdfs:label "Has step type"@en ;
	rdfs:comment "Relates a step to its type. A step may only be of one type. A step type may be related to one or more steps, or none."@en ;
	rdfs:domain ppr:Step ;
	rdfs:range ppr:StepType ;
	rdfs:isDefinedBy <http://parliament.uk/ontologies/procedure/> .

ppr:fromStep rdf:type owl:ObjectProperty ;
	rdfs:label "From step"@en ;
	rdfs:comment "Relates a path to its input step. A path is related to one input step."@en ;
	rdfs:domain ppr:Path ;
	rdfs:range ppr:Step ;
	rdfs:isDefinedBy <http://parliament.uk/ontologies/procedure/> .

ppr:toStep rdf:type owl:ObjectProperty ;
	rdfs:label "To step"@en ;
	rdfs:comment "Relates a path to its output step. A path is related to one output step."@en ;
	rdfs:domain ppr:Path ;
	rdfs:range ppr:Step ;
	rdfs:isDefinedBy <http://parliament.uk/ontologies/procedure/> .
	
ppr:cites rdf:type owl:ObjectProperty ;
	rdfs:label "Cites"@en ;
	rdfs:comment ""@en ;
	rdfs:domain ppr:CitingThing ;
	rdfs:range ppr:Citation ;
	rdfs:isDefinedBy <http://parliament.uk/ontologies/procedure/> .
	
ppr:hasCitedThingType rdf:type owl:ObjectProperty ;
	rdfs:label "Has cited thing type"@en ;
	rdfs:comment ""@en ;
	rdfs:domain ppr:Citation ;
	rdfs:range ppr:CitedThingType ;
	rdfs:isDefinedBy <http://parliament.uk/ontologies/procedure/> .
	
ppr:parentCitedThingType rdf:type owl:ObjectProperty ;
	rdfs:label "Parent cited thing type"@en ;
	rdfs:comment ""@en ;
	rdfs:domain ppr:CitationType ;
	rdfs:range ppr:CitationType ;
	rdfs:isDefinedBy <http://parliament.uk/ontologies/procedure/> .

ppr:availabilityOf rdf:type owl:ObjectProperty ;
	rdfs:label "Availability of"@en ;
	rdfs:comment "Relates a path to its availability over a period of time. A path may have a different availability at different times, but only one availability at any one time. Path with no defined availability are taken to be open."@en ;
	rdfs:domain ppr:Availability ;
	rdfs:range ppr:AvailableThing ;
	rdfs:isDefinedBy <http://parliament.uk/ontologies/procedure/> .
	
ppr:hasAvailabilityStatus rdf:type owl:ObjectProperty ;
	rdfs:label "Has availability status"@en ;
	rdfs:comment "Relates a route availability over a period of time to the status of that availability. A route availability has one route availability status."@en ;
	rdfs:domain ppr:Availability ;
	rdfs:range ppr:AvailabilityStatus ;
	rdfs:isDefinedBy <http://parliament.uk/ontologies/procedure/> .
	
ppr:inProcedure rdf:type owl:ObjectProperty ;
	rdfs:label "In procedure"@en ;
	rdfs:comment "Relates a path to the procedure that path appears in. A path appears in one procedure. A procedure may have one or more paths, or none. A procedure having a component procedure allows the paths in the 'child' procedure to be shared with the 'parent' procedure."@en ;
	rdfs:domain ppr:Path ;
	rdfs:range ppr:Procedure ;
	rdfs:isDefinedBy <http://parliament.uk/ontologies/procedure/> .

ppr:subjectTo rdf:type owl:ObjectProperty ;
	rdfs:label "Subject to"@en ;
	rdfs:comment "Relates a work package to the procedure it is subject to. A work package is only subject to one procedure."@en ;
	rdfs:domain ppr:ProceduralWorkPackage ;
	rdfs:range ppr:Procedure ;
	rdfs:isDefinedBy <http://parliament.uk/ontologies/procedure/> .

ppr:proceduralWorkPackageHasCalculationStyle rdf:type owl:ObjectProperty ;
	rdfs:label "Procedural work package has calculation style"@en ;
	rdfs:comment "Relates a procedural work package to the calculation style used by that work package. A procedural work package has one calculation style, or none. Where a work package has a calculation style, that style is one of the calculation styles applied to the procedure that the work package is subject to."@en ;
	rdfs:domain ppr:ProceduralWorkPackage ;
	rdfs:range ppr:CalculationStyle ;
	rdfs:isDefinedBy <http://parliament.uk/ontologies/procedure/> .
	
ppr:procedureHasCalculationStyle rdf:type owl:ObjectProperty ;
	rdfs:label "Procedure has calculation style"@en ;
	rdfs:comment "Relates a procedure to the calculation styles applicable for work packages subject to that procedure. A calculation style may apply to one or more procedures. A procedure may have one or more calculation styles, or none. For example, depending on enabling legislation: a made affirmative statutory instrument may count days when both Houses are sitting or adjourned for fewer than five days, when either House is sitting or adjourned for fewer than five days or when the House of Commons is sitting or adjourned for fewer than five days."@en ;
	rdfs:domain ppr:Procedure ;
	rdfs:range ppr:CalculationStyle ;
	rdfs:isDefinedBy <http://parliament.uk/ontologies/procedure/> .
	
ppr:componentOf rdf:type owl:ObjectProperty ;
	rdfs:label "Component of"@en ;
	rdfs:comment "Relates a procedure to another procedure. A procedure forming a component of another procedure has all the routes in the 'child' procedure appearing as routes in the 'parent' procedure. A procedure may be composed of one or more other procedures, or none. A procedure may be a component of one or more other procedures, or none. A procedure cannot be a component of itself."@en ;
	rdfs:domain ppr:Procedure ;
	rdfs:range ppr:Procedure ;
	rdfs:isDefinedBy <http://parliament.uk/ontologies/procedure/> .
	
ppr:partOf rdf:type owl:ObjectProperty ;
	rdfs:label "Part of"@en ;
	rdfs:comment "Relates a procedure to the procedure collection of which it forms part. For example: the Made Affirmative Remedial Order procedure forming part of the Remedial Order procedure collection. A procedure forms part of one or more collections, or none."@en ;
	rdfs:domain ppr:Procedure ;
	rdfs:range ppr:ProcedureCollection ;
	rdfs:isDefinedBy <http://parliament.uk/ontologies/procedure/> .
	
ppr:parentProcedureCollection rdf:type owl:ObjectProperty ;
	rdfs:label "Parent procedure collection"@en ;
	rdfs:comment "Relates a procedure collection to its parent procedure collection. A procedure collection has one parent procedure collection, or none."@en ;
	rdfs:domain ppr:ProcedureCollection ;
	rdfs:range ppr:ProcedureCollection ;
	rdfs:isDefinedBy <http://parliament.uk/ontologies/procedure/> .
	
ppr:forStep rdf:type owl:ObjectProperty ;
	rdfs:label "For step"@en ;
	rdfs:comment "Relates a step display depth in a procedure to a business step. A step display depth in a procedure is always related to one step. A step may have different step display depths in different procedures."@en ;
	rdfs:domain ppr:StepDisplayDepthInProcedure ;
	rdfs:range ppr:EventStep ;
	rdfs:isDefinedBy <http://parliament.uk/ontologies/procedure/> .

ppr:depthInProcedure rdf:type owl:ObjectProperty ;
	rdfs:label "Depth In procedure"@en ;
	rdfs:comment "Relates a step display depth in a procedure to that procedure. A step display depth in a procedure is always related to one procedure. A procedure may have more than one step display depth for individual steps."@en ;
	rdfs:domain ppr:StepDisplayDepthInProcedure ;
	rdfs:range ppr:Procedure ;
	rdfs:isDefinedBy <http://parliament.uk/ontologies/procedure/> .
	
ppr:stepInLegislature rdf:type owl:ObjectProperty ;
	rdfs:label "Step in legislature"@en ;
	rdfs:comment "Relates a step to the devolved legislature in which that step takes place, for example: a legislative consent motion being tabled in the Scottish Parliament."@en ;
	rdfs:domain ppr:EventStep ;
	rdfs:range ppr:Legislature ;
	rdfs:isDefinedBy <http://parliament.uk/ontologies/procedure/> .
	
ppr:stepInHouse rdf:type owl:ObjectProperty ;
	rdfs:label "Step in House"@en ;
	rdfs:comment "Relates a step to one or both Houses where such a relationship exists. A step may exist with no relationship to a House. For example, the making of a statutory instrument takes place outside of Parliament."@en ;
	rdfs:domain ppr:EventStep ;
	rdfs:range ppr:House ;
	rdfs:isDefinedBy <http://parliament.uk/ontologies/procedure/> .
	
ppr:inLegislature rdf:type owl:ObjectProperty ;
	rdfs:label "In legislature"@en ;
	rdfs:comment "Relates a House to the Legislature it forms part of. This is only used to relate the House of Commons and the House of Lords to the UK Parliament, devolved legislatures being unicameral."@en ;
	rdfs:domain ppr:House ;
	rdfs:range ppr:Legislature ;
	rdfs:isDefinedBy <http://parliament.uk/ontologies/procedure/> .
	
ppr:memberOf rdf:type owl:ObjectProperty ;
	rdfs:label "Member of"@en ;
	rdfs:comment "Relates a step to the step collection that step is a member of. A step may belong to one or more step collections, or none."@en ;
	rdfs:domain ppr:EventStep ;
	rdfs:range ppr:StepCollection ;
	rdfs:isDefinedBy <http://parliament.uk/ontologies/procedure/> .
	
ppr:parentStepCollection rdf:type owl:ObjectProperty ;
	rdfs:label "Parent step collection"@en ;
	rdfs:comment "Relates a step collection to its parent step collection. A step collection may have one parent step collection, or none."@en ;
	rdfs:domain ppr:StepCollection ;
	rdfs:range ppr:StepCollection ;
	rdfs:isDefinedBy <http://parliament.uk/ontologies/procedure/> .
	
ppr:stepCollectionInHouse rdf:type owl:ObjectProperty ;
	rdfs:label "Step collection in House"@en ;
	rdfs:comment "Relates a step collection to one House, or none. For example: a step collection named 'Second reading', related to the House of Commons, collects steps forming that stage of public bill procedure in that House. A House may have one or more step collections, or none."@en ;
	rdfs:domain ppr:StepCollection ;
	rdfs:range ppr:House ;
	rdfs:isDefinedBy <http://parliament.uk/ontologies/procedure/> .
	
ppr:stepCollectionInProcedure rdf:type owl:ObjectProperty ;
	rdfs:label "Step collection in procedure"@en ;
	rdfs:comment "Relates a step collection to a procedure. A step collection has one procedure, or none.  For example: a step collection named 'Second reading', related to the public bill procedure, collects steps forming that stage of public bill procedure.  A procedure may have one or more step collections, or none."@en ;
	rdfs:domain ppr:StepCollection ;
	rdfs:range ppr:Procedure ;
	rdfs:isDefinedBy <http://parliament.uk/ontologies/procedure/> .
	


#######  Data properties #####

ppr:isClockFrozen rdf:type owl:DatatypeProperty ;
	rdfs:label "Is clock frozen"@en ;
	rdfs:comment "Used to record whether the clocks in the procedure a work package is subject to are frozen. A work package marked as frozen will not have the dates of business items actualising clock end steps automatically updated when sitting days change. For example: the treaty procedure set out in the Constitutional Reform and Governance Act 2010 specifies no limitation on the length of any extension to objection period A. Should a Government minister choose to extend period A, dates on any business items actualising clock end steps cannot be automatically updated. The work package is marked as frozen and any changes to dates are manually updated."@en ;
	rdfs:domain ppr:ProceduralWorkPackage ;
	rdfs:range xsd:boolean ;
	rdfs:isDefinedBy <http://parliament.uk/ontologies/procedure/> .
	
ppr:workPackageDayCount rdf:type owl:DatatypeProperty ;
	rdfs:label "Work package day count"@en ;
	rdfs:comment "Relates a work package to the number of days of a type - as defined by the calculation style applied to the work package - to be counted by any clock in the procedure the work package is subject to. Where a work package day count is set, its value overrides the day counts set on clocks in the procedure that work package is subject to."@en ;
	rdfs:domain ppr:ProceduralWorkPackage ;
	rdfs:range xsd:integer ;
	rdfs:isDefinedBy <http://parliament.uk/ontologies/procedure/> .
	
ppr:dayCount rdf:type owl:DatatypeProperty ;
	rdfs:label "Day count"@en ;
	rdfs:comment "Relates a clock to the number of days of a type - as defined by the calculation style applied to the work package - to be counted by that clock. The day count of a clock may be overridden by the day count set on a work package. Clock day counts in the made affirmative procedure are not set, day counts being set on the work package."@en ;
	rdfs:domain ppr:Clock ;
	rdfs:range xsd:integer ;
	rdfs:isDefinedBy <http://parliament.uk/ontologies/procedure/> .
	
ppr:displayDepth rdf:type owl:DatatypeProperty ;
	rdfs:label "Display depth"@en ;
	rdfs:comment "Relates a step display depth in a procedure to the depth value of the step in that procedure. The depth value is stored as a float in order to allow for the insertion of new steps into a procedure without having to renumber existing steps, for example: 1, 1.12, 2, 3."@en ;
	rdfs:domain ppr:StepDisplayDepthInProcedure ;
	rdfs:range xsd:float ;
	rdfs:isDefinedBy <http://parliament.uk/ontologies/procedure/> .
