@prefix ppr: <http://parliament.uk/ontologies/procedure/> . 
@prefix xsd: <http://www.w3.org/2001/XMLSchema#> . 
@prefix rdf: <http://www.w3.org/1999/02/22-rdf-syntax-ns#> .
@prefix dcterms: <http://purl.org/dc/terms/> .
@prefix owl:     <http://www.w3.org/2002/07/owl#> .
@prefix rdfs:    <http://www.w3.org/2000/01/rdf-schema#> .
@prefix foaf:	<http://xmlns.com/foaf/0.1/> .

<http://parliament.uk/ontologies/procedure/> 
    rdf:type owl:Ontology ;
    dcterms:title "Procedure ontology"@en ;
    dcterms:created "2018-02-20"^^xsd:date ;
	dcterms:rights "Open Parliament Licence v3.0"@en ;
    dcterms:description "A process flow model used to describe parliamentary procedure as a set of steps connected by routes. A step is a waypoint in a process, a route is a direction between steps and a procedure is analogous to a map of all possible routes. The model also describes the package of work resulting from a bill or an instrument subject to a procedure."@en ;
	foaf:depiction <https://ukparliament.github.io/ontologies/procedure/procedure.svg> ;
	foaf:maker
		[ foaf:name "Chris Alcock" ],
		[ foaf:name "David Beamish" ],
		[ foaf:name "Robert Brook"; foaf:homepage <https://robert-brook.com/> ],
		[ foaf:name "Gordon Clarke" ],
		[ foaf:name "Jack Dent" ],
		[ foaf:name "Ayesha Khan" ],
		[ foaf:name "Samu Lang" ],
		[ foaf:name "Ned Morrell" ],
		[ foaf:name "Silver Oliver" ],
		[ foaf:name "Michael Smethurst"; foaf:homepage <http://smethur.st/> ],
	    [ foaf:name "Anya Somerville" ],
	    [ foaf:name "Dominic Stockbridge" ],
	    [ foaf:name "Jayne Bosworth" ],
		[ foaf:name "James Vinter" ],
		[ foaf:name "Jane White" ],
		[ foaf:name "Ben Woodhams" ].


#######  Classes #####

ppr:Event rdf:type owl:Class ;
	rdfs:label "Event"@en ;
	rdfs:comment "An event taking place inside or outside Parliament. For example: a second reading debate, the tabling of an early day motion, a laying of a paper or the making of a statutory instrument by a government minister."@en ;
	rdfs:isDefinedBy <http://parliament.uk/ontologies/procedure/> .
	
ppr:BusinessItem rdf:type owl:Class ;
	rdfs:label "Business item"@en ;
	rdfs:comment "An item of business forming part of a work package, for example: the consideration of an instrument by a Delegated Legislation Committee taking place as part of a meeting of that committee."@en ;
	rdfs:isDefinedBy <http://parliament.uk/ontologies/procedure/> .
	
ppr:WorkPackage rdf:type owl:Class ;
	rdfs:label "Work package"@en ;
	rdfs:comment "A group of events occurring as part of a procedure or as determined by a committee, for example: business items considered during the passage of a Statutory Instrument or Public Bill, or during an inquiry by a Select Committee."@en ;
	rdfs:isDefinedBy <http://parliament.uk/ontologies/procedure/> .
	
ppr:ProceduralWorkPackage rdf:type owl:Class ;
	rdfs:subClassOf ppr:WorkPackage ;
	rdfs:label "Procedural work package"@en ;
	rdfs:comment "A group of events occurring as part of a procedure, for example: business items considered during the passage of a Statutory Instrument or Public Bill."@en ;
	rdfs:isDefinedBy <http://parliament.uk/ontologies/procedure/> .
	
ppr:PaperWork rdf:type owl:Class ;
	rdfs:label "Paper work"@en ;
	rdfs:comment "A paper as a single intellectual work, as defined in the Functional Requirements for Bibliographic Records specification."@en ;
	rdfs:isDefinedBy <http://parliament.uk/ontologies/procedure/> .
	
ppr:StepType rdf:type owl:Class ;
	rdfs:label "Step type"@en ;
	rdfs:comment "The type of a step being an event step, decision step, logical NOT step, logical AND step, logical OR step, arithmetic SUM step, arithmetic INCREMENT step, arithmetic EQUALS step, or summation step."@en ;
	rdfs:seeAlso <https://ukparliament.github.io/ontologies/procedure/maps/meta/design-notes/> ;
	rdfs:isDefinedBy <http://parliament.uk/ontologies/procedure/> .
	
ppr:Step rdf:type owl:Class ;
	rdfs:label "Step"@en ;
	rdfs:comment "A step having a type. Steps are joined by routes to form procedures. For example, within the SI procedures there exists a step named 'English Votes for English Laws (EVEL) consideration'. Steps may occur in more than one procedure. For example, all statutory instrument procedures include the EVEL consideration step by means of routes."@en ;
	rdfs:isDefinedBy <http://parliament.uk/ontologies/procedure/> .
	
ppr:BusinessStep rdf:type owl:Class ;
	rdfs:subClassOf ppr:Step ;
	rdfs:subClassOf ppr:CitingThing ;
	rdfs:label "Business step"@en ;
	rdfs:comment "A step of type business. A business step describes a set of potential business items, for example: the potential for papers to be laid before the House of Commons. Potential business items described by a business step may take place inside or outside Parliament."@en ;
	rdfs:isDefinedBy <http://parliament.uk/ontologies/procedure/> .
	
ppr:CitingThing rdf:type owl:Class ;
	rdfs:label "Citing thing"@en ;
	rdfs:comment "A thing which may have a citation."@en ;
	rdfs:isDefinedBy <http://parliament.uk/ontologies/procedure/> .

ppr:Citation rdf:type owl:Class ;
	rdfs:label "Citation"@en ;
	rdfs:comment "A citation."@en ;
	rdfs:isDefinedBy <http://parliament.uk/ontologies/procedure/> .
	
ppr:CitedThingType rdf:type owl:Class ;
	rdfs:label "Cited thing type"@en ;
	rdfs:comment "The type of the thing being cited, for example: an Act of Parliament, a House of Commons public standing order or a Speaker's ruling."@en ;
	rdfs:isDefinedBy <http://parliament.uk/ontologies/procedure/> .
	
ppr:AvailableThing rdf:type owl:Class ;
	rdfs:subClassOf ppr:CitingThing ;
	rdfs:label "Available thing"@en ;
	rdfs:comment "A thing having periods of availability and unavailability."@en ;
	rdfs:isDefinedBy <http://parliament.uk/ontologies/procedure/> .
	
ppr:Availability rdf:type owl:Class ;
	rdfs:subClassOf ppr:CitingThing ;
	rdfs:label "Availability"@en ;
	rdfs:comment "The availability of a path - being a route or a clock - or a procedure over time. Availability may change as a result of a change to legislation, for example: the procedure for proposed negative statutory instruments laid under Section 8 of the European Union (Withdrawal) Act 2018 will remain open - as set out under the Act - until two years after completion day. The availability of a route may change as a result of a standing order being introduced, suspended or rescinded, for example: the standing orders setting out rules for English Votes for English Laws were first suspended, then rescinded. The availability of a route may change as a result of an order of a House in Parliament, for example: a formal proceeding may establish a new committee, creating a new route to a step for consideration by that committee. A thing, having been closed, may reopen."@en ;
	rdfs:isDefinedBy <http://parliament.uk/ontologies/procedure/> .

ppr:AvailabilityStatus rdf:type owl:Class ;
	rdfs:label "Availability status"@en ;
	rdfs:comment "The status of an availability, being either open or closed."@en ;
	rdfs:isDefinedBy <http://parliament.uk/ontologies/procedure/> .
	
ppr:Path rdf:type owl:Class ;
	rdfs:subClassOf ppr:AvailableThing ;
	rdfs:label "Path"@en ;
	rdfs:comment "A path is a link from one step to another step in a procedure."@en ;
	rdfs:isDefinedBy <http://parliament.uk/ontologies/procedure/> .
	
ppr:Route rdf:type owl:Class ;
	rdfs:subClassOf ppr:Path ;
	rdfs:label "Route"@en ;
	rdfs:comment "A path which may be traversed, taking inputs from event steps actualised by events in a work package, being processed by logical, arithmetic and decision steps, in order to determine the potential future states of all event steps in the procedure the work package is subject to."@en ;
	rdfs:isDefinedBy <http://parliament.uk/ontologies/procedure/> .

ppr:Clock rdf:type owl:Class ;
	rdfs:subClassOf ppr:Path ;
	rdfs:label "Clock"@en ;
	rdfs:comment "A clock sets out a number of days to be counted between a clock start step and a clock end step in a procedure. Within a work package, a clock is used to record the period of time between the date of the event actualising a clock start step and the date of the event actualising a clock end step. The period of time resulting from a clock is dependent on the start date of the clock, the day count of the clock and the calculation style. End dates of clocks in work packages currently before Parliament may change."@en ;
	rdfs:isDefinedBy <http://parliament.uk/ontologies/procedure/> .
	
ppr:Procedure rdf:type owl:Class ;
	rdfs:subClassOf ppr:AvailableThing ;
	rdfs:label "Procedure"@en ;
	rdfs:comment "A procedure in a legislature. For example, the passage of a made affirmative statutory instrument in both Houses. This procedure consists of business in a House, such as a division; business undertaken by both Houses jointly, such as consideration by a joint committee; processes applying to either House, such as a clock; and activities outside Parliament, such as the making of the statutory instrument."@en ;
	rdfs:isDefinedBy <http://parliament.uk/ontologies/procedure/> .
	
ppr:ProcedureCollection rdf:type owl:Class ;
	rdfs:label "Procedure collection"@en ;
	rdfs:comment "A collection of procedures, for example: the collection containing the Made Affirmative Remedial Order and Draft Affirmative Remedial Order procedures."@en ;
	rdfs:isDefinedBy <http://parliament.uk/ontologies/procedure/> .
	
ppr:CalculationStyle rdf:type owl:Class ;
	rdfs:label "Calculation style"@en ;
	rdfs:comment "A calculation style is used to record the form of a calculation based on the sitting days counted by a clock, for example: either House being sitting or adjourned for less than four days, both Houses sitting or being adjourned for less than four days, or the House of Commons sitting or being adjourned for less than four days. A calculation style may set out the definition of the first day to be counted."@en ;
	rdfs:seeAlso <https://api.parliament.uk/egg-timer/calculator/styles> ;
	rdfs:isDefinedBy <http://parliament.uk/ontologies/procedure/> .
	
ppr:StepDisplayDepthInProcedure rdf:type owl:Class ;
	rdfs:label "Step display depth in procedure"@en ;
	rdfs:comment "The display depth of an event step in a procedure. An event or events may actualise two different steps in the same work package on the same day. Because we capture dates rather than times of events it was not possible to order events in a way that made 'procedural sense', for example: we may have shown 'Procedure concluded' before 'Instrument approved'. This class records the display depth of an event step forming part of the procedure, associating a display depth number with each step. For example: the 'Instrument created' event step in the draft affirmative procedure has a display depth of 1.0, whereas the 'Laid before the House of Commons' event step in the same procedure has a display depth of 3.1. These numbers are used to order events in a work package sharing the same date. The context of display depth is constrained to parts of a procedure map where procedure specifies that if X happens it must happen before Y but that Y may happen without X happening. An event step with depth 8 may happen before an event step with depth 7, if those two event steps are on different branches of the procedure map. An event step may have different step display depths in different procedures."@en ;
	rdfs:isDefinedBy <http://parliament.uk/ontologies/procedure/> .
	
ppr:Legislature rdf:type owl:Class ;
	rdfs:label "Legislature"@en ;
	rdfs:comment "A legislature, being either the UK Parliament or a devolved legislature."@en ;
	rdfs:isDefinedBy <http://parliament.uk/ontologies/procedure/> .
	
ppr:House rdf:type owl:Class ;
	rdfs:label "House"@en ;
	rdfs:comment "A parliamentary House, for example: the House of Lords."@en ;
	rdfs:isDefinedBy <http://parliament.uk/ontologies/procedure/> .
	
ppr:StepCollection rdf:type owl:Class ;
	rdfs:label "Step collection"@en ;
	rdfs:comment "A collection of steps. Step collections collect steps of one type, for example: starting steps, concluding steps, website display steps, bill stage steps, or Member action steps."@en ;
	rdfs:seeAlso <https://ukparliament.github.io/ontologies/procedure/maps/meta/design-notes/#step-collections> ;
	rdfs:isDefinedBy <http://parliament.uk/ontologies/procedure/> .



#######  Object properties #####

ppr:takesPlaceDuring rdf:type owl:ObjectProperty ;
	rdfs:label "Takes place during"@en ;
	rdfs:comment "Relates a business item to the event during which that business item takes place. A business item takes place during one event. An event may include one or more business items, or none. For example: a meeting of the Joint Committee on Statutory Instruments being one event during which the committee may consider one or more instruments, the consideration of each instrument being a business item in a work package."@en ;
	rdfs:domain ppr:BusinessItem ;
	rdfs:range ppr:Event ;
	rdfs:isDefinedBy <http://parliament.uk/ontologies/procedure/> .

ppr:formsPartOf rdf:type owl:ObjectProperty ;
	rdfs:label "Forms part of"@en ;
	rdfs:comment "Relates a business item to the work package it forms part of. One or more business items may form part of a work package. A business item forms part of one work package."@en ;
	rdfs:domain ppr:BusinessItem ;
	rdfs:range ppr:WorkPackage ;
	rdfs:isDefinedBy <http://parliament.uk/ontologies/procedure/> .

ppr:focus rdf:type owl:ObjectProperty ;
	rdfs:label "Focus"@en ;
	rdfs:comment "Relates a procedural work package to the focus of that work package, being a paper work. A procedural work package has focus on one paper work. A paper work may be the focus of one or more procedural work packages, or none."@en ;
	rdfs:domain ppr:ProceduralWorkPackage ;
	rdfs:range ppr:PaperWork ;
	rdfs:isDefinedBy <http://parliament.uk/ontologies/procedure/> .
	
ppr:actualises rdf:type owl:ObjectProperty ;
	rdfs:label "Actualises"@en ;
	rdfs:comment "Relates a business item to the business step or steps being actualised by that business item. A record of a business item forming part of a work package actualises the potential step described by the business step, procedurally indexing the business item with the concept embodied by the business step. For example: a business item recording the laying of a paper before the House of Commons in a work package actualises the business step 'Laid before the House of Commons', making that potential step actual. A business item may actualise one or more business steps, for example: the business step for the putting of a question and the business step for the outcome may be actualised by one business item. A business step may be actualised one or more times, or none."@en ;
	rdfs:domain ppr:BusinessItem ;
	rdfs:range ppr:BusinessStep ;
	rdfs:isDefinedBy <http://parliament.uk/ontologies/procedure/> .
	
ppr:hasStepType rdf:type owl:ObjectProperty ;
	rdfs:label "Has step type"@en ;
	rdfs:comment "Relates a step to its type. A step may only be of one type. A step type may be related to one or more steps, or none."@en ;
	rdfs:domain ppr:Step ;
	rdfs:range ppr:StepType ;
	rdfs:isDefinedBy <http://parliament.uk/ontologies/procedure/> .
	
ppr:fromStep rdf:type owl:ObjectProperty ;
	rdfs:label "From step"@en ;
	rdfs:comment "Relates a path to the step that path comes from. A path comes from one input step."@en ;
	rdfs:domain ppr:Path ;
	rdfs:range ppr:Step ;
	rdfs:isDefinedBy <http://parliament.uk/ontologies/procedure/> .
	
ppr:toStep rdf:type owl:ObjectProperty ;
	rdfs:label "To step"@en ;
	rdfs:comment "Relates a path to the step that path goes to. A path goes to one input step."@en ;
	rdfs:domain ppr:Path ;
	rdfs:range ppr:Step ;
	rdfs:isDefinedBy <http://parliament.uk/ontologies/procedure/> .
	
ppr:cites rdf:type owl:ObjectProperty ;
	rdfs:label "Cites"@en ;
	rdfs:comment "Relates a citing thing to its citation. A thing having a citation may have one or more citations, or none. A citation is always from one citing thing."@en ;
	rdfs:domain ppr:CitingThing ;
	rdfs:range ppr:Citation ;
	rdfs:isDefinedBy <http://parliament.uk/ontologies/procedure/> .
	
ppr:hasCitedThingType rdf:type owl:ObjectProperty ;
	rdfs:label "Has cited thing type"@en ;
	rdfs:comment "Relates a citation to the type of the thing being cited, for example: a citation of a section of an Act of Parliament having cited thing type 'Act of Parliament'. A citation has one cited thing type."@en ;
	rdfs:domain ppr:Citation ;
	rdfs:range ppr:CitedThingType ;
	rdfs:isDefinedBy <http://parliament.uk/ontologies/procedure/> .
	
ppr:parentCitedThingType rdf:type owl:ObjectProperty ;
	rdfs:label "Parent cited thing type"@en ;
	rdfs:comment "Relates a cited thing type to its parent cited thing type, for example: the cited thing type 'Act of Parliament' having parent cited thing type 'Primary legislation'. A cited thing type may have one or more parent cited thing types, or none."@en ;
	rdfs:domain ppr:CitedThingType ;
	rdfs:range ppr:CitedThingType ;
	rdfs:isDefinedBy <http://parliament.uk/ontologies/procedure/> .
	
ppr:availabilityOf rdf:type owl:ObjectProperty ;
	rdfs:label "Availability of"@en ;
	rdfs:comment "Relates an availability to the thing having that availability. A thing may have different availabilities at different times, but only one availability at any one time. An availability is always of one thing."@en ;
	rdfs:domain ppr:Availability ;
	rdfs:range ppr:AvailableThing ;
	rdfs:isDefinedBy <http://parliament.uk/ontologies/procedure/> .
	
ppr:hasAvailabilityStatus rdf:type owl:ObjectProperty ;
	rdfs:label "Has availability status"@en ;
	rdfs:comment "Relates an availability to its status. An availability has one type, being open or closed."@en ;
	rdfs:domain ppr:Availability ;
	rdfs:range ppr:AvailabilityStatus ;
	rdfs:isDefinedBy <http://parliament.uk/ontologies/procedure/> .
	
ppr:inProcedure rdf:type owl:ObjectProperty ;
	rdfs:label "In procedure"@en ;
	rdfs:comment "Relates a path to the procedure that path appears in. A path appears in one procedure. A procedure may have one or more paths, or none. A procedure having a component procedure allows the paths in that component procedure to be shared with the 'parent' procedure."@en ;
	rdfs:domain ppr:Path ;
	rdfs:range ppr:Procedure ;
	rdfs:isDefinedBy <http://parliament.uk/ontologies/procedure/> .
	
ppr:subjectTo rdf:type owl:ObjectProperty ;
	rdfs:label "Subject to"@en ;
	rdfs:comment "Relates a procedural work package to the procedure it is subject to. A procedural work package is subject to one procedure."@en ;
	rdfs:domain ppr:ProceduralWorkPackage ;
	rdfs:range ppr:Procedure ;
	rdfs:isDefinedBy <http://parliament.uk/ontologies/procedure/> .
	
ppr:proceduralWorkPackageHasCalculationStyle rdf:type owl:ObjectProperty ;
	rdfs:label "Procedural work package has calculation style"@en ;
	rdfs:comment "Relates a procedural work package to the calculation style used by that work package. A procedural work package has one calculation style, or none. Where a procedural work package has a calculation style, that style is one of the calculation styles applied to the procedure that the procedural work package is subject to."@en ;
	rdfs:domain ppr:ProceduralWorkPackage ;
	rdfs:range ppr:CalculationStyle ;
	rdfs:isDefinedBy <http://parliament.uk/ontologies/procedure/> .
	
ppr:procedureHasCalculationStyle rdf:type owl:ObjectProperty ;
	rdfs:label "Procedure has calculation style"@en ;
	rdfs:comment "Relates a procedure to the calculation styles applicable for work packages subject to that procedure. A calculation style may apply to one or more procedures. A procedure may have one or more calculation styles, or none. For example, depending on enabling legislation: a made affirmative statutory instrument may count days when both Houses are sitting or adjourned for fewer than five days, when either House is sitting or adjourned for fewer than five days or when the House of Commons is sitting or adjourned for fewer than five days."@en ;
	rdfs:domain ppr:Procedure ;
	rdfs:range ppr:CalculationStyle ;
	rdfs:isDefinedBy <http://parliament.uk/ontologies/procedure/> .
	
ppr:componentOf rdf:type owl:ObjectProperty ;
	rdfs:label "Component of"@en ;
	rdfs:comment "Relates a procedure to its 'parent' procedure. A procedure forming a component of another procedure has all the routes in the component procedure appearing as routes in the 'parent' procedure. A procedure may be composed of one or more component procedures, or none. A procedure may be a component of one or more other procedures, or none. A procedure cannot be a component of itself."@en ;
	rdfs:domain ppr:Procedure ;
	rdfs:range ppr:Procedure ;
	rdfs:isDefinedBy <http://parliament.uk/ontologies/procedure/> .
	
ppr:partOf rdf:type owl:ObjectProperty ;
	rdfs:label "Part of"@en ;
	rdfs:comment "Relates a procedure to the procedure collection of which it forms part. For example: the Made Affirmative Remedial Order procedure forming part of the Remedial Order procedure collection. A procedure forms part of one or more collections, or none."@en ;
	rdfs:domain ppr:Procedure ;
	rdfs:range ppr:ProcedureCollection ;
	rdfs:isDefinedBy <http://parliament.uk/ontologies/procedure/> .
	
ppr:parentProcedureCollection rdf:type owl:ObjectProperty ;
	rdfs:label "Parent procedure collection"@en ;
	rdfs:comment "Relates a procedure collection to its parent procedure collection. A procedure collection has one parent procedure collection, or none."@en ;
	rdfs:domain ppr:ProcedureCollection ;
	rdfs:range ppr:ProcedureCollection ;
	rdfs:isDefinedBy <http://parliament.uk/ontologies/procedure/> .
	
ppr:forBusinessStep rdf:type owl:ObjectProperty ;
	rdfs:label "For business step"@en ;
	rdfs:comment "Relates a step display depth in a procedure to a business step. A step display depth in a procedure is always related to one business step. A business step in a procedure has one step display depth, or none. A busines step may have different step display depths in different procedures."@en ;
	rdfs:domain ppr:StepDisplayDepthInProcedure ;
	rdfs:range ppr:BusinessStep ;
	rdfs:isDefinedBy <http://parliament.uk/ontologies/procedure/> .

ppr:depthInProcedure rdf:type owl:ObjectProperty ;
	rdfs:label "Depth In procedure"@en ;
	rdfs:comment "Relates a step display depth in a procedure to that procedure. A step display depth in a procedure is always related to one procedure. A procedure may have one or more step display depths, or none."@en ;
	rdfs:domain ppr:StepDisplayDepthInProcedure ;
	rdfs:range ppr:Procedure ;
	rdfs:isDefinedBy <http://parliament.uk/ontologies/procedure/> .
	
ppr:businessStepInLegislature rdf:type owl:ObjectProperty ;
	rdfs:label "Business step in legislature"@en ;
	rdfs:comment "Relates a business step to the legislature in which it is possible for that business step to take place, for example: a Scottish Parliament legislative consent motion which may be tabled in the Scottish Parliament. A business step may take place in one legislature, or none."@en ;
	rdfs:domain ppr:BusinessStep ;
	rdfs:range ppr:Legislature ;
	rdfs:isDefinedBy <http://parliament.uk/ontologies/procedure/> .
	
ppr:businessStepInHouse rdf:type owl:ObjectProperty ;
	rdfs:label "Business step in House"@en ;
	rdfs:comment "Relates a business step to the House in which it is possible for that business step to take place, for example: a motion to refer to a Delegated Legislation Committee which may be tabled in the House of Commons. A business step may take place in one or more Houses, or none."@en ;
	rdfs:domain ppr:BusinessStep ;
	rdfs:range ppr:House ;
	rdfs:isDefinedBy <http://parliament.uk/ontologies/procedure/> .
	
ppr:inLegislature rdf:type owl:ObjectProperty ;
	rdfs:label "In legislature"@en ;
	rdfs:comment "Relates a House to the Legislature it forms part of. This is only used to relate the House of Commons and the House of Lords to the UK Parliament, devolved legislatures being unicameral."@en ;
	rdfs:domain ppr:House ;
	rdfs:range ppr:Legislature ;
	rdfs:isDefinedBy <http://parliament.uk/ontologies/procedure/> .
	
ppr:memberOf rdf:type owl:ObjectProperty ;
	rdfs:label "Member of"@en ;
	rdfs:comment "Relates a business step to the step collection that business step is a member of. A business step may belong to one or more step collections, or none."@en ;
	rdfs:domain ppr:BusinessStep ;
	rdfs:range ppr:StepCollection ;
	rdfs:isDefinedBy <http://parliament.uk/ontologies/procedure/> .
	
ppr:parentStepCollection rdf:type owl:ObjectProperty ;
	rdfs:label "Parent step collection"@en ;
	rdfs:comment "Relates a step collection to its parent step collection. A step collection may have one parent step collection, or none."@en ;
	rdfs:domain ppr:StepCollection ;
	rdfs:range ppr:StepCollection ;
	rdfs:isDefinedBy <http://parliament.uk/ontologies/procedure/> .
	
ppr:stepCollectionInHouse rdf:type owl:ObjectProperty ;
	rdfs:label "Step collection in House"@en ;
	rdfs:comment "Relates a step collection to one House, or none. For example: a step collection named 'Second reading', related to the House of Commons, collects steps forming that stage of public bill procedure in that House. A House may have one or more step collections, or none."@en ;
	rdfs:domain ppr:StepCollection ;
	rdfs:range ppr:House ;
	rdfs:isDefinedBy <http://parliament.uk/ontologies/procedure/> .
	
ppr:stepCollectionInProcedure rdf:type owl:ObjectProperty ;
	rdfs:label "Step collection in procedure"@en ;
	rdfs:comment "Relates a step collection to a procedure. A step collection has one procedure, or none.  For example: a step collection named 'Second reading', related to the public bill procedure, collects steps forming that stage of public bill procedure.  A procedure may have one or more step collections, or none."@en ;
	rdfs:domain ppr:StepCollection ;
	rdfs:range ppr:Procedure ;
	rdfs:isDefinedBy <http://parliament.uk/ontologies/procedure/> .
	


#######  Data properties #####

ppr:isClockFrozen rdf:type owl:DatatypeProperty ;
	rdfs:label "Is clock frozen"@en ;
	rdfs:comment "Used to record whether the clocks in the procedure a work package is subject to are frozen. A work package marked as frozen will not have the dates of business items actualising clock end steps automatically updated when sitting days change. For example: the treaty procedure set out in the Constitutional Reform and Governance Act 2010 specifies no limitation on the length of any extension to objection period A. Should a Government minister choose to extend period A, dates on any business items actualising clock end steps cannot be automatically updated. The work package is marked as frozen and any changes to dates are manually updated."@en ;
	rdfs:domain ppr:ProceduralWorkPackage ;
	rdfs:range xsd:boolean ;
	rdfs:isDefinedBy <http://parliament.uk/ontologies/procedure/> .
	
ppr:workPackageDayCount rdf:type owl:DatatypeProperty ;
	rdfs:label "Work package day count"@en ;
	rdfs:comment "Relates a work package to the number of days of a type - as defined by the calculation style applied to the work package - to be counted by any clock in the procedure the work package is subject to. Where a work package day count is set, its value overrides the day counts set on clocks in the procedure that work package is subject to."@en ;
	rdfs:domain ppr:ProceduralWorkPackage ;
	rdfs:range xsd:integer ;
	rdfs:isDefinedBy <http://parliament.uk/ontologies/procedure/> .
	
ppr:dayCount rdf:type owl:DatatypeProperty ;
	rdfs:label "Day count"@en ;
	rdfs:comment "Relates a clock to the number of days of a type - as defined by the calculation style applied to the work package - to be counted by that clock. The day count of a clock may be overridden by the day count set on a work package. Clock day counts in the made affirmative procedure are not set, day counts being set on the work package."@en ;
	rdfs:domain ppr:Clock ;
	rdfs:range xsd:integer ;
	rdfs:isDefinedBy <http://parliament.uk/ontologies/procedure/> .
	
ppr:displayDepth rdf:type owl:DatatypeProperty ;
	rdfs:label "Display depth"@en ;
	rdfs:comment "Relates a step display depth in a procedure to the depth value of the step in that procedure. The depth value is stored as a float in order to allow for the insertion of new steps into a procedure without having to renumber existing steps, for example: 1, 1.12, 2, 3."@en ;
	rdfs:domain ppr:StepDisplayDepthInProcedure ;
	rdfs:range xsd:float ;
	rdfs:isDefinedBy <http://parliament.uk/ontologies/procedure/> .
